<?xml version="1.0"?>
<rdf:RDF xmlns="http://openenergy-platform.org/ontology/oeo/oeo-social/"
     xml:base="http://openenergy-platform.org/ontology/oeo/oeo-social/"
     xmlns:dc="http://purl.org/dc/elements/1.1/"
     xmlns:uo="http://purl.obolibrary.org/obo/uo#"
     xmlns:obo="http://purl.obolibrary.org/obo/"
     xmlns:oeo="http://openenergy-platform.org/ontology/oeo/"
     xmlns:owl="http://www.w3.org/2002/07/owl#"
     xmlns:rdf="http://www.w3.org/1999/02/22-rdf-syntax-ns#"
     xmlns:xml="http://www.w3.org/XML/1998/namespace"
     xmlns:xsd="http://www.w3.org/2001/XMLSchema#"
     xmlns:foaf="http://xmlns.com/foaf/0.1/"
     xmlns:rdfs="http://www.w3.org/2000/01/rdf-schema#"
     xmlns:terms="http://purl.org/dc/terms/"
     xmlns:protege="http://protege.stanford.edu/plugins/owl/protege#"
     xmlns:oboInOwl="http://www.geneontology.org/formats/oboInOwl#">
    <owl:Ontology rdf:about="http://openenergy-platform.org/ontology/oeo/oeo-social/">
        <owl:versionIRI rdf:resource="http://openenergy-platform.org/ontology/oeo/releases/1.12.0/oeo-social.omn"/>
        <owl:imports rdf:resource="http://openenergy-platform.org/ontology/oeo/releases/1.12.0/oeo-shared.omn"/>
        <dc:description>The Open Energy Ontology is an ontology for all aspects of the energy modelling domain. The &apos;Social&apos; module covers entities that relate to people and the social, organisational and economic environment in which energy is produced and consumed, including sector, organisation, and various roles.</dc:description>
        <terms:license>http://creativecommons.org/publicdomain/zero/1.0/</terms:license>
        <terms:title>Open Energy Ontology (social module)</terms:title>
    </owl:Ontology>
    


    <!-- 
    ///////////////////////////////////////////////////////////////////////////////////////
    //
    // Annotation properties
    //
    ///////////////////////////////////////////////////////////////////////////////////////
     -->

    


    <!-- http://openenergy-platform.org/ontology/oeo/OEO_00010037 -->

    <owl:AnnotationProperty rdf:about="http://openenergy-platform.org/ontology/oeo/OEO_00010037"/>
    


    <!-- http://openenergy-platform.org/ontology/oeo/OEO_00040001 -->

    <owl:AnnotationProperty rdf:about="http://openenergy-platform.org/ontology/oeo/OEO_00040001"/>
    


    <!-- http://purl.obolibrary.org/obo/IAO_0000112 -->

    <owl:AnnotationProperty rdf:about="http://purl.obolibrary.org/obo/IAO_0000112"/>
    


    <!-- http://purl.obolibrary.org/obo/IAO_0000115 -->

    <owl:AnnotationProperty rdf:about="http://purl.obolibrary.org/obo/IAO_0000115"/>
    


    <!-- http://purl.obolibrary.org/obo/IAO_0000116 -->

    <owl:AnnotationProperty rdf:about="http://purl.obolibrary.org/obo/IAO_0000116"/>
    


    <!-- http://purl.obolibrary.org/obo/IAO_0000118 -->

    <owl:AnnotationProperty rdf:about="http://purl.obolibrary.org/obo/IAO_0000118"/>
    


    <!-- http://purl.obolibrary.org/obo/IAO_0000119 -->

    <owl:AnnotationProperty rdf:about="http://purl.obolibrary.org/obo/IAO_0000119"/>
    


    <!-- http://purl.obolibrary.org/obo/IAO_0000233 -->

    <owl:AnnotationProperty rdf:about="http://purl.obolibrary.org/obo/IAO_0000233"/>
    


    <!-- http://purl.org/dc/elements/1.1/contributor -->

    <owl:AnnotationProperty rdf:about="http://purl.org/dc/elements/1.1/contributor"/>
    


    <!-- http://purl.org/dc/elements/1.1/description -->

    <owl:AnnotationProperty rdf:about="http://purl.org/dc/elements/1.1/description"/>
    


    <!-- http://purl.org/dc/elements/1.1/identifier -->

    <owl:AnnotationProperty rdf:about="http://purl.org/dc/elements/1.1/identifier"/>
    


    <!-- http://purl.org/dc/terms/license -->

    <owl:AnnotationProperty rdf:about="http://purl.org/dc/terms/license"/>
    


    <!-- http://purl.org/dc/terms/source -->

    <owl:AnnotationProperty rdf:about="http://purl.org/dc/terms/source"/>
    


    <!-- http://purl.org/dc/terms/title -->

    <owl:AnnotationProperty rdf:about="http://purl.org/dc/terms/title"/>
    


    <!-- http://www.w3.org/2000/01/rdf-schema#comment -->

    <owl:AnnotationProperty rdf:about="http://www.w3.org/2000/01/rdf-schema#comment"/>
    


    <!-- http://www.w3.org/2000/01/rdf-schema#isDefinedBy -->

    <owl:AnnotationProperty rdf:about="http://www.w3.org/2000/01/rdf-schema#isDefinedBy"/>
    


    <!-- http://www.w3.org/2000/01/rdf-schema#label -->

    <owl:AnnotationProperty rdf:about="http://www.w3.org/2000/01/rdf-schema#label"/>
    


    <!-- http://www.w3.org/2000/01/rdf-schema#seeAlso -->

    <owl:AnnotationProperty rdf:about="http://www.w3.org/2000/01/rdf-schema#seeAlso"/>
    


    <!-- 
    ///////////////////////////////////////////////////////////////////////////////////////
    //
    // Datatypes
    //
    ///////////////////////////////////////////////////////////////////////////////////////
     -->

    


    <!-- http://www.w3.org/1999/02/22-rdf-syntax-ns#PlainLiteral -->

    <rdfs:Datatype rdf:about="http://www.w3.org/1999/02/22-rdf-syntax-ns#PlainLiteral"/>
    


    <!-- http://www.w3.org/2001/XMLSchema#string -->

    <rdfs:Datatype rdf:about="http://www.w3.org/2001/XMLSchema#string"/>
    


    <!-- 
    ///////////////////////////////////////////////////////////////////////////////////////
    //
    // Object Properties
    //
    ///////////////////////////////////////////////////////////////////////////////////////
     -->

    


    <!-- http://openenergy-platform.org/ontology/oeo/OEO_00000503 -->

    <owl:ObjectProperty rdf:about="http://openenergy-platform.org/ontology/oeo/OEO_00000503"/>
    


    <!-- http://openenergy-platform.org/ontology/oeo/OEO_00000504 -->

    <owl:ObjectProperty rdf:about="http://openenergy-platform.org/ontology/oeo/OEO_00000504">
        <rdfs:range rdf:resource="http://purl.obolibrary.org/obo/BFO_0000002"/>
        <obo:IAO_0000115>A relation between a continuant (A) and a continuant or occurent (B) in which (A) determines the semantic of (B)</obo:IAO_0000115>
        <obo:IAO_0000233>issue: https://github.com/OpenEnergyPlatform/ontology/issues/460
pull request: https://github.com/OpenEnergyPlatform/ontology/pull/480/

domain:
issue: https://github.com/OpenEnergyPlatform/ontology/issues/850
pull request: https://github.com/OpenEnergyPlatform/ontology/pull/871

adapt domains and ranges:
issue: https://github.com/OpenEnergyPlatform/ontology/issues/973
issue: https://github.com/OpenEnergyPlatform/ontology/pull/1085</obo:IAO_0000233>
        <rdfs:label>is defined by</rdfs:label>
    </owl:ObjectProperty>
    


    <!-- http://openenergy-platform.org/ontology/oeo/OEO_00000505 -->

    <owl:ObjectProperty rdf:about="http://openenergy-platform.org/ontology/oeo/OEO_00000505"/>
    


    <!-- http://openenergy-platform.org/ontology/oeo/OEO_00000506 -->

    <owl:ObjectProperty rdf:about="http://openenergy-platform.org/ontology/oeo/OEO_00000506"/>
    


    <!-- http://openenergy-platform.org/ontology/oeo/OEO_00000507 -->

    <owl:ObjectProperty rdf:about="http://openenergy-platform.org/ontology/oeo/OEO_00000507"/>
    


    <!-- http://openenergy-platform.org/ontology/oeo/OEO_00000508 -->

    <owl:ObjectProperty rdf:about="http://openenergy-platform.org/ontology/oeo/OEO_00000508"/>
    


    <!-- http://openenergy-platform.org/ontology/oeo/OEO_00000509 -->

    <owl:ObjectProperty rdf:about="http://openenergy-platform.org/ontology/oeo/OEO_00000509"/>
    


    <!-- http://openenergy-platform.org/ontology/oeo/OEO_00000510 -->

    <owl:ObjectProperty rdf:about="http://openenergy-platform.org/ontology/oeo/OEO_00000510"/>
    


    <!-- http://openenergy-platform.org/ontology/oeo/OEO_00000522 -->

    <owl:ObjectProperty rdf:about="http://openenergy-platform.org/ontology/oeo/OEO_00000522"/>
    


    <!-- http://openenergy-platform.org/ontology/oeo/OEO_00010119 -->

    <owl:ObjectProperty rdf:about="http://openenergy-platform.org/ontology/oeo/OEO_00010119">
        <rdfs:subPropertyOf rdf:resource="http://purl.obolibrary.org/obo/RO_0000056"/>
        <rdfs:domain rdf:resource="http://openenergy-platform.org/ontology/oeo/OEO_00140151"/>
        <rdfs:range rdf:resource="http://openenergy-platform.org/ontology/oeo/OEO_00140149"/>
        <obo:IAO_0000115>A relation between a policy instrument and a transformative measure where a policy instrument guides a transformative measure.</obo:IAO_0000115>
        <obo:IAO_0000233>issue: https://github.com/OpenEnergyPlatform/ontology/issues/444
pull request: https://github.com/OpenEnergyPlatform/ontology/pull/853</obo:IAO_0000233>
        <rdfs:label xml:lang="en">guides</rdfs:label>
    </owl:ObjectProperty>
    


    <!-- http://openenergy-platform.org/ontology/oeo/OEO_00010121 -->

    <owl:ObjectProperty rdf:about="http://openenergy-platform.org/ontology/oeo/OEO_00010121"/>
    


    <!-- http://openenergy-platform.org/ontology/oeo/OEO_00010128 -->

    <owl:ObjectProperty rdf:about="http://openenergy-platform.org/ontology/oeo/OEO_00010128">
        <rdfs:domain>
            <owl:Class>
                <owl:unionOf rdf:parseType="Collection">
                    <rdf:Description rdf:about="http://openenergy-platform.org/ontology/oeo/OEO_00140150"/>
                    <rdf:Description rdf:about="http://openenergy-platform.org/ontology/oeo/OEO_00140151"/>
                </owl:unionOf>
            </owl:Class>
        </rdfs:domain>
        <obo:IAO_0000115>A relation that holds between a policy or policy instrument and the thing it governs.</obo:IAO_0000115>
        <obo:IAO_0000233>issue: https://github.com/OpenEnergyPlatform/ontology/issues/855
pull request: https://github.com/OpenEnergyPlatform/ontology/pull/868</obo:IAO_0000233>
        <rdfs:label xml:lang="en">governs</rdfs:label>
    </owl:ObjectProperty>
    


    <!-- http://openenergy-platform.org/ontology/oeo/OEO_00010231 -->

    <owl:ObjectProperty rdf:about="http://openenergy-platform.org/ontology/oeo/OEO_00010231"/>
    


    <!-- http://openenergy-platform.org/ontology/oeo/OEO_00010232 -->

    <owl:ObjectProperty rdf:about="http://openenergy-platform.org/ontology/oeo/OEO_00010232">
        <rdfs:subPropertyOf rdf:resource="http://openenergy-platform.org/ontology/oeo/OEO_00010231"/>
        <rdfs:domain rdf:resource="http://openenergy-platform.org/ontology/oeo/OEO_00000367"/>
        <rdfs:range rdf:resource="http://openenergy-platform.org/ontology/oeo/OEO_00010227"/>
        <obo:IAO_0000115>A relation between a sector and a memo item.</obo:IAO_0000115>
        <obo:IAO_0000233>issue: https://github.com/OpenEnergyPlatform/ontology/issues/858
pull request: https://github.com/OpenEnergyPlatform/ontology/pull/965</obo:IAO_0000233>
        <rdfs:label>has memo item</rdfs:label>
    </owl:ObjectProperty>
    


    <!-- http://openenergy-platform.org/ontology/oeo/OEO_00010312 -->

    <owl:ObjectProperty rdf:about="http://openenergy-platform.org/ontology/oeo/OEO_00010312"/>
    


    <!-- http://openenergy-platform.org/ontology/oeo/OEO_00020056 -->

    <owl:ObjectProperty rdf:about="http://openenergy-platform.org/ontology/oeo/OEO_00020056"/>
    


    <!-- http://openenergy-platform.org/ontology/oeo/OEO_00020070 -->

    <owl:ObjectProperty rdf:about="http://openenergy-platform.org/ontology/oeo/OEO_00020070">
        <rdfs:subPropertyOf rdf:resource="http://www.w3.org/2002/07/owl#topObjectProperty"/>
        <owl:inverseOf rdf:resource="http://openenergy-platform.org/ontology/oeo/OEO_00020071"/>
        <rdfs:domain>
            <owl:Class>
                <owl:unionOf rdf:parseType="Collection">
                    <rdf:Description rdf:about="http://openenergy-platform.org/ontology/oeo/OEO_00010116"/>
                    <rdf:Description rdf:about="http://openenergy-platform.org/ontology/oeo/OEO_00020067"/>
                    <rdf:Description rdf:about="http://openenergy-platform.org/ontology/oeo/OEO_00140124"/>
                </owl:unionOf>
            </owl:Class>
        </rdfs:domain>
        <rdfs:range>
            <owl:Restriction>
                <owl:onProperty rdf:resource="http://purl.obolibrary.org/obo/RO_0000087"/>
                <owl:someValuesFrom rdf:resource="http://openenergy-platform.org/ontology/oeo/OEO_00040002"/>
            </owl:Restriction>
        </rdfs:range>
        <obo:IAO_0000115>Is traded at is a relation that holds between a market exchange and the financial instruments, commodities, or other products, services, or goods which are traded there.</obo:IAO_0000115>
        <obo:IAO_0000233>pull request: https://github.com/OpenEnergyPlatform/ontology/pull/748

change range:
issue: https://github.com/OpenEnergyPlatform/ontology/issues/791
pull request: https://github.com/OpenEnergyPlatform/ontology/pull/842

add domain:
issue: https://github.com/OpenEnergyPlatform/ontology/issues/973
pull request: https://github.com/OpenEnergyPlatform/ontology/pull/1127</obo:IAO_0000233>
        <rdfs:label>is traded at</rdfs:label>
    </owl:ObjectProperty>
    <owl:Axiom>
        <owl:annotatedSource rdf:resource="http://openenergy-platform.org/ontology/oeo/OEO_00020070"/>
        <owl:annotatedProperty rdf:resource="http://www.w3.org/2000/01/rdf-schema#domain"/>
        <owl:annotatedTarget>
            <owl:Class>
                <owl:unionOf rdf:parseType="Collection">
                    <rdf:Description rdf:about="http://openenergy-platform.org/ontology/oeo/OEO_00010116"/>
                    <rdf:Description rdf:about="http://openenergy-platform.org/ontology/oeo/OEO_00020067"/>
                    <rdf:Description rdf:about="http://openenergy-platform.org/ontology/oeo/OEO_00140124"/>
                </owl:unionOf>
            </owl:Class>
        </owl:annotatedTarget>
        <obo:IAO_0000116>Extension of domain to financial instrument and other products planned</obo:IAO_0000116>
    </owl:Axiom>
    


    <!-- http://openenergy-platform.org/ontology/oeo/OEO_00020071 -->

    <owl:ObjectProperty rdf:about="http://openenergy-platform.org/ontology/oeo/OEO_00020071">
        <rdfs:subPropertyOf rdf:resource="http://www.w3.org/2002/07/owl#topObjectProperty"/>
        <rdfs:domain>
            <owl:Restriction>
                <owl:onProperty rdf:resource="http://purl.obolibrary.org/obo/RO_0000087"/>
                <owl:someValuesFrom rdf:resource="http://openenergy-platform.org/ontology/oeo/OEO_00040002"/>
            </owl:Restriction>
        </rdfs:domain>
        <rdfs:range>
            <owl:Class>
                <owl:unionOf rdf:parseType="Collection">
                    <rdf:Description rdf:about="http://openenergy-platform.org/ontology/oeo/OEO_00010116"/>
                    <rdf:Description rdf:about="http://openenergy-platform.org/ontology/oeo/OEO_00020067"/>
                    <rdf:Description rdf:about="http://openenergy-platform.org/ontology/oeo/OEO_00140124"/>
                </owl:unionOf>
            </owl:Class>
        </rdfs:range>
        <obo:IAO_0000115>A relation that holds between financial instruments, commodities, or other products, services, or goods and a market exchange.</obo:IAO_0000115>
        <obo:IAO_0000233>pull request: https://github.com/OpenEnergyPlatform/ontology/pull/748

add domain and range:
issue: https://github.com/OpenEnergyPlatform/ontology/issues/973
pull request: https://github.com/OpenEnergyPlatform/ontology/pull/1127</obo:IAO_0000233>
        <rdfs:label>trades</rdfs:label>
    </owl:ObjectProperty>
    <owl:Axiom>
        <owl:annotatedSource rdf:resource="http://openenergy-platform.org/ontology/oeo/OEO_00020071"/>
        <owl:annotatedProperty rdf:resource="http://www.w3.org/2000/01/rdf-schema#range"/>
        <owl:annotatedTarget>
            <owl:Class>
                <owl:unionOf rdf:parseType="Collection">
                    <rdf:Description rdf:about="http://openenergy-platform.org/ontology/oeo/OEO_00010116"/>
                    <rdf:Description rdf:about="http://openenergy-platform.org/ontology/oeo/OEO_00020067"/>
                    <rdf:Description rdf:about="http://openenergy-platform.org/ontology/oeo/OEO_00140124"/>
                </owl:unionOf>
            </owl:Class>
        </owl:annotatedTarget>
        <obo:IAO_0000116>Extension of range to financial instrument and other products planned</obo:IAO_0000116>
    </owl:Axiom>
    


    <!-- http://openenergy-platform.org/ontology/oeo/OEO_00040010 -->

    <owl:ObjectProperty rdf:about="http://openenergy-platform.org/ontology/oeo/OEO_00040010"/>
    


    <!-- http://openenergy-platform.org/ontology/oeo/OEO_00140008 -->

    <owl:ObjectProperty rdf:about="http://openenergy-platform.org/ontology/oeo/OEO_00140008"/>
    


    <!-- http://openenergy-platform.org/ontology/oeo/OEO_00140017 -->

    <owl:ObjectProperty rdf:about="http://openenergy-platform.org/ontology/oeo/OEO_00140017">
        <rdfs:domain rdf:resource="http://openenergy-platform.org/ontology/oeo/OEO_00000323"/>
        <rdfs:range rdf:resource="http://openenergy-platform.org/ontology/oeo/OEO_00030022"/>
        <obo:IAO_0000115>A relation between a person and an organisation where the person is a member of the organisation.</obo:IAO_0000115>
        <obo:IAO_0000233>issue: https://github.com/OpenEnergyPlatform/ontology/issues/486
pull request: https://github.com/OpenEnergyPlatform/ontology/pull/562</obo:IAO_0000233>
        <rdfs:label xml:lang="en">member of</rdfs:label>
    </owl:ObjectProperty>
    


    <!-- http://openenergy-platform.org/ontology/oeo/OEO_00140018 -->

    <owl:ObjectProperty rdf:about="http://openenergy-platform.org/ontology/oeo/OEO_00140018">
        <rdfs:subPropertyOf rdf:resource="http://www.w3.org/2002/07/owl#topObjectProperty"/>
        <rdfs:domain rdf:resource="http://openenergy-platform.org/ontology/oeo/OEO_00030022"/>
        <rdfs:range rdf:resource="http://openenergy-platform.org/ontology/oeo/OEO_00000323"/>
        <obo:IAO_0000115>A relation between an organisation and a person where the person is a member of the organisation.</obo:IAO_0000115>
        <obo:IAO_0000233>issue: https://github.com/OpenEnergyPlatform/ontology/issues/486
pull request: https://github.com/OpenEnergyPlatform/ontology/pull/562</obo:IAO_0000233>
        <rdfs:label xml:lang="en">has member</rdfs:label>
    </owl:ObjectProperty>
    


    <!-- http://openenergy-platform.org/ontology/oeo/OEO_00140164 -->

    <owl:ObjectProperty rdf:about="http://openenergy-platform.org/ontology/oeo/OEO_00140164"/>
    


    <!-- http://purl.obolibrary.org/obo/BFO_0000050 -->

    <owl:ObjectProperty rdf:about="http://purl.obolibrary.org/obo/BFO_0000050"/>
    


    <!-- http://purl.obolibrary.org/obo/BFO_0000051 -->

    <owl:ObjectProperty rdf:about="http://purl.obolibrary.org/obo/BFO_0000051"/>
    


    <!-- http://purl.obolibrary.org/obo/IAO_0000136 -->

    <owl:ObjectProperty rdf:about="http://purl.obolibrary.org/obo/IAO_0000136"/>
    


    <!-- http://purl.obolibrary.org/obo/RO_0000056 -->

    <owl:ObjectProperty rdf:about="http://purl.obolibrary.org/obo/RO_0000056"/>
    


    <!-- http://purl.obolibrary.org/obo/RO_0000057 -->

    <owl:ObjectProperty rdf:about="http://purl.obolibrary.org/obo/RO_0000057"/>
    


    <!-- http://purl.obolibrary.org/obo/RO_0000086 -->

    <owl:ObjectProperty rdf:about="http://purl.obolibrary.org/obo/RO_0000086"/>
    


    <!-- http://purl.obolibrary.org/obo/RO_0000087 -->

    <owl:ObjectProperty rdf:about="http://purl.obolibrary.org/obo/RO_0000087"/>
    


    <!-- http://www.w3.org/2002/07/owl#topObjectProperty -->

    <owl:ObjectProperty rdf:about="http://www.w3.org/2002/07/owl#topObjectProperty"/>
    


    <!-- 
    ///////////////////////////////////////////////////////////////////////////////////////
    //
    // Classes
    //
    ///////////////////////////////////////////////////////////////////////////////////////
     -->

    


    <!-- http://openenergy-platform.org/ontology/oeo/OEO_00000006 -->

    <owl:Class rdf:about="http://openenergy-platform.org/ontology/oeo/OEO_00000006">
        <rdfs:subClassOf rdf:resource="http://openenergy-platform.org/ontology/oeo/OEO_00000331"/>
        <rdfs:label xml:lang="en">carbon dioxide</rdfs:label>
    </owl:Class>
    


    <!-- http://openenergy-platform.org/ontology/oeo/OEO_00000045 -->

    <owl:Class rdf:about="http://openenergy-platform.org/ontology/oeo/OEO_00000045">
        <rdfs:subClassOf rdf:resource="http://openenergy-platform.org/ontology/oeo/OEO_00000051"/>
        <rdfs:subClassOf>
            <owl:Restriction>
                <owl:onProperty rdf:resource="http://purl.obolibrary.org/obo/RO_0000056"/>
                <owl:someValuesFrom rdf:resource="http://openenergy-platform.org/ontology/oeo/OEO_00240003"/>
            </owl:Restriction>
        </rdfs:subClassOf>
        <oeo:OEO_00040001 rdf:datatype="http://www.w3.org/2001/XMLSchema#string">http://openenergy-platform.org/ontology/oeo/oeo-social</oeo:OEO_00040001>
        <obo:IAO_0000115>A producer is an agent that makes goods.</obo:IAO_0000115>
        <obo:IAO_0000233>issue: https://github.com/OpenEnergyPlatform/ontology/issues/835
pull request: https://github.com/OpenEnergyPlatform/ontology/pull/845

issue: https://github.com/OpenEnergyPlatform/ontology/issues/314
pull request: https://github.com/OpenEnergyPlatform/ontology/pull/370</obo:IAO_0000233>
        <rdfs:label>producer</rdfs:label>
    </owl:Class>
    


    <!-- http://openenergy-platform.org/ontology/oeo/OEO_00000051 -->

    <owl:Class rdf:about="http://openenergy-platform.org/ontology/oeo/OEO_00000051"/>
    


    <!-- http://openenergy-platform.org/ontology/oeo/OEO_00000064 -->

    <owl:Class rdf:about="http://openenergy-platform.org/ontology/oeo/OEO_00000064"/>
    


    <!-- http://openenergy-platform.org/ontology/oeo/OEO_00000087 -->

    <owl:Class rdf:about="http://openenergy-platform.org/ontology/oeo/OEO_00000087"/>
    


    <!-- http://openenergy-platform.org/ontology/oeo/OEO_00000105 -->

    <owl:Class rdf:about="http://openenergy-platform.org/ontology/oeo/OEO_00000105">
        <rdfs:subClassOf rdf:resource="http://openenergy-platform.org/ontology/oeo/OEO_00000431"/>
        <oeo:OEO_00040001 rdf:datatype="http://www.w3.org/2001/XMLSchema#string">http://openenergy-platform.org/ontology/oeo/oeo-social</oeo:OEO_00040001>
        <obo:IAO_0000115 xml:lang="en">A consumer is a user of a commercial product or service.</obo:IAO_0000115>
        <rdfs:label>consumer</rdfs:label>
    </owl:Class>
    


    <!-- http://openenergy-platform.org/ontology/oeo/OEO_00000107 -->

    <owl:Class rdf:about="http://openenergy-platform.org/ontology/oeo/OEO_00000107"/>
    


    <!-- http://openenergy-platform.org/ontology/oeo/OEO_00000128 -->

    <owl:Class rdf:about="http://openenergy-platform.org/ontology/oeo/OEO_00000128">
        <rdfs:subClassOf rdf:resource="http://openenergy-platform.org/ontology/oeo/OEO_00000367"/>
        <oeo:OEO_00040001 rdf:datatype="http://www.w3.org/2001/XMLSchema#string">http://openenergy-platform.org/ontology/oeo/oeo-social</oeo:OEO_00040001>
        <obo:IAO_0000115 xml:lang="en">An energy demand sector is a sector that covers energy consumers.</obo:IAO_0000115>
        <obo:IAO_0000118>final energy sector</obo:IAO_0000118>
        <obo:IAO_0000233>issue: https://github.com/OpenEnergyPlatform/ontology/issues/30
pull request: https://github.com/OpenEnergyPlatform/ontology/pull/484</obo:IAO_0000233>
        <rdfs:label>energy demand sector</rdfs:label>
    </owl:Class>
    <owl:Axiom>
        <owl:annotatedSource rdf:resource="http://openenergy-platform.org/ontology/oeo/OEO_00000128"/>
        <owl:annotatedProperty rdf:resource="http://purl.obolibrary.org/obo/IAO_0000118"/>
        <owl:annotatedTarget>final energy sector</owl:annotatedTarget>
        <obo:IAO_0000233>issue: https://github.com/OpenEnergyPlatform/ontology/issues/1014
pull request: https://github.com/OpenEnergyPlatform/ontology/pull/1015</obo:IAO_0000233>
    </owl:Axiom>
    


    <!-- http://openenergy-platform.org/ontology/oeo/OEO_00000145 -->

    <owl:Class rdf:about="http://openenergy-platform.org/ontology/oeo/OEO_00000145">
        <rdfs:subClassOf rdf:resource="http://openenergy-platform.org/ontology/oeo/OEO_00000158"/>
        <oeo:OEO_00040001 rdf:datatype="http://www.w3.org/2001/XMLSchema#string">http://openenergy-platform.org/ontology/oeo/oeo-social</oeo:OEO_00040001>
        <obo:IAO_0000115 xml:lang="en">An electricity sector is a transformation sector that covers electricity generation and transport of electrical energy to consumers of electrical energy.</obo:IAO_0000115>
        <obo:IAO_0000233>issue: https://github.com/OpenEnergyPlatform/ontology/issues/30
pull request: https://github.com/OpenEnergyPlatform/ontology/pull/484</obo:IAO_0000233>
        <rdfs:label>electricity sector</rdfs:label>
    </owl:Class>
    


    <!-- http://openenergy-platform.org/ontology/oeo/OEO_00000147 -->

    <owl:Class rdf:about="http://openenergy-platform.org/ontology/oeo/OEO_00000147"/>
    


    <!-- http://openenergy-platform.org/ontology/oeo/OEO_00000158 -->

    <owl:Class rdf:about="http://openenergy-platform.org/ontology/oeo/OEO_00000158">
        <rdfs:subClassOf rdf:resource="http://openenergy-platform.org/ontology/oeo/OEO_00000367"/>
        <oeo:OEO_00040001 rdf:datatype="http://www.w3.org/2001/XMLSchema#string">http://openenergy-platform.org/ontology/oeo/oeo-social</oeo:OEO_00040001>
        <obo:IAO_0000115>An energy transformation sector is a sector that covers energy production, energy transformation from primary to secondary energy and transport of energy to the demand sector.</obo:IAO_0000115>
        <obo:IAO_0000118>energy industry sector</obo:IAO_0000118>
        <obo:IAO_0000118>energy sector</obo:IAO_0000118>
        <obo:IAO_0000233>issue: https://github.com/OpenEnergyPlatform/ontology/issues/30
pull request: https://github.com/OpenEnergyPlatform/ontology/pull/484</obo:IAO_0000233>
        <rdfs:label>energy transformation sector</rdfs:label>
    </owl:Class>
    


    <!-- http://openenergy-platform.org/ontology/oeo/OEO_00000213 -->

    <owl:Class rdf:about="http://openenergy-platform.org/ontology/oeo/OEO_00000213">
        <rdfs:subClassOf rdf:resource="http://openenergy-platform.org/ontology/oeo/OEO_00000128"/>
        <oeo:OEO_00040001 rdf:datatype="http://www.w3.org/2001/XMLSchema#string">http://openenergy-platform.org/ontology/oeo/oeo-social</oeo:OEO_00040001>
        <obo:IAO_0000115 xml:lang="en">A heating and cooling sector is a sector that covers heating and cooling activities.</obo:IAO_0000115>
        <obo:IAO_0000118>H&amp;C sector</obo:IAO_0000118>
        <obo:IAO_0000233>issue: https://github.com/OpenEnergyPlatform/ontology/issues/30
pull request: https://github.com/OpenEnergyPlatform/ontology/pull/484</obo:IAO_0000233>
        <rdfs:label>heating and cooling sector</rdfs:label>
    </owl:Class>
    


    <!-- http://openenergy-platform.org/ontology/oeo/OEO_00000214 -->

    <owl:Class rdf:about="http://openenergy-platform.org/ontology/oeo/OEO_00000214">
        <rdfs:subClassOf rdf:resource="http://openenergy-platform.org/ontology/oeo/OEO_00000128"/>
        <oeo:OEO_00040001 rdf:datatype="http://www.w3.org/2001/XMLSchema#string">http://openenergy-platform.org/ontology/oeo/oeo-social</oeo:OEO_00040001>
        <obo:IAO_0000115 xml:lang="en">A household sector is a sector that covers households.</obo:IAO_0000115>
        <obo:IAO_0000118>private household sector</obo:IAO_0000118>
        <obo:IAO_0000233>issue: https://github.com/OpenEnergyPlatform/ontology/issues/30
pull request: https://github.com/OpenEnergyPlatform/ontology/pull/484</obo:IAO_0000233>
        <rdfs:label>household sector</rdfs:label>
    </owl:Class>
    


    <!-- http://openenergy-platform.org/ontology/oeo/OEO_00000227 -->

    <owl:Class rdf:about="http://openenergy-platform.org/ontology/oeo/OEO_00000227">
        <rdfs:subClassOf rdf:resource="http://openenergy-platform.org/ontology/oeo/OEO_00000367"/>
        <oeo:OEO_00040001 rdf:datatype="http://www.w3.org/2001/XMLSchema#string">http://openenergy-platform.org/ontology/oeo/oeo-social</oeo:OEO_00040001>
        <obo:IAO_0000115 xml:lang="en">An industry sector is a sector that covers industrial activities with other main purposes of energy transformation.</obo:IAO_0000115>
        <obo:IAO_0000233>issue: https://github.com/OpenEnergyPlatform/ontology/issues/30
pull request: https://github.com/OpenEnergyPlatform/ontology/pull/484</obo:IAO_0000233>
        <rdfs:label>industry sector</rdfs:label>
    </owl:Class>
    


    <!-- http://openenergy-platform.org/ontology/oeo/OEO_00000238 -->

    <owl:Class rdf:about="http://openenergy-platform.org/ontology/oeo/OEO_00000238"/>
    


    <!-- http://openenergy-platform.org/ontology/oeo/OEO_00000264 -->

    <owl:Class rdf:about="http://openenergy-platform.org/ontology/oeo/OEO_00000264">
        <rdfs:subClassOf>
            <owl:Restriction>
                <owl:onProperty rdf:resource="http://openenergy-platform.org/ontology/oeo/OEO_00140164"/>
                <owl:someValuesFrom rdf:resource="http://openenergy-platform.org/ontology/oeo/OEO_00020065"/>
            </owl:Restriction>
        </rdfs:subClassOf>
    </owl:Class>
    <owl:Axiom>
        <owl:annotatedSource rdf:resource="http://openenergy-platform.org/ontology/oeo/OEO_00000264"/>
        <owl:annotatedProperty rdf:resource="http://www.w3.org/2000/01/rdf-schema#subClassOf"/>
        <owl:annotatedTarget>
            <owl:Restriction>
                <owl:onProperty rdf:resource="http://openenergy-platform.org/ontology/oeo/OEO_00140164"/>
                <owl:someValuesFrom rdf:resource="http://openenergy-platform.org/ontology/oeo/OEO_00020065"/>
            </owl:Restriction>
        </owl:annotatedTarget>
        <obo:IAO_0000233>issue: https://github.com/OpenEnergyPlatform/ontology/issues/415
pull request: https://github.com/OpenEnergyPlatform/ontology/pull/821</obo:IAO_0000233>
    </owl:Axiom>
    


    <!-- http://openenergy-platform.org/ontology/oeo/OEO_00000315 -->

    <owl:Class rdf:about="http://openenergy-platform.org/ontology/oeo/OEO_00000315"/>
    


    <!-- http://openenergy-platform.org/ontology/oeo/OEO_00000323 -->

    <owl:Class rdf:about="http://openenergy-platform.org/ontology/oeo/OEO_00000323"/>
    


    <!-- http://openenergy-platform.org/ontology/oeo/OEO_00000329 -->

    <owl:Class rdf:about="http://openenergy-platform.org/ontology/oeo/OEO_00000329">
        <rdfs:subClassOf rdf:resource="http://openenergy-platform.org/ontology/oeo/OEO_00030022"/>
        <oeo:OEO_00040001 rdf:datatype="http://www.w3.org/2001/XMLSchema#string">http://openenergy-platform.org/ontology/oeo/oeo-social</oeo:OEO_00040001>
        <obo:IAO_0000115 xml:lang="en">A political party is a organisation of a group of people with common views or goals that wants to have influence in politics.</obo:IAO_0000115>
        <rdfs:label>political party</rdfs:label>
    </owl:Class>
    


    <!-- http://openenergy-platform.org/ontology/oeo/OEO_00000331 -->

    <owl:Class rdf:about="http://openenergy-platform.org/ontology/oeo/OEO_00000331"/>
    


    <!-- http://openenergy-platform.org/ontology/oeo/OEO_00000341 -->

    <owl:Class rdf:about="http://openenergy-platform.org/ontology/oeo/OEO_00000341">
        <rdfs:subClassOf rdf:resource="http://openenergy-platform.org/ontology/oeo/OEO_00000051"/>
        <oeo:OEO_00040001 rdf:datatype="http://www.w3.org/2001/XMLSchema#string">http://openenergy-platform.org/ontology/oeo/oeo-social</oeo:OEO_00040001>
        <obo:IAO_0000115 xml:lang="en">A prosumer is an agent who is producer and consumer at the same time.</obo:IAO_0000115>
        <rdfs:label>prosumer</rdfs:label>
    </owl:Class>
    


    <!-- http://openenergy-platform.org/ontology/oeo/OEO_00000350 -->

    <owl:Class rdf:about="http://openenergy-platform.org/ontology/oeo/OEO_00000350"/>
    


    <!-- http://openenergy-platform.org/ontology/oeo/OEO_00000367 -->

    <owl:Class rdf:about="http://openenergy-platform.org/ontology/oeo/OEO_00000367"/>
    


    <!-- http://openenergy-platform.org/ontology/oeo/OEO_00000368 -->

    <owl:Class rdf:about="http://openenergy-platform.org/ontology/oeo/OEO_00000368">
        <rdfs:subClassOf rdf:resource="http://purl.obolibrary.org/obo/BFO_0000031"/>
        <oeo:OEO_00040001 rdf:datatype="http://www.w3.org/2001/XMLSchema#string">http://openenergy-platform.org/ontology/oeo/oeo-social</oeo:OEO_00040001>
        <obo:IAO_0000115 xml:lang="en">A sector division is a specific way to subdivide a system.</obo:IAO_0000115>
        <obo:IAO_0000233>issue: https://github.com/OpenEnergyPlatform/ontology/issues/30</obo:IAO_0000233>
        <rdfs:label>sector division</rdfs:label>
    </owl:Class>
    


    <!-- http://openenergy-platform.org/ontology/oeo/OEO_00000379 -->

    <owl:Class rdf:about="http://openenergy-platform.org/ontology/oeo/OEO_00000379">
        <rdfs:subClassOf rdf:resource="http://openenergy-platform.org/ontology/oeo/OEO_00000051"/>
        <oeo:OEO_00040001 rdf:datatype="http://www.w3.org/2001/XMLSchema#string">http://openenergy-platform.org/ontology/oeo/oeo-social</oeo:OEO_00040001>
        <obo:IAO_0000115>A software developer is an agent that creates computer software.</obo:IAO_0000115>
        <rdfs:label>software developer</rdfs:label>
    </owl:Class>
    


    <!-- http://openenergy-platform.org/ontology/oeo/OEO_00000405 -->

    <owl:Class rdf:about="http://openenergy-platform.org/ontology/oeo/OEO_00000405">
        <rdfs:subClassOf rdf:resource="http://openenergy-platform.org/ontology/oeo/OEO_00000128"/>
        <oeo:OEO_00040001 rdf:datatype="http://www.w3.org/2001/XMLSchema#string">http://openenergy-platform.org/ontology/oeo/oeo-social</oeo:OEO_00040001>
        <obo:IAO_0000115 xml:lang="en">A commercial sector is a sector that covers non-industrial commercial activities.</obo:IAO_0000115>
        <obo:IAO_0000118>TCS sector</obo:IAO_0000118>
        <obo:IAO_0000118>service sector</obo:IAO_0000118>
        <obo:IAO_0000118>trading, commerce and service sector</obo:IAO_0000118>
        <obo:IAO_0000233>issue: https://github.com/OpenEnergyPlatform/ontology/issues/30
pull request: https://github.com/OpenEnergyPlatform/ontology/pull/484</obo:IAO_0000233>
        <rdfs:label>commercial sector</rdfs:label>
    </owl:Class>
    


    <!-- http://openenergy-platform.org/ontology/oeo/OEO_00000422 -->

    <owl:Class rdf:about="http://openenergy-platform.org/ontology/oeo/OEO_00000422">
        <rdfs:subClassOf rdf:resource="http://openenergy-platform.org/ontology/oeo/OEO_00000128"/>
        <oeo:OEO_00040001 rdf:datatype="http://www.w3.org/2001/XMLSchema#string">http://openenergy-platform.org/ontology/oeo/oeo-social</oeo:OEO_00040001>
        <obo:IAO_0000115 xml:lang="en">A transport sector is a sector that covers transport of people and/or goods.</obo:IAO_0000115>
        <obo:IAO_0000118>traffic sector</obo:IAO_0000118>
        <obo:IAO_0000233>issue: https://github.com/OpenEnergyPlatform/ontology/issues/30
pull request: https://github.com/OpenEnergyPlatform/ontology/pull/484</obo:IAO_0000233>
        <rdfs:label>transport sector</rdfs:label>
    </owl:Class>
    


    <!-- http://openenergy-platform.org/ontology/oeo/OEO_00000431 -->

    <owl:Class rdf:about="http://openenergy-platform.org/ontology/oeo/OEO_00000431">
        <rdfs:subClassOf rdf:resource="http://openenergy-platform.org/ontology/oeo/OEO_00000051"/>
        <oeo:OEO_00040001 rdf:datatype="http://www.w3.org/2001/XMLSchema#string">http://openenergy-platform.org/ontology/oeo/oeo-social</oeo:OEO_00040001>
        <obo:IAO_0000115>A user is an agent that employs an aid, tool or information system to achieve a goal/benefit.</obo:IAO_0000115>
        <rdfs:label>user</rdfs:label>
    </owl:Class>
    


    <!-- http://openenergy-platform.org/ontology/oeo/OEO_00010034 -->

    <owl:Class rdf:about="http://openenergy-platform.org/ontology/oeo/OEO_00010034">
        <rdfs:subClassOf rdf:resource="http://openenergy-platform.org/ontology/oeo/OEO_00000128"/>
        <oeo:OEO_00040001 rdf:datatype="http://www.w3.org/2001/XMLSchema#string">http://openenergy-platform.org/ontology/oeo/oeo-social</oeo:OEO_00040001>
        <obo:IAO_0000115>A building sector is a sector that covers buildings.</obo:IAO_0000115>
        <obo:IAO_0000233>issue: https://github.com/OpenEnergyPlatform/ontology/issues/30
pull request: https://github.com/OpenEnergyPlatform/ontology/pull/484</obo:IAO_0000233>
        <rdfs:label>building sector</rdfs:label>
    </owl:Class>
    


    <!-- http://openenergy-platform.org/ontology/oeo/OEO_00010035 -->

    <owl:Class rdf:about="http://openenergy-platform.org/ontology/oeo/OEO_00010035">
        <rdfs:subClassOf rdf:resource="http://openenergy-platform.org/ontology/oeo/OEO_00000367"/>
        <oeo:OEO_00040001 rdf:datatype="http://www.w3.org/2001/XMLSchema#string">http://openenergy-platform.org/ontology/oeo/oeo-social</oeo:OEO_00040001>
        <obo:IAO_0000115>A agriculture, forestry and land use (AFOLU) sector is a sector that covers activities and natural processes from agriculture, forestry, land use and land use change.</obo:IAO_0000115>
        <obo:IAO_0000118>AFOLU sector</obo:IAO_0000118>
        <obo:IAO_0000233>issue: https://github.com/OpenEnergyPlatform/ontology/issues/30
pull request: https://github.com/OpenEnergyPlatform/ontology/pull/484</obo:IAO_0000233>
        <rdfs:label>agriculture, forestry and land use sector</rdfs:label>
    </owl:Class>
    


    <!-- http://openenergy-platform.org/ontology/oeo/OEO_00010036 -->

    <owl:Class rdf:about="http://openenergy-platform.org/ontology/oeo/OEO_00010036">
        <rdfs:subClassOf rdf:resource="http://openenergy-platform.org/ontology/oeo/OEO_00000367"/>
        <oeo:OEO_00040001 rdf:datatype="http://www.w3.org/2001/XMLSchema#string">http://openenergy-platform.org/ontology/oeo/oeo-social</oeo:OEO_00040001>
        <obo:IAO_0000115>A waste and wastewater sector is a sector that covers activities related the collection and treatment of waste and wastewater.</obo:IAO_0000115>
        <obo:IAO_0000233>issue: https://github.com/OpenEnergyPlatform/ontology/issues/30
pull request: https://github.com/OpenEnergyPlatform/ontology/pull/484</obo:IAO_0000233>
        <rdfs:label>waste and wastewater sector</rdfs:label>
    </owl:Class>
    


    <!-- http://openenergy-platform.org/ontology/oeo/OEO_00010055 -->

    <owl:Class rdf:about="http://openenergy-platform.org/ontology/oeo/OEO_00010055">
        <rdfs:subClassOf rdf:resource="http://openenergy-platform.org/ontology/oeo/OEO_00000368"/>
        <oeo:OEO_00040001 rdf:datatype="http://www.w3.org/2001/XMLSchema#string">http://openenergy-platform.org/ontology/oeo/oeo-social</oeo:OEO_00040001>
        <obo:IAO_0000115>The common reporting format (CRF) is a sector division used for compiling national inventory reports on greenhouse gas emissions and providing emission relevant data in so called CRF tables.</obo:IAO_0000115>
        <obo:IAO_0000118>CRF</obo:IAO_0000118>
        <obo:IAO_0000233>issue: https://github.com/OpenEnergyPlatform/ontology/issues/461
pull request: https://github.com/OpenEnergyPlatform/ontology/pull/578</obo:IAO_0000233>
        <rdfs:label>common reporting format</rdfs:label>
    </owl:Class>
    


    <!-- http://openenergy-platform.org/ontology/oeo/OEO_00010079 -->

    <owl:Class rdf:about="http://openenergy-platform.org/ontology/oeo/OEO_00010079">
        <rdfs:subClassOf>
            <owl:Restriction>
                <owl:onProperty rdf:resource="http://openenergy-platform.org/ontology/oeo/OEO_00020056"/>
                <owl:someValuesFrom rdf:resource="http://openenergy-platform.org/ontology/oeo/OEO_00020063"/>
            </owl:Restriction>
        </rdfs:subClassOf>
    </owl:Class>
    


    <!-- http://openenergy-platform.org/ontology/oeo/OEO_00010082 -->

    <owl:Class rdf:about="http://openenergy-platform.org/ontology/oeo/OEO_00010082">
        <rdfs:subClassOf rdf:resource="http://purl.obolibrary.org/obo/BFO_0000015"/>
        <rdfs:subClassOf>
            <owl:Restriction>
                <owl:onProperty rdf:resource="http://purl.obolibrary.org/obo/RO_0000057"/>
                <owl:someValuesFrom rdf:resource="http://openenergy-platform.org/ontology/oeo/OEO_00040011"/>
            </owl:Restriction>
        </rdfs:subClassOf>
        <oeo:OEO_00040001 rdf:datatype="http://www.w3.org/2001/XMLSchema#string">http://openenergy-platform.org/ontology/oeo/oeo-social</oeo:OEO_00040001>
        <obo:IAO_0000115>A trade is a process in which one commodity or service is exchanged for another commodity or service.</obo:IAO_0000115>
        <obo:IAO_0000233>issue: https://github.com/OpenEnergyPlatform/ontology/issues/307
pull request: https://github.com/OpenEnergyPlatform/ontology/pull/745</obo:IAO_0000233>
        <rdfs:label xml:lang="en">trade</rdfs:label>
    </owl:Class>
    


    <!-- http://openenergy-platform.org/ontology/oeo/OEO_00010083 -->

    <owl:Class rdf:about="http://openenergy-platform.org/ontology/oeo/OEO_00010083">
        <rdfs:subClassOf rdf:resource="http://openenergy-platform.org/ontology/oeo/OEO_00000051"/>
        <rdfs:subClassOf>
            <owl:Restriction>
                <owl:onProperty rdf:resource="http://purl.obolibrary.org/obo/RO_0000056"/>
                <owl:someValuesFrom rdf:resource="http://openenergy-platform.org/ontology/oeo/OEO_00010082"/>
            </owl:Restriction>
        </rdfs:subClassOf>
        <oeo:OEO_00040001 rdf:datatype="http://www.w3.org/2001/XMLSchema#string">http://openenergy-platform.org/ontology/oeo/oeo-social</oeo:OEO_00040001>
        <obo:IAO_0000115>A market participant is an agent who participates in trading in a market exchange.</obo:IAO_0000115>
        <obo:IAO_0000233>issue: https://github.com/OpenEnergyPlatform/ontology/issues/330
pull request: https://github.com/OpenEnergyPlatform/ontology/pull/745

update definition and improve axiom:
https://github.com/OpenEnergyPlatform/ontology/issues/617
https://github.com/OpenEnergyPlatform/ontology/pull/1019</obo:IAO_0000233>
        <rdfs:label xml:lang="en">market participant</rdfs:label>
    </owl:Class>
    


    <!-- http://openenergy-platform.org/ontology/oeo/OEO_00010115 -->

    <owl:Class rdf:about="http://openenergy-platform.org/ontology/oeo/OEO_00010115">
        <rdfs:subClassOf rdf:resource="http://purl.obolibrary.org/obo/RO_0002577"/>
        <oeo:OEO_00040001 rdf:datatype="http://www.w3.org/2001/XMLSchema#string">http://openenergy-platform.org/ontology/oeo/oeo-social</oeo:OEO_00040001>
        <obo:IAO_0000115>An economy is a system of production, distribution, trade and consumption of goods and services.</obo:IAO_0000115>
        <obo:IAO_0000233>issue: https://github.com/OpenEnergyPlatform/ontology/issues/832
pull request: https://github.com/OpenEnergyPlatform/ontology/pull/843</obo:IAO_0000233>
        <rdfs:label xml:lang="en">economy</rdfs:label>
    </owl:Class>
    


    <!-- http://openenergy-platform.org/ontology/oeo/OEO_00010116 -->

    <owl:Class rdf:about="http://openenergy-platform.org/ontology/oeo/OEO_00010116"/>
    


    <!-- http://openenergy-platform.org/ontology/oeo/OEO_00010117 -->

    <owl:Class rdf:about="http://openenergy-platform.org/ontology/oeo/OEO_00010117"/>
    


    <!-- http://openenergy-platform.org/ontology/oeo/OEO_00010123 -->

    <owl:Class rdf:about="http://openenergy-platform.org/ontology/oeo/OEO_00010123">
        <rdfs:subClassOf rdf:resource="http://openenergy-platform.org/ontology/oeo/OEO_00140151"/>
        <rdfs:subClassOf>
            <owl:Restriction>
                <owl:onProperty rdf:resource="http://openenergy-platform.org/ontology/oeo/OEO_00000503"/>
                <owl:someValuesFrom rdf:resource="http://openenergy-platform.org/ontology/oeo/OEO_00020063"/>
            </owl:Restriction>
        </rdfs:subClassOf>
        <oeo:OEO_00040001 rdf:datatype="http://www.w3.org/2001/XMLSchema#string">http://openenergy-platform.org/ontology/oeo/oeo-social</oeo:OEO_00040001>
        <obo:IAO_0000115>Effort sharing is a policy instrument that sets a common emission reduction goal for a number of countries. Each country has a national reduction goal. Under- or overachievement of that goal can be compensated by trading emission certificates.</obo:IAO_0000115>
        <obo:IAO_0000233>issue: https://github.com/OpenEnergyPlatform/ontology/issues/834
pull request: https://github.com/OpenEnergyPlatform/ontology/pull/857</obo:IAO_0000233>
        <rdfs:label xml:lang="en">effort sharing</rdfs:label>
    </owl:Class>
    


    <!-- http://openenergy-platform.org/ontology/oeo/OEO_00010126 -->

    <owl:Class rdf:about="http://openenergy-platform.org/ontology/oeo/OEO_00010126">
        <rdfs:subClassOf rdf:resource="http://openenergy-platform.org/ontology/oeo/OEO_00020063"/>
        <oeo:OEO_00040001 rdf:datatype="http://www.w3.org/2001/XMLSchema#string">http://openenergy-platform.org/ontology/oeo/oeo-social</oeo:OEO_00040001>
        <obo:IAO_0000115>An Annual Emission Allocation (AEA) is an emission certificate used in the Effort Sharing Decision (ESD) and the Effort Sharing Regulation (ESR). It permits the emission of a CO2 equivalent quantity of 1 tonne.</obo:IAO_0000115>
        <obo:IAO_0000118>AEA</obo:IAO_0000118>
        <obo:IAO_0000233>issue: https://github.com/OpenEnergyPlatform/ontology/issues/834
pull request: https://github.com/OpenEnergyPlatform/ontology/pull/857</obo:IAO_0000233>
        <rdfs:label xml:lang="en">Annual Emission Allocation</rdfs:label>
    </owl:Class>
    


    <!-- http://openenergy-platform.org/ontology/oeo/OEO_00010136 -->

    <owl:Class rdf:about="http://openenergy-platform.org/ontology/oeo/OEO_00010136">
        <rdfs:subClassOf rdf:resource="http://purl.obolibrary.org/obo/BFO_0000015"/>
        <oeo:OEO_00040001 rdf:datatype="http://www.w3.org/2001/XMLSchema#string">http://openenergy-platform.org/ontology/oeo/oeo-social</oeo:OEO_00040001>
        <obo:IAO_0000115>Distribution is the process of delivering goods and services to agents</obo:IAO_0000115>
        <obo:IAO_0000233>issue: https://github.com/OpenEnergyPlatform/ontology/issues/836
pull request: https://github.com/OpenEnergyPlatform/ontology/pull/876</obo:IAO_0000233>
        <rdfs:label xml:lang="en">distribution</rdfs:label>
    </owl:Class>
    


    <!-- http://openenergy-platform.org/ontology/oeo/OEO_00010212 -->

    <owl:Class rdf:about="http://openenergy-platform.org/ontology/oeo/OEO_00010212">
        <rdfs:subClassOf rdf:resource="http://openenergy-platform.org/ontology/oeo/OEO_00140150"/>
        <oeo:OEO_00040001 rdf:datatype="http://www.w3.org/2001/XMLSchema#string">http://openenergy-platform.org/ontology/oeo/oeo-social</oeo:OEO_00040001>
        <obo:IAO_0000115>A decarbonisation pathway is a policy that aims at long-term emissions reductions.</obo:IAO_0000115>
        <obo:IAO_0000233>issue: https://github.com/OpenEnergyPlatform/ontology/issues/831
pull request: https://github.com/OpenEnergyPlatform/ontology/pull/951</obo:IAO_0000233>
        <rdfs:label xml:lang="en">decarbonisation pathway</rdfs:label>
    </owl:Class>
    


    <!-- http://openenergy-platform.org/ontology/oeo/OEO_00010227 -->

    <owl:Class rdf:about="http://openenergy-platform.org/ontology/oeo/OEO_00010227">
        <rdfs:subClassOf rdf:resource="http://purl.obolibrary.org/obo/IAO_0000030"/>
        <rdfs:subClassOf>
            <owl:Restriction>
                <owl:onProperty rdf:resource="http://purl.obolibrary.org/obo/IAO_0000136"/>
                <owl:someValuesFrom rdf:resource="http://openenergy-platform.org/ontology/oeo/OEO_00000367"/>
            </owl:Restriction>
        </rdfs:subClassOf>
        <oeo:OEO_00040001 rdf:datatype="http://www.w3.org/2001/XMLSchema#string">http://openenergy-platform.org/ontology/oeo/oeo-social</oeo:OEO_00040001>
        <obo:IAO_0000115>A memo item is an information content entity about a sector that describes that the sector is excluded from some kind of total and only reported to provide further information (memo).</obo:IAO_0000115>
        <obo:IAO_0000233>issue: https://github.com/OpenEnergyPlatform/ontology/issues/858
pull request: https://github.com/OpenEnergyPlatform/ontology/pull/965</obo:IAO_0000233>
        <rdfs:label xml:lang="en">memo item</rdfs:label>
    </owl:Class>
    


    <!-- http://openenergy-platform.org/ontology/oeo/OEO_00010315 -->

    <owl:Class rdf:about="http://openenergy-platform.org/ontology/oeo/OEO_00010315"/>
    


    <!-- http://openenergy-platform.org/ontology/oeo/OEO_00010319 -->

    <owl:Class rdf:about="http://openenergy-platform.org/ontology/oeo/OEO_00010319">
        <rdfs:subClassOf rdf:resource="http://openenergy-platform.org/ontology/oeo/OEO_00000158"/>
        <rdfs:subClassOf>
            <owl:Restriction>
                <owl:onProperty rdf:resource="http://openenergy-platform.org/ontology/oeo/OEO_00010312"/>
                <owl:someValuesFrom rdf:resource="http://openenergy-platform.org/ontology/oeo/OEO_00010315"/>
            </owl:Restriction>
        </rdfs:subClassOf>
        <obo:IAO_0000115>A mineral oil refining sector is an energy transformation sector that covers mineral oil refining.</obo:IAO_0000115>
        <obo:IAO_0000233>issue: https://github.com/OpenEnergyPlatform/ontology/issues/1318
pull request: https://github.com/OpenEnergyPlatform/ontology/pull/1331</obo:IAO_0000233>
        <rdfs:label>mineral oil refining sector</rdfs:label>
    </owl:Class>
    


    <!-- http://openenergy-platform.org/ontology/oeo/OEO_00010320 -->

    <owl:Class rdf:about="http://openenergy-platform.org/ontology/oeo/OEO_00010320">
        <rdfs:subClassOf rdf:resource="http://openenergy-platform.org/ontology/oeo/OEO_00000422"/>
        <rdfs:subClassOf>
            <owl:Restriction>
                <owl:onProperty rdf:resource="http://openenergy-platform.org/ontology/oeo/OEO_00010312"/>
                <owl:someValuesFrom rdf:resource="http://openenergy-platform.org/ontology/oeo/OEO_00140004"/>
            </owl:Restriction>
        </rdfs:subClassOf>
        <obo:IAO_0000115>An international transport sector is a transport sector of international transport processes.</obo:IAO_0000115>
        <obo:IAO_0000233>issue: https://github.com/OpenEnergyPlatform/ontology/issues/969
pull request: https://github.com/OpenEnergyPlatform/ontology/pull/1334</obo:IAO_0000233>
        <rdfs:label xml:lang="en">international transport sector</rdfs:label>
    </owl:Class>
    


    <!-- http://openenergy-platform.org/ontology/oeo/OEO_00020015 -->

    <owl:Class rdf:about="http://openenergy-platform.org/ontology/oeo/OEO_00020015"/>
    


    <!-- http://openenergy-platform.org/ontology/oeo/OEO_00020060 -->

    <owl:Class rdf:about="http://openenergy-platform.org/ontology/oeo/OEO_00020060">
        <rdfs:subClassOf rdf:resource="http://openenergy-platform.org/ontology/oeo/OEO_00020065"/>
        <rdfs:subClassOf>
            <owl:Restriction>
                <owl:onProperty rdf:resource="http://openenergy-platform.org/ontology/oeo/OEO_00020071"/>
                <owl:someValuesFrom>
                    <owl:Restriction>
                        <owl:onProperty rdf:resource="http://purl.obolibrary.org/obo/RO_0000087"/>
                        <owl:someValuesFrom rdf:resource="http://openenergy-platform.org/ontology/oeo/OEO_00020066"/>
                    </owl:Restriction>
                </owl:someValuesFrom>
            </owl:Restriction>
        </rdfs:subClassOf>
        <oeo:OEO_00040001 rdf:datatype="http://www.w3.org/2001/XMLSchema#string">http://openenergy-platform.org/ontology/oeo/oeo-social</oeo:OEO_00040001>
        <obo:IAO_0000115>A fuel market exchange is an energy market exchange where fuels like oil, coal, renewable fuels, and natural gas are traded.</obo:IAO_0000115>
        <obo:IAO_0000233>issue https://github.com/OpenEnergyPlatform/ontology/issues/677
pull request https://github.com/OpenEnergyPlatform/ontology/pull/740
pull request https://github.com/OpenEnergyPlatform/ontology/pull/748</obo:IAO_0000233>
        <rdfs:label>fuel market exchange</rdfs:label>
    </owl:Class>
    


    <!-- http://openenergy-platform.org/ontology/oeo/OEO_00020063 -->

    <owl:Class rdf:about="http://openenergy-platform.org/ontology/oeo/OEO_00020063"/>
    


    <!-- http://openenergy-platform.org/ontology/oeo/OEO_00020064 -->

    <owl:Class rdf:about="http://openenergy-platform.org/ontology/oeo/OEO_00020064">
        <rdfs:subClassOf rdf:resource="http://openenergy-platform.org/ontology/oeo/OEO_00020063"/>
        <oeo:OEO_00040001 rdf:datatype="http://www.w3.org/2001/XMLSchema#string">http://openenergy-platform.org/ontology/oeo/oeo-social</oeo:OEO_00040001>
        <obo:IAO_0000115>An EU Allowance (EUA) is an emission certificate used in the European Union Emissions Trading System (EU ETS). It permits the emission of a CO2 equivalent quantity of 1 tonne.</obo:IAO_0000115>
        <obo:IAO_0000118>EUA</obo:IAO_0000118>
        <obo:IAO_0000233>issue https://github.com/OpenEnergyPlatform/ontology/issues/677
pull request https://github.com/OpenEnergyPlatform/ontology/pull/740</obo:IAO_0000233>
        <rdfs:label>EU allowance</rdfs:label>
    </owl:Class>
    


    <!-- http://openenergy-platform.org/ontology/oeo/OEO_00020065 -->

    <owl:Class rdf:about="http://openenergy-platform.org/ontology/oeo/OEO_00020065">
        <rdfs:subClassOf rdf:resource="http://openenergy-platform.org/ontology/oeo/OEO_00020069"/>
        <oeo:OEO_00040001 rdf:datatype="http://www.w3.org/2001/XMLSchema#string">http://openenergy-platform.org/ontology/oeo/oeo-social</oeo:OEO_00040001>
        <obo:IAO_0000115>An energy market exchange is a market exchange in which energy commodities are traded.</obo:IAO_0000115>
        <obo:IAO_0000233>issue https://github.com/OpenEnergyPlatform/ontology/issues/256
pull request https://github.com/OpenEnergyPlatform/ontology/pull/748</obo:IAO_0000233>
        <rdfs:label>energy market exchange</rdfs:label>
    </owl:Class>
    


    <!-- http://openenergy-platform.org/ontology/oeo/OEO_00020066 -->

    <owl:Class rdf:about="http://openenergy-platform.org/ontology/oeo/OEO_00020066"/>
    


    <!-- http://openenergy-platform.org/ontology/oeo/OEO_00020067 -->

    <owl:Class rdf:about="http://openenergy-platform.org/ontology/oeo/OEO_00020067">
        <rdfs:subClassOf>
            <owl:Restriction>
                <owl:onProperty rdf:resource="http://openenergy-platform.org/ontology/oeo/OEO_00020070"/>
                <owl:someValuesFrom rdf:resource="http://openenergy-platform.org/ontology/oeo/OEO_00020069"/>
            </owl:Restriction>
        </rdfs:subClassOf>
        <obo:IAO_0000118>product</obo:IAO_0000118>
    </owl:Class>
    


    <!-- http://openenergy-platform.org/ontology/oeo/OEO_00020068 -->

    <owl:Class rdf:about="http://openenergy-platform.org/ontology/oeo/OEO_00020068">
        <rdfs:subClassOf>
            <owl:Restriction>
                <owl:onProperty rdf:resource="http://openenergy-platform.org/ontology/oeo/OEO_00020070"/>
                <owl:someValuesFrom rdf:resource="http://openenergy-platform.org/ontology/oeo/OEO_00020060"/>
            </owl:Restriction>
        </rdfs:subClassOf>
    </owl:Class>
    


    <!-- http://openenergy-platform.org/ontology/oeo/OEO_00020069 -->

    <owl:Class rdf:about="http://openenergy-platform.org/ontology/oeo/OEO_00020069">
        <owl:equivalentClass>
            <owl:Restriction>
                <owl:onProperty rdf:resource="http://purl.obolibrary.org/obo/RO_0000087"/>
                <owl:someValuesFrom rdf:resource="http://openenergy-platform.org/ontology/oeo/OEO_00040002"/>
            </owl:Restriction>
        </owl:equivalentClass>
        <rdfs:subClassOf rdf:resource="http://openenergy-platform.org/ontology/oeo/OEO_00030022"/>
        <rdfs:subClassOf>
            <owl:Restriction>
                <owl:onProperty rdf:resource="http://purl.obolibrary.org/obo/RO_0000056"/>
                <owl:someValuesFrom>
                    <owl:Class>
                        <owl:intersectionOf rdf:parseType="Collection">
                            <rdf:Description rdf:about="http://openenergy-platform.org/ontology/oeo/OEO_00010082"/>
                            <owl:Restriction>
                                <owl:onProperty rdf:resource="http://purl.obolibrary.org/obo/RO_0000057"/>
                                <owl:someValuesFrom rdf:resource="http://openenergy-platform.org/ontology/oeo/OEO_00010083"/>
                            </owl:Restriction>
                        </owl:intersectionOf>
                    </owl:Class>
                </owl:someValuesFrom>
            </owl:Restriction>
        </rdfs:subClassOf>
        <oeo:OEO_00040001 rdf:datatype="http://www.w3.org/2001/XMLSchema#string">http://openenergy-platform.org/ontology/oeo/oeo-social</oeo:OEO_00040001>
        <obo:IAO_0000115>A market exchange is an organisation that has the market exchange role.</obo:IAO_0000115>
        <obo:IAO_0000233>pull request: https://github.com/OpenEnergyPlatform/ontology/pull/748</obo:IAO_0000233>
        <rdfs:label>market exchange</rdfs:label>
    </owl:Class>
    <owl:Axiom>
        <owl:annotatedSource rdf:resource="http://openenergy-platform.org/ontology/oeo/OEO_00020069"/>
        <owl:annotatedProperty rdf:resource="http://www.w3.org/2000/01/rdf-schema#subClassOf"/>
        <owl:annotatedTarget>
            <owl:Restriction>
                <owl:onProperty rdf:resource="http://purl.obolibrary.org/obo/RO_0000056"/>
                <owl:someValuesFrom>
                    <owl:Class>
                        <owl:intersectionOf rdf:parseType="Collection">
                            <rdf:Description rdf:about="http://openenergy-platform.org/ontology/oeo/OEO_00010082"/>
                            <owl:Restriction>
                                <owl:onProperty rdf:resource="http://purl.obolibrary.org/obo/RO_0000057"/>
                                <owl:someValuesFrom rdf:resource="http://openenergy-platform.org/ontology/oeo/OEO_00010083"/>
                            </owl:Restriction>
                        </owl:intersectionOf>
                    </owl:Class>
                </owl:someValuesFrom>
            </owl:Restriction>
        </owl:annotatedTarget>
        <obo:IAO_0000233>https://github.com/OpenEnergyPlatform/ontology/issues/617
https://github.com/OpenEnergyPlatform/ontology/pull/1019</obo:IAO_0000233>
    </owl:Axiom>
    


    <!-- http://openenergy-platform.org/ontology/oeo/OEO_00020075 -->

    <owl:Class rdf:about="http://openenergy-platform.org/ontology/oeo/OEO_00020075">
        <rdfs:subClassOf rdf:resource="http://openenergy-platform.org/ontology/oeo/OEO_00020069"/>
        <rdfs:subClassOf>
            <owl:Restriction>
                <owl:onProperty rdf:resource="http://openenergy-platform.org/ontology/oeo/OEO_00020071"/>
                <owl:someValuesFrom rdf:resource="http://openenergy-platform.org/ontology/oeo/OEO_00020063"/>
            </owl:Restriction>
        </rdfs:subClassOf>
        <oeo:OEO_00040001 rdf:datatype="http://www.w3.org/2001/XMLSchema#string">http://openenergy-platform.org/ontology/oeo/oeo-social</oeo:OEO_00040001>
        <obo:IAO_0000115>An emission market exchange is a market exchange where emission certificates are traded</obo:IAO_0000115>
        <obo:IAO_0000233>issue https://github.com/OpenEnergyPlatform/ontology/issues/302
pull request https://github.com/OpenEnergyPlatform/ontology/pull/781</obo:IAO_0000233>
        <rdfs:label>emission market exchange</rdfs:label>
    </owl:Class>
    


    <!-- http://openenergy-platform.org/ontology/oeo/OEO_00020076 -->

    <owl:Class rdf:about="http://openenergy-platform.org/ontology/oeo/OEO_00020076">
        <rdfs:subClassOf rdf:resource="http://openenergy-platform.org/ontology/oeo/OEO_00140012"/>
        <rdfs:subClassOf>
            <owl:Restriction>
                <owl:onProperty rdf:resource="http://openenergy-platform.org/ontology/oeo/OEO_00040010"/>
                <owl:someValuesFrom rdf:resource="http://openenergy-platform.org/ontology/oeo/OEO_00040004"/>
            </owl:Restriction>
        </rdfs:subClassOf>
        <oeo:OEO_00040001 rdf:datatype="http://www.w3.org/2001/XMLSchema#string">http://openenergy-platform.org/ontology/oeo/oeo-social</oeo:OEO_00040001>
        <obo:IAO_0000115>A markup is an economic value that indicates a virtual amount added to an assumed or historical price to predict a price in a different context.</obo:IAO_0000115>
        <obo:IAO_0000233>https://github.com/OpenEnergyPlatform/ontology/issues/256
https://github.com/OpenEnergyPlatform/ontology/pull/800</obo:IAO_0000233>
        <rdfs:label>markup</rdfs:label>
    </owl:Class>
    


    <!-- http://openenergy-platform.org/ontology/oeo/OEO_00020077 -->

    <owl:Class rdf:about="http://openenergy-platform.org/ontology/oeo/OEO_00020077">
        <rdfs:subClassOf rdf:resource="http://openenergy-platform.org/ontology/oeo/OEO_00140012"/>
        <rdfs:subClassOf>
            <owl:Restriction>
                <owl:onProperty rdf:resource="http://openenergy-platform.org/ontology/oeo/OEO_00040010"/>
                <owl:someValuesFrom rdf:resource="http://openenergy-platform.org/ontology/oeo/OEO_00040004"/>
            </owl:Restriction>
        </rdfs:subClassOf>
        <oeo:OEO_00040001 rdf:datatype="http://www.w3.org/2001/XMLSchema#string">http://openenergy-platform.org/ontology/oeo/oeo-social</oeo:OEO_00040001>
        <obo:IAO_0000115>A markdown is an economic value that indicates a virtual amount deducted from an assumed or historical price to predict a price in a different context.</obo:IAO_0000115>
        <obo:IAO_0000233>https://github.com/OpenEnergyPlatform/ontology/issues/256
https://github.com/OpenEnergyPlatform/ontology/pull/800</obo:IAO_0000233>
        <rdfs:label>markdown</rdfs:label>
    </owl:Class>
    


    <!-- http://openenergy-platform.org/ontology/oeo/OEO_00020108 -->

    <owl:Class rdf:about="http://openenergy-platform.org/ontology/oeo/OEO_00020108">
        <rdfs:subClassOf rdf:resource="http://openenergy-platform.org/ontology/oeo/OEO_00140151"/>
        <oeo:OEO_00040001 rdf:datatype="http://www.w3.org/2001/XMLSchema#string">http://openenergy-platform.org/ontology/oeo/oeo-social</oeo:OEO_00040001>
        <obo:IAO_0000115>A feed-in tariff is a policy instrument designed to stimulate investment in renewable energy technologies by offering long-term contracts to agents who are producers of renewable energy.</obo:IAO_0000115>
        <obo:IAO_0000233>issue: https://github.com/OpenEnergyPlatform/ontology/issues/839
issue: https://github.com/OpenEnergyPlatform/ontology/issues/898
pull request: https://github.com/OpenEnergyPlatform/ontology/pull/909</obo:IAO_0000233>
        <rdfs:comment>Feed-in tariffs provide cost-based compensation to renewable energy producers, leading to price certainty and long-term contracts that help finance energy transformation units, e.g. power plants</rdfs:comment>
        <rdfs:label>feed-in tariff</rdfs:label>
    </owl:Class>
    


    <!-- http://openenergy-platform.org/ontology/oeo/OEO_00020109 -->

    <owl:Class rdf:about="http://openenergy-platform.org/ontology/oeo/OEO_00020109">
        <rdfs:subClassOf rdf:resource="http://openenergy-platform.org/ontology/oeo/OEO_00140151"/>
        <oeo:OEO_00040001 rdf:datatype="http://www.w3.org/2001/XMLSchema#string">http://openenergy-platform.org/ontology/oeo/oeo-social</oeo:OEO_00040001>
        <obo:IAO_0000115>A market premium is a policy instrument that ensures a guaranteed remuneration, e.g. a fixed feed-in tariff, by paying to the producing agent the difference between a guaranteed return on a good/product and the monetary price for which the good/product is traded on the market</obo:IAO_0000115>
        <obo:IAO_0000233>issue: https://github.com/OpenEnergyPlatform/ontology/issues/839
issue: https://github.com/OpenEnergyPlatform/ontology/issues/899
pull request: https://github.com/OpenEnergyPlatform/ontology/pull/909</obo:IAO_0000233>
        <rdfs:label>market premium</rdfs:label>
    </owl:Class>
    


    <!-- http://openenergy-platform.org/ontology/oeo/OEO_00020110 -->

    <owl:Class rdf:about="http://openenergy-platform.org/ontology/oeo/OEO_00020110">
        <rdfs:subClassOf rdf:resource="http://openenergy-platform.org/ontology/oeo/OEO_00140151"/>
        <oeo:OEO_00040001 rdf:datatype="http://www.w3.org/2001/XMLSchema#string">http://openenergy-platform.org/ontology/oeo/oeo-social</oeo:OEO_00040001>
        <obo:IAO_0000115>A levy is a policy instrument that consists of a compulsory financial charge imposed on an agent or institution by a governmental organisation.</obo:IAO_0000115>
        <obo:IAO_0000233>issue: https://github.com/OpenEnergyPlatform/ontology/issues/839
issue: https://github.com/OpenEnergyPlatform/ontology/issues/900
pull request: https://github.com/OpenEnergyPlatform/ontology/pull/909</obo:IAO_0000233>
        <rdfs:label>levy</rdfs:label>
    </owl:Class>
    


    <!-- http://openenergy-platform.org/ontology/oeo/OEO_00020111 -->

    <owl:Class rdf:about="http://openenergy-platform.org/ontology/oeo/OEO_00020111">
        <rdfs:subClassOf rdf:resource="http://openenergy-platform.org/ontology/oeo/OEO_00020109"/>
        <oeo:OEO_00040001 rdf:datatype="http://www.w3.org/2001/XMLSchema#string">http://openenergy-platform.org/ontology/oeo/oeo-social</oeo:OEO_00040001>
        <obo:IAO_0000115>A capacity premium is a market premium that guarantees remuneration for reserving capacity of energy transformation units to be available for unexpected events.</obo:IAO_0000115>
        <obo:IAO_0000233>issue: https://github.com/OpenEnergyPlatform/ontology/issues/839
issue: https://github.com/OpenEnergyPlatform/ontology/issues/903
pull request: https://github.com/OpenEnergyPlatform/ontology/pull/909</obo:IAO_0000233>
        <rdfs:label>capacity premium</rdfs:label>
    </owl:Class>
    


    <!-- http://openenergy-platform.org/ontology/oeo/OEO_00020112 -->

    <owl:Class rdf:about="http://openenergy-platform.org/ontology/oeo/OEO_00020112">
        <rdfs:subClassOf rdf:resource="http://openenergy-platform.org/ontology/oeo/OEO_00020110"/>
        <oeo:OEO_00040001 rdf:datatype="http://www.w3.org/2001/XMLSchema#string">http://openenergy-platform.org/ontology/oeo/oeo-social</oeo:OEO_00040001>
        <obo:IAO_0000115>A tax is a levy whose returns are used by the government to finance expenditures for the common welfare.</obo:IAO_0000115>
        <obo:IAO_0000233>issue: https://github.com/OpenEnergyPlatform/ontology/issues/839
issue: https://github.com/OpenEnergyPlatform/ontology/issues/901
pull request: https://github.com/OpenEnergyPlatform/ontology/pull/909</obo:IAO_0000233>
        <rdfs:label>tax</rdfs:label>
    </owl:Class>
    


    <!-- http://openenergy-platform.org/ontology/oeo/OEO_00020113 -->

    <owl:Class rdf:about="http://openenergy-platform.org/ontology/oeo/OEO_00020113">
        <rdfs:subClassOf rdf:resource="http://openenergy-platform.org/ontology/oeo/OEO_00140012"/>
        <rdfs:subClassOf>
            <owl:Restriction>
                <owl:onProperty rdf:resource="http://openenergy-platform.org/ontology/oeo/OEO_00040010"/>
                <owl:someValuesFrom rdf:resource="http://purl.obolibrary.org/obo/UO_0010006"/>
            </owl:Restriction>
        </rdfs:subClassOf>
        <oeo:OEO_00040001 rdf:datatype="http://www.w3.org/2001/XMLSchema#string">http://openenergy-platform.org/ontology/oeo/oeo-social</oeo:OEO_00040001>
        <obo:IAO_0000115>Inflation rate is an economic value reprensenting the ratio between the monetary price for a good at two different points in time that equalises differences in monetary price levels between these two points in time.</obo:IAO_0000115>
        <obo:IAO_0000233>https://github.com/OpenEnergyPlatform/ontology/issues/335
https://github.com/OpenEnergyPlatform/ontology/pull/910</obo:IAO_0000233>
        <rdfs:label>inflation rate</rdfs:label>
    </owl:Class>
    


    <!-- http://openenergy-platform.org/ontology/oeo/OEO_00020114 -->

    <owl:Class rdf:about="http://openenergy-platform.org/ontology/oeo/OEO_00020114">
        <rdfs:subClassOf rdf:resource="http://openenergy-platform.org/ontology/oeo/OEO_00140012"/>
        <rdfs:subClassOf>
            <owl:Restriction>
                <owl:onProperty rdf:resource="http://openenergy-platform.org/ontology/oeo/OEO_00040010"/>
                <owl:someValuesFrom rdf:resource="http://purl.obolibrary.org/obo/UO_0010006"/>
            </owl:Restriction>
        </rdfs:subClassOf>
        <oeo:OEO_00040001 rdf:datatype="http://www.w3.org/2001/XMLSchema#string">http://openenergy-platform.org/ontology/oeo/oeo-social</oeo:OEO_00040001>
        <obo:IAO_0000112>The exchange rate between USD and EUR on March 15, 2020 was X.X.</obo:IAO_0000112>
        <obo:IAO_0000115>The exchange rate is an economic value representing the ratio at which one currency can be exchanged for another.</obo:IAO_0000115>
        <obo:IAO_0000118>market exchange rate</obo:IAO_0000118>
        <obo:IAO_0000233>https://github.com/OpenEnergyPlatform/ontology/issues/335
https://github.com/OpenEnergyPlatform/ontology/pull/910</obo:IAO_0000233>
        <rdfs:comment>The ratio at which one can exchange one currency for another can differ over time therefore it is necessary to specify a time point when referring to an exchange rate.</rdfs:comment>
        <rdfs:label>exchange rate</rdfs:label>
    </owl:Class>
    


    <!-- http://openenergy-platform.org/ontology/oeo/OEO_00020115 -->

    <owl:Class rdf:about="http://openenergy-platform.org/ontology/oeo/OEO_00020115">
        <rdfs:subClassOf rdf:resource="http://openenergy-platform.org/ontology/oeo/OEO_00140012"/>
        <rdfs:subClassOf>
            <owl:Restriction>
                <owl:onProperty rdf:resource="http://openenergy-platform.org/ontology/oeo/OEO_00040010"/>
                <owl:someValuesFrom rdf:resource="http://purl.obolibrary.org/obo/UO_0010006"/>
            </owl:Restriction>
        </rdfs:subClassOf>
        <oeo:OEO_00040001 rdf:datatype="http://www.w3.org/2001/XMLSchema#string">http://openenergy-platform.org/ontology/oeo/oeo-social</oeo:OEO_00040001>
        <obo:IAO_0000115>Purchasing power parity is an economic value reprensenting the ratio between currencies that equalises differences in monetary price levels between countries for the same set of goods.</obo:IAO_0000115>
        <obo:IAO_0000118>PPP</obo:IAO_0000118>
        <obo:IAO_0000233>https://github.com/OpenEnergyPlatform/ontology/issues/867
https://github.com/OpenEnergyPlatform/ontology/pull/910</obo:IAO_0000233>
        <terms:source>https://www.oecd.org/sdd/prices-ppp/purchasingpowerparities-frequentlyaskedquestionsfaqs.htm#FAQ1</terms:source>
        <rdfs:label>purchasing power parity</rdfs:label>
    </owl:Class>
    


    <!-- http://openenergy-platform.org/ontology/oeo/OEO_00020116 -->

    <owl:Class rdf:about="http://openenergy-platform.org/ontology/oeo/OEO_00020116">
        <rdfs:subClassOf rdf:resource="http://openenergy-platform.org/ontology/oeo/OEO_00040009"/>
        <oeo:OEO_00040001 rdf:datatype="http://www.w3.org/2001/XMLSchema#string">http://openenergy-platform.org/ontology/oeo/oeo-social</oeo:OEO_00040001>
        <obo:IAO_0000115>System cost are total costs of a system.</obo:IAO_0000115>
        <obo:IAO_0000233>issue: https://github.com/OpenEnergyPlatform/ontology/issues/335
pull request: https://github.com/OpenEnergyPlatform/ontology/pull/910</obo:IAO_0000233>
        <rdfs:label>system cost</rdfs:label>
    </owl:Class>
    


    <!-- http://openenergy-platform.org/ontology/oeo/OEO_00020117 -->

    <owl:Class rdf:about="http://openenergy-platform.org/ontology/oeo/OEO_00020117">
        <rdfs:subClassOf rdf:resource="http://openenergy-platform.org/ontology/oeo/OEO_00040003"/>
        <oeo:OEO_00040001 rdf:datatype="http://www.w3.org/2001/XMLSchema#string">http://openenergy-platform.org/ontology/oeo/oeo-social</oeo:OEO_00040001>
        <obo:IAO_0000112>The electricity price is Y EUR per megawatt-hour.</obo:IAO_0000112>
        <obo:IAO_0000115>Electricity price is the monetary price per energy unit of electricity.</obo:IAO_0000115>
        <obo:IAO_0000233>issue: https://github.com/OpenEnergyPlatform/ontology/issues/335
pull request: https://github.com/OpenEnergyPlatform/ontology/pull/910</obo:IAO_0000233>
        <rdfs:comment>has unit some &quot;currency per energy unit&quot;</rdfs:comment>
        <rdfs:label>electricity price</rdfs:label>
    </owl:Class>
    


    <!-- http://openenergy-platform.org/ontology/oeo/OEO_00020124 -->

    <owl:Class rdf:about="http://openenergy-platform.org/ontology/oeo/OEO_00020124">
        <rdfs:subClassOf rdf:resource="http://openenergy-platform.org/ontology/oeo/OEO_00140012"/>
        <rdfs:subClassOf>
            <owl:Restriction>
                <owl:onProperty rdf:resource="http://openenergy-platform.org/ontology/oeo/OEO_00040010"/>
                <owl:someValuesFrom rdf:resource="http://openenergy-platform.org/ontology/oeo/OEO_00040004"/>
            </owl:Restriction>
        </rdfs:subClassOf>
        <oeo:OEO_00040001 rdf:datatype="http://www.w3.org/2001/XMLSchema#string">http://openenergy-platform.org/ontology/oeo/oeo-social</oeo:OEO_00040001>
        <obo:IAO_0000115>A due is an economic value that represents a payment that an agent makes to belong to an organisation.</obo:IAO_0000115>
        <obo:IAO_0000233>issue: https://github.com/OpenEnergyPlatform/ontology/issues/904
pull request: https://github.com/OpenEnergyPlatform/ontology/pull/913</obo:IAO_0000233>
        <rdfs:label>due</rdfs:label>
    </owl:Class>
    


    <!-- http://openenergy-platform.org/ontology/oeo/OEO_00020125 -->

    <owl:Class rdf:about="http://openenergy-platform.org/ontology/oeo/OEO_00020125">
        <rdfs:subClassOf rdf:resource="http://openenergy-platform.org/ontology/oeo/OEO_00140012"/>
        <rdfs:subClassOf>
            <owl:Restriction>
                <owl:onProperty rdf:resource="http://openenergy-platform.org/ontology/oeo/OEO_00040010"/>
                <owl:someValuesFrom rdf:resource="http://openenergy-platform.org/ontology/oeo/OEO_00040004"/>
            </owl:Restriction>
        </rdfs:subClassOf>
        <oeo:OEO_00040001 rdf:datatype="http://www.w3.org/2001/XMLSchema#string">http://openenergy-platform.org/ontology/oeo/oeo-social</oeo:OEO_00040001>
        <obo:IAO_0000115>A remuneration is an economic value that describes a financial compensation provided in exchange for services performed.</obo:IAO_0000115>
        <obo:IAO_0000233>issue: https://github.com/OpenEnergyPlatform/ontology/issues/902
pull request: https://github.com/OpenEnergyPlatform/ontology/pull/913</obo:IAO_0000233>
        <rdfs:label>remuneration</rdfs:label>
    </owl:Class>
    


    <!-- http://openenergy-platform.org/ontology/oeo/OEO_00020126 -->

    <owl:Class rdf:about="http://openenergy-platform.org/ontology/oeo/OEO_00020126">
        <rdfs:subClassOf rdf:resource="http://openenergy-platform.org/ontology/oeo/OEO_00140012"/>
        <rdfs:subClassOf>
            <owl:Restriction>
                <owl:onProperty rdf:resource="http://openenergy-platform.org/ontology/oeo/OEO_00040010"/>
                <owl:someValuesFrom rdf:resource="http://openenergy-platform.org/ontology/oeo/OEO_00040004"/>
            </owl:Restriction>
        </rdfs:subClassOf>
        <oeo:OEO_00040001 rdf:datatype="http://www.w3.org/2001/XMLSchema#string">http://openenergy-platform.org/ontology/oeo/oeo-social</oeo:OEO_00040001>
        <obo:IAO_0000115>A fee is an economic value that represents an amount of money paid for a  particular piece of work or for a particular right or service.</obo:IAO_0000115>
        <obo:IAO_0000233>issue: https://github.com/OpenEnergyPlatform/ontology/issues/905
pull request: https://github.com/OpenEnergyPlatform/ontology/pull/913</obo:IAO_0000233>
        <rdfs:label>fee</rdfs:label>
    </owl:Class>
    


    <!-- http://openenergy-platform.org/ontology/oeo/OEO_00020127 -->

    <owl:Class rdf:about="http://openenergy-platform.org/ontology/oeo/OEO_00020127">
        <rdfs:subClassOf rdf:resource="http://openenergy-platform.org/ontology/oeo/OEO_00040009"/>
        <oeo:OEO_00040001 rdf:datatype="http://www.w3.org/2001/XMLSchema#string">http://openenergy-platform.org/ontology/oeo/oeo-social</oeo:OEO_00040001>
        <obo:IAO_0000115>Levelised cost of electricity are the net cost of converting energy to electricity / electric energy over the lifetime of an energy transformation unit. They are calculated considering all relevant costs including investment, operation, maintenance and fuel cost, etc.</obo:IAO_0000115>
        <obo:IAO_0000118>LCOE</obo:IAO_0000118>
        <obo:IAO_0000233>issue: https://github.com/OpenEnergyPlatform/ontology/issues/906
pull request: https://github.com/OpenEnergyPlatform/ontology/pull/913</obo:IAO_0000233>
        <rdfs:comment>Since over the lifetime of an energy transformation unit different costs exhibit different relevance or vary over time, the LCOE differ over the course of the lifetime.</rdfs:comment>
        <rdfs:label>levelised cost of electricity</rdfs:label>
    </owl:Class>
    


    <!-- http://openenergy-platform.org/ontology/oeo/OEO_00020128 -->

    <owl:Class rdf:about="http://openenergy-platform.org/ontology/oeo/OEO_00020128">
        <rdfs:subClassOf rdf:resource="http://openenergy-platform.org/ontology/oeo/OEO_00140012"/>
        <rdfs:subClassOf>
            <owl:Restriction>
                <owl:onProperty rdf:resource="http://openenergy-platform.org/ontology/oeo/OEO_00040010"/>
                <owl:someValuesFrom rdf:resource="http://openenergy-platform.org/ontology/oeo/OEO_00040004"/>
            </owl:Restriction>
        </rdfs:subClassOf>
        <oeo:OEO_00040001 rdf:datatype="http://www.w3.org/2001/XMLSchema#string">http://openenergy-platform.org/ontology/oeo/oeo-social</oeo:OEO_00040001>
        <obo:IAO_0000115>Market revenue is an economic value that represents the income from a trade at a market exchange.</obo:IAO_0000115>
        <obo:IAO_0000233>add term
https://github.com/OpenEnergyPlatform/ontology/issues/908
https://github.com/OpenEnergyPlatform/ontology/pull/929</obo:IAO_0000233>
        <rdfs:label>market revenue</rdfs:label>
    </owl:Class>
    


    <!-- http://openenergy-platform.org/ontology/oeo/OEO_00020145 -->

    <owl:Class rdf:about="http://openenergy-platform.org/ontology/oeo/OEO_00020145">
        <rdfs:subClassOf rdf:resource="http://openenergy-platform.org/ontology/oeo/OEO_00040009"/>
        <oeo:OEO_00040001 rdf:datatype="http://www.w3.org/2001/XMLSchema#string">http://openenergy-platform.org/ontology/oeo/oeo-social</oeo:OEO_00040001>
        <obo:IAO_0000115>A variable cost is a cost that depends on an amount of goods or services.</obo:IAO_0000115>
        <obo:IAO_0000118>unit-level cost</obo:IAO_0000118>
        <obo:IAO_0000233>issue: https://github.com/OpenEnergyPlatform/ontology/issues/891
pull request: https://github.com/OpenEnergyPlatform/ontology/pull/953

Reformulate definition to singular:
issue: https://github.com/OpenEnergyPlatform/ontology/issues/1257
pull request: https://github.com/OpenEnergyPlatform/ontology/pull/1260</obo:IAO_0000233>
        <rdfs:label>variable cost</rdfs:label>
    </owl:Class>
    


    <!-- http://openenergy-platform.org/ontology/oeo/OEO_00020146 -->

    <owl:Class rdf:about="http://openenergy-platform.org/ontology/oeo/OEO_00020146">
        <rdfs:subClassOf rdf:resource="http://openenergy-platform.org/ontology/oeo/OEO_00020145"/>
        <oeo:OEO_00040001 rdf:datatype="http://www.w3.org/2001/XMLSchema#string">http://openenergy-platform.org/ontology/oeo/oeo-social</oeo:OEO_00040001>
        <obo:IAO_0000112>An example for variable cost are costs incurred for raw materials (of which more are needed if production is increased).</obo:IAO_0000112>
        <obo:IAO_0000115>Variable costs are costs that depend on the amount of goods or services produced and which are payed by the producer.</obo:IAO_0000115>
        <obo:IAO_0000233>issue: https://github.com/OpenEnergyPlatform/ontology/issues/891
pull request: https://github.com/OpenEnergyPlatform/ontology/pull/953</obo:IAO_0000233>
        <rdfs:label>variable production cost</rdfs:label>
    </owl:Class>
    


    <!-- http://openenergy-platform.org/ontology/oeo/OEO_00020156 -->

    <owl:Class rdf:about="http://openenergy-platform.org/ontology/oeo/OEO_00020156">
        <rdfs:subClassOf rdf:resource="http://openenergy-platform.org/ontology/oeo/OEO_00020112"/>
        <oeo:OEO_00040001 rdf:datatype="http://www.w3.org/2001/XMLSchema#string">http://openenergy-platform.org/ontology/oeo/oeo-social</oeo:OEO_00040001>
        <obo:IAO_0000115>Carbon tax is a tax for emitting CO2 or other greenhouse gases (measured in CO2 equivalent values).</obo:IAO_0000115>
        <obo:IAO_0000118>CO2 tax</obo:IAO_0000118>
        <obo:IAO_0000233>issue: https://github.com/OpenEnergyPlatform/ontology/issues/866
pull request: https://github.com/OpenEnergyPlatform/ontology/pull/956</obo:IAO_0000233>
        <rdfs:label>carbon tax</rdfs:label>
    </owl:Class>
    


    <!-- http://openenergy-platform.org/ontology/oeo/OEO_00020167 -->

    <owl:Class rdf:about="http://openenergy-platform.org/ontology/oeo/OEO_00020167">
        <rdfs:subClassOf rdf:resource="http://openenergy-platform.org/ontology/oeo/OEO_00040009"/>
        <oeo:OEO_00040001 rdf:datatype="http://www.w3.org/2001/XMLSchema#string">http://openenergy-platform.org/ontology/oeo/oeo-social</oeo:OEO_00040001>
        <obo:IAO_0000115>Investment costs are costs of a long-term commitment of financial resources in tangible or intangible assets.</obo:IAO_0000115>
        <obo:IAO_0000118>capital investment cost</obo:IAO_0000118>
        <obo:IAO_0000118>fixed investment cost</obo:IAO_0000118>
        <obo:IAO_0000118>investment</obo:IAO_0000118>
        <obo:IAO_0000119>FIBO definition of investment relates to property only: https://spec.edmcouncil.org/fibo/ontology?searchBoxQuery=investment,

Gabler on Investition: langfristige Bindung finanzieller Mittel in materiellen oder in immateriellen Vermögensgegenständen (https://wirtschaftslexikon.gabler.de/definition/investition-39454)</obo:IAO_0000119>
        <obo:IAO_0000233>issue: https://github.com/OpenEnergyPlatform/ontology/issues/891
pull request: https://github.com/OpenEnergyPlatform/ontology/pull/1022</obo:IAO_0000233>
        <rdfs:label>investment cost</rdfs:label>
    </owl:Class>
    


    <!-- http://openenergy-platform.org/ontology/oeo/OEO_00020168 -->

    <owl:Class rdf:about="http://openenergy-platform.org/ontology/oeo/OEO_00020168">
        <rdfs:subClassOf rdf:resource="http://openenergy-platform.org/ontology/oeo/OEO_00040009"/>
        <oeo:OEO_00040001 rdf:datatype="http://www.w3.org/2001/XMLSchema#string">http://openenergy-platform.org/ontology/oeo/oeo-social</oeo:OEO_00040001>
        <obo:IAO_0000112>rent, regular technical maintenance cost, staff cost, certification cost</obo:IAO_0000112>
        <obo:IAO_0000115>A fixed cost is a cost for operation and mantainance that does not vary with the amount of goods or services produced.</obo:IAO_0000115>
        <obo:IAO_0000118>fixed operation and maintanance cost</obo:IAO_0000118>
        <obo:IAO_0000119>oemof-Model: https://oemof-solph.readthedocs.io/en/latest/_modules/oemof/solph/options.html?highlight=fix%20costs

Fixe Kosten: Kosten, die von der jeweils betrachteten Einflussgröße bzw. Entscheidung unabhängig sind, d.h. Kosten, die sich nicht mit der jeweils betrachteten Einflussgröße ändern. (https://wirtschaftslexikon.gabler.de/definition/fixe-kosten-33359)</obo:IAO_0000119>
        <obo:IAO_0000233>issue: https://github.com/OpenEnergyPlatform/ontology/issues/891
pull request: https://github.com/OpenEnergyPlatform/ontology/pull/1022

Reformulate definition to singular:
issue: https://github.com/OpenEnergyPlatform/ontology/issues/1257
pull request: https://github.com/OpenEnergyPlatform/ontology/pull/1260</obo:IAO_0000233>
        <rdfs:label>fixed cost</rdfs:label>
    </owl:Class>
    


    <!-- http://openenergy-platform.org/ontology/oeo/OEO_00020169 -->

    <owl:Class rdf:about="http://openenergy-platform.org/ontology/oeo/OEO_00020169">
        <rdfs:subClassOf rdf:resource="http://openenergy-platform.org/ontology/oeo/OEO_00020167"/>
        <oeo:OEO_00040001 rdf:datatype="http://www.w3.org/2001/XMLSchema#string">http://openenergy-platform.org/ontology/oeo/oeo-social</oeo:OEO_00040001>
        <obo:IAO_0000115>Equipment cost is an investment cost for acquisition of the components and machinery including environmental facilities.</obo:IAO_0000115>
        <obo:IAO_0000233>issue: https://github.com/OpenEnergyPlatform/ontology/issues/891
pull request: https://github.com/OpenEnergyPlatform/ontology/pull/1022

Reformulate definition to singular:
issue: https://github.com/OpenEnergyPlatform/ontology/issues/1257
pull request: https://github.com/OpenEnergyPlatform/ontology/pull/1260</obo:IAO_0000233>
        <rdfs:label>equipment cost</rdfs:label>
    </owl:Class>
    


    <!-- http://openenergy-platform.org/ontology/oeo/OEO_00020170 -->

    <owl:Class rdf:about="http://openenergy-platform.org/ontology/oeo/OEO_00020170">
        <rdfs:subClassOf rdf:resource="http://openenergy-platform.org/ontology/oeo/OEO_00020167"/>
        <oeo:OEO_00040001 rdf:datatype="http://www.w3.org/2001/XMLSchema#string">http://openenergy-platform.org/ontology/oeo/oeo-social</oeo:OEO_00040001>
        <obo:IAO_0000112>costs that occur for becoming operational</obo:IAO_0000112>
        <obo:IAO_0000115>Installation and development cost are investment costs incurred for setting up the installation.</obo:IAO_0000115>
        <obo:IAO_0000118>installation and development cost</obo:IAO_0000118>
        <obo:IAO_0000118>site development cost</obo:IAO_0000118>
        <obo:IAO_0000233>issue: https://github.com/OpenEnergyPlatform/ontology/issues/891
pull request: https://github.com/OpenEnergyPlatform/ontology/pull/1022</obo:IAO_0000233>
        <rdfs:label>installation cost</rdfs:label>
    </owl:Class>
    


    <!-- http://openenergy-platform.org/ontology/oeo/OEO_00020171 -->

    <owl:Class rdf:about="http://openenergy-platform.org/ontology/oeo/OEO_00020171">
        <rdfs:subClassOf rdf:resource="http://openenergy-platform.org/ontology/oeo/OEO_00020167"/>
        <oeo:OEO_00040001 rdf:datatype="http://www.w3.org/2001/XMLSchema#string">http://openenergy-platform.org/ontology/oeo/oeo-social</oeo:OEO_00040001>
        <obo:IAO_0000115>Grid connection costs are investment costs for establishing the grid connection from the energy generating device to point of connection to national grid.</obo:IAO_0000115>
        <obo:IAO_0000233>issue: https://github.com/OpenEnergyPlatform/ontology/issues/891
pull request: https://github.com/OpenEnergyPlatform/ontology/pull/1022</obo:IAO_0000233>
        <rdfs:label>grid connection cost</rdfs:label>
    </owl:Class>
    


    <!-- http://openenergy-platform.org/ontology/oeo/OEO_00020172 -->

    <owl:Class rdf:about="http://openenergy-platform.org/ontology/oeo/OEO_00020172">
        <rdfs:subClassOf rdf:resource="http://openenergy-platform.org/ontology/oeo/OEO_00020167"/>
        <oeo:OEO_00040001 rdf:datatype="http://www.w3.org/2001/XMLSchema#string">http://openenergy-platform.org/ontology/oeo/oeo-social</oeo:OEO_00040001>
        <obo:IAO_0000115>A property cost is an investment cost arising from the acquisition of a property.</obo:IAO_0000115>
        <obo:IAO_0000118>land cost</obo:IAO_0000118>
        <obo:IAO_0000233>issue: https://github.com/OpenEnergyPlatform/ontology/issues/891
pull request: https://github.com/OpenEnergyPlatform/ontology/pull/1022

Reformulate definition to singular:
issue: https://github.com/OpenEnergyPlatform/ontology/issues/1257
pull request: https://github.com/OpenEnergyPlatform/ontology/pull/1260</obo:IAO_0000233>
        <rdfs:label>property cost</rdfs:label>
    </owl:Class>
    


    <!-- http://openenergy-platform.org/ontology/oeo/OEO_00020173 -->

    <owl:Class rdf:about="http://openenergy-platform.org/ontology/oeo/OEO_00020173">
        <rdfs:subClassOf rdf:resource="http://openenergy-platform.org/ontology/oeo/OEO_00020167"/>
        <oeo:OEO_00040001 rdf:datatype="http://www.w3.org/2001/XMLSchema#string">http://openenergy-platform.org/ontology/oeo/oeo-social</oeo:OEO_00040001>
        <obo:IAO_0000115>Decommissioning costs are investment costs arising from the decommissioning of a technological device at the end of its lifetime.</obo:IAO_0000115>
        <obo:IAO_0000233>issue: https://github.com/OpenEnergyPlatform/ontology/issues/891
pull request: https://github.com/OpenEnergyPlatform/ontology/pull/1022</obo:IAO_0000233>
        <rdfs:label>decommissioning cost</rdfs:label>
    </owl:Class>
    


    <!-- http://openenergy-platform.org/ontology/oeo/OEO_00020174 -->

    <owl:Class rdf:about="http://openenergy-platform.org/ontology/oeo/OEO_00020174">
        <rdfs:subClassOf rdf:resource="http://openenergy-platform.org/ontology/oeo/OEO_00040009"/>
        <oeo:OEO_00040001 rdf:datatype="http://www.w3.org/2001/XMLSchema#string">http://openenergy-platform.org/ontology/oeo/oeo-social</oeo:OEO_00040001>
        <obo:IAO_0000115>A delivery cost is a cost for a product or service that refers to the total unit cost of a product or commodity delivered to a certain market, city or customer. It is normally composed of all associated transport costs and the unit cost of production for that product.</obo:IAO_0000115>
        <obo:IAO_0000233>issue: https://github.com/OpenEnergyPlatform/ontology/issues/891
pull request: https://github.com/OpenEnergyPlatform/ontology/pull/1022

Reformulate definition to singular:
issue: https://github.com/OpenEnergyPlatform/ontology/issues/1257
pull request: https://github.com/OpenEnergyPlatform/ontology/pull/1260</obo:IAO_0000233>
        <rdfs:label>delivery cost</rdfs:label>
    </owl:Class>
    


    <!-- http://openenergy-platform.org/ontology/oeo/OEO_00030016 -->

    <owl:Class rdf:about="http://openenergy-platform.org/ontology/oeo/OEO_00030016">
        <rdfs:subClassOf rdf:resource="http://openenergy-platform.org/ontology/oeo/OEO_00030022"/>
        <rdfs:subClassOf>
            <owl:Restriction>
                <owl:onProperty rdf:resource="http://purl.obolibrary.org/obo/RO_0000087"/>
                <owl:someValuesFrom rdf:resource="http://openenergy-platform.org/ontology/oeo/OEO_00000045"/>
            </owl:Restriction>
        </rdfs:subClassOf>
        <oeo:OEO_00040001 rdf:datatype="http://www.w3.org/2001/XMLSchema#string">http://openenergy-platform.org/ontology/oeo/oeo-social</oeo:OEO_00040001>
        <obo:IAO_0000115>An organisational energy producer is an organisation that undertakes the generation of electricity and/or heat.&quot;</obo:IAO_0000115>
        <obo:IAO_0000118>organisational energy producer</obo:IAO_0000118>
        <obo:IAO_0000119>inspired by https://ec.europa.eu/eurostat/documents/38154/41386/Ele_AQ_documentation.pdf/a06bf650-1830-4fcb-9376-7be1f8ab080c</obo:IAO_0000119>
        <obo:IAO_0000233>issue: https://github.com/OpenEnergyPlatform/ontology/issues/314
pull request: https://github.com/OpenEnergyPlatform/ontology/pull/370</obo:IAO_0000233>
        <rdfs:label>organisational energy producer</rdfs:label>
    </owl:Class>
    


    <!-- http://openenergy-platform.org/ontology/oeo/OEO_00030017 -->

    <owl:Class rdf:about="http://openenergy-platform.org/ontology/oeo/OEO_00030017">
        <rdfs:subClassOf rdf:resource="http://openenergy-platform.org/ontology/oeo/OEO_00030016"/>
        <oeo:OEO_00040001 rdf:datatype="http://www.w3.org/2001/XMLSchema#string">http://openenergy-platform.org/ontology/oeo/oeo-social</oeo:OEO_00040001>
        <obo:IAO_0000115>An energy autoproducer is an organisational energy producer who produces electrical energy and/or heat wholly or partly for their own use as an activity which supports their primary activity.</obo:IAO_0000115>
        <obo:IAO_0000119>inspired by https://ec.europa.eu/eurostat/documents/38154/41386/Ele_AQ_documentation.pdf/a06bf650-1830-4fcb-9376-7be1f8ab080c</obo:IAO_0000119>
        <obo:IAO_0000233>issue: https://github.com/OpenEnergyPlatform/ontology/issues/314
pull request: https://github.com/OpenEnergyPlatform/ontology/pull/370</obo:IAO_0000233>
        <rdfs:comment>They may be privately or publicly owned.</rdfs:comment>
        <rdfs:label>energy autoproducer</rdfs:label>
    </owl:Class>
    


    <!-- http://openenergy-platform.org/ontology/oeo/OEO_00030018 -->

    <owl:Class rdf:about="http://openenergy-platform.org/ontology/oeo/OEO_00030018">
        <rdfs:subClassOf rdf:resource="http://openenergy-platform.org/ontology/oeo/OEO_00030016"/>
        <oeo:OEO_00040001 rdf:datatype="http://www.w3.org/2001/XMLSchema#string">http://openenergy-platform.org/ontology/oeo/oeo-social</oeo:OEO_00040001>
        <obo:IAO_0000115>A main activity energy producer is an organisational energy producer whose primary activity is electrical energy and/or heat production.</obo:IAO_0000115>
        <obo:IAO_0000119>inspired by https://ec.europa.eu/eurostat/documents/38154/41386/Ele_AQ_documentation.pdf/a06bf650-1830-4fcb-9376-7be1f8ab080c</obo:IAO_0000119>
        <obo:IAO_0000233>issue: https://github.com/OpenEnergyPlatform/ontology/issues/314
pull request: https://github.com/OpenEnergyPlatform/ontology/pull/370</obo:IAO_0000233>
        <rdfs:comment>They may be privately or publicly owned. Note that the sale need not take place through the public grid.</rdfs:comment>
        <rdfs:label>main activity energy producer</rdfs:label>
    </owl:Class>
    


    <!-- http://openenergy-platform.org/ontology/oeo/OEO_00030022 -->

    <owl:Class rdf:about="http://openenergy-platform.org/ontology/oeo/OEO_00030022"/>
    


    <!-- http://openenergy-platform.org/ontology/oeo/OEO_00030035 -->

    <owl:Class rdf:about="http://openenergy-platform.org/ontology/oeo/OEO_00030035"/>
    


    <!-- http://openenergy-platform.org/ontology/oeo/OEO_00040002 -->

    <owl:Class rdf:about="http://openenergy-platform.org/ontology/oeo/OEO_00040002">
        <rdfs:subClassOf rdf:resource="http://purl.obolibrary.org/obo/BFO_0000023"/>
        <oeo:OEO_00040001 rdf:datatype="http://www.w3.org/2001/XMLSchema#string">http://openenergy-platform.org/ontology/oeo/oeo-social</oeo:OEO_00040001>
        <obo:IAO_0000115>A role of an organisation, association, or group of persons, whether incorporated or unincorporated, which constitutes, maintains, or provides a facility for bringing together purchasers and sellers of financial instruments, commodities, or other products, services, or goods, and includes the market place and facilities maintained by the exchange</obo:IAO_0000115>
        <obo:IAO_0000118>exchange</obo:IAO_0000118>
        <obo:IAO_0000118>market</obo:IAO_0000118>
        <obo:IAO_0000119>fibo-fbc-fct-mkt:Exchange</obo:IAO_0000119>
        <obo:IAO_0000233>https://github.com/OpenEnergyPlatform/ontology/issues/341
https://github.com/OpenEnergyPlatform/ontology/pull/639

https://github.com/OpenEnergyPlatform/ontology/issues/677
https://github.com/OpenEnergyPlatform/ontology/pull/740

change label to market exchange role
https://github.com/OpenEnergyPlatform/ontology/pull/748</obo:IAO_0000233>
        <rdfs:label xml:lang="en">market exchange role</rdfs:label>
        <rdfs:seeAlso>https://spec.edmcouncil.org/fibo/ontology/FBC/FunctionalEntities/Markets/Exchange</rdfs:seeAlso>
    </owl:Class>
    


    <!-- http://openenergy-platform.org/ontology/oeo/OEO_00040003 -->

    <owl:Class rdf:about="http://openenergy-platform.org/ontology/oeo/OEO_00040003"/>
    


    <!-- http://openenergy-platform.org/ontology/oeo/OEO_00040004 -->

    <owl:Class rdf:about="http://openenergy-platform.org/ontology/oeo/OEO_00040004"/>
    


    <!-- http://openenergy-platform.org/ontology/oeo/OEO_00040005 -->

    <owl:Class rdf:about="http://openenergy-platform.org/ontology/oeo/OEO_00040005">
        <rdfs:subClassOf rdf:resource="http://openenergy-platform.org/ontology/oeo/OEO_00010083"/>
        <oeo:OEO_00040001 rdf:datatype="http://www.w3.org/2001/XMLSchema#string">http://openenergy-platform.org/ontology/oeo/oeo-social</oeo:OEO_00040001>
        <obo:IAO_0000115>A trader is a market participant that engages in the transfer of financial assets in any financial market on behalf of a client or a financial services provider.</obo:IAO_0000115>
        <obo:IAO_0000119>fibo-fbc-pas-fpas:Trader</obo:IAO_0000119>
        <obo:IAO_0000233>Implement in line with FIBO:
issue: https://github.com/OpenEnergyPlatform/ontology/issues/377
pull request: https://github.com/OpenEnergyPlatform/ontology/pull/641

Make trader subclass of market participant:
issue: https://github.com/OpenEnergyPlatform/ontology/issues/330
https://github.com/OpenEnergyPlatform/ontology/pull/745</obo:IAO_0000233>
        <rdfs:label xml:lang="en">trader</rdfs:label>
        <rdfs:seeAlso>https://spec.edmcouncil.org/fibo/ontology/FBC/ProductsAndServices/FinancialProductsAndServices/Trader</rdfs:seeAlso>
    </owl:Class>
    


    <!-- http://openenergy-platform.org/ontology/oeo/OEO_00040006 -->

    <owl:Class rdf:about="http://openenergy-platform.org/ontology/oeo/OEO_00040006">
        <rdfs:subClassOf rdf:resource="http://purl.obolibrary.org/obo/BFO_0000015"/>
        <oeo:OEO_00040001 rdf:datatype="http://www.w3.org/2001/XMLSchema#string">http://openenergy-platform.org/ontology/oeo/oeo-social</oeo:OEO_00040001>
        <obo:IAO_0000115>A request is a process whereby an agent asks another agent for something or to do something.</obo:IAO_0000115>
        <obo:IAO_0000119>https://spec.edmcouncil.org/fibo/ontology/FND/Arrangements/Communications/Request</obo:IAO_0000119>
        <obo:IAO_0000233>https://github.com/OpenEnergyPlatform/ontology/issues/376
https://github.com/OpenEnergyPlatform/ontology/pull/642</obo:IAO_0000233>
        <rdfs:label xml:lang="en">request</rdfs:label>
    </owl:Class>
    


    <!-- http://openenergy-platform.org/ontology/oeo/OEO_00040007 -->

    <owl:Class rdf:about="http://openenergy-platform.org/ontology/oeo/OEO_00040007">
        <rdfs:subClassOf rdf:resource="http://openenergy-platform.org/ontology/oeo/OEO_00040006"/>
        <oeo:OEO_00040001 rdf:datatype="http://www.w3.org/2001/XMLSchema#string">http://openenergy-platform.org/ontology/oeo/oeo-social</oeo:OEO_00040001>
        <obo:IAO_0000115>A price request is a request in which an agent asks another agent for a price.</obo:IAO_0000115>
        <obo:IAO_0000233>https://github.com/OpenEnergyPlatform/ontology/issues/376
https://github.com/OpenEnergyPlatform/ontology/pull/642</obo:IAO_0000233>
        <rdfs:label xml:lang="en">price request</rdfs:label>
    </owl:Class>
    


    <!-- http://openenergy-platform.org/ontology/oeo/OEO_00040008 -->

    <owl:Class rdf:about="http://openenergy-platform.org/ontology/oeo/OEO_00040008">
        <rdfs:subClassOf rdf:resource="http://openenergy-platform.org/ontology/oeo/OEO_00140012"/>
        <oeo:OEO_00040001 rdf:datatype="http://www.w3.org/2001/XMLSchema#string">http://openenergy-platform.org/ontology/oeo/oeo-social</oeo:OEO_00040001>
        <obo:IAO_0000115>Marginal cost is the economic value that corresponds to the change in the total cost that arises when the quantity produced is incremented by one unit; that is, it is the cost of producing one more unit of a good.</obo:IAO_0000115>
        <obo:IAO_0000119>O&apos;Sullivan, Arthur; Sheffrin, Steven M. (2003). Economics: Principles in Action.</obo:IAO_0000119>
        <obo:IAO_0000233>https://github.com/OpenEnergyPlatform/ontology/issues/376
https://github.com/OpenEnergyPlatform/ontology/pull/642</obo:IAO_0000233>
        <rdfs:label xml:lang="en">marginal cost</rdfs:label>
    </owl:Class>
    


    <!-- http://openenergy-platform.org/ontology/oeo/OEO_00040009 -->

    <owl:Class rdf:about="http://openenergy-platform.org/ontology/oeo/OEO_00040009"/>
    


    <!-- http://openenergy-platform.org/ontology/oeo/OEO_00040011 -->

    <owl:Class rdf:about="http://openenergy-platform.org/ontology/oeo/OEO_00040011"/>
    


    <!-- http://openenergy-platform.org/ontology/oeo/OEO_00090001 -->

    <owl:Class rdf:about="http://openenergy-platform.org/ontology/oeo/OEO_00090001"/>
    


    <!-- http://openenergy-platform.org/ontology/oeo/OEO_00090002 -->

    <owl:Class rdf:about="http://openenergy-platform.org/ontology/oeo/OEO_00090002">
        <rdfs:subClassOf rdf:resource="http://openenergy-platform.org/ontology/oeo/OEO_00090001"/>
        <oeo:OEO_00040001 rdf:datatype="http://www.w3.org/2001/XMLSchema#string">http://openenergy-platform.org/ontology/oeo/oeo-social</oeo:OEO_00040001>
        <obo:IAO_0000115>A public funder is a funder that gives public money.</obo:IAO_0000115>
        <obo:IAO_0000233>issue: https://github.com/OpenEnergyPlatform/ontology/issues/246
pull request: https://github.com/OpenEnergyPlatform/ontology/pull/776</obo:IAO_0000233>
        <rdfs:label xml:lang="en">public funder</rdfs:label>
    </owl:Class>
    


    <!-- http://openenergy-platform.org/ontology/oeo/OEO_00090003 -->

    <owl:Class rdf:about="http://openenergy-platform.org/ontology/oeo/OEO_00090003">
        <rdfs:subClassOf rdf:resource="http://openenergy-platform.org/ontology/oeo/OEO_00090001"/>
        <oeo:OEO_00040001 rdf:datatype="http://www.w3.org/2001/XMLSchema#string">http://openenergy-platform.org/ontology/oeo/oeo-social</oeo:OEO_00040001>
        <obo:IAO_0000115>A private funder is a funder that gives private money.</obo:IAO_0000115>
        <obo:IAO_0000233>issue: https://github.com/OpenEnergyPlatform/ontology/issues/246
pull request: https://github.com/OpenEnergyPlatform/ontology/pull/776</obo:IAO_0000233>
        <rdfs:label xml:lang="en">private funder</rdfs:label>
    </owl:Class>
    


    <!-- http://openenergy-platform.org/ontology/oeo/OEO_00140004 -->

    <owl:Class rdf:about="http://openenergy-platform.org/ontology/oeo/OEO_00140004"/>
    


    <!-- http://openenergy-platform.org/ontology/oeo/OEO_00140009 -->

    <owl:Class rdf:about="http://openenergy-platform.org/ontology/oeo/OEO_00140009"/>
    


    <!-- http://openenergy-platform.org/ontology/oeo/OEO_00140012 -->

    <owl:Class rdf:about="http://openenergy-platform.org/ontology/oeo/OEO_00140012"/>
    


    <!-- http://openenergy-platform.org/ontology/oeo/OEO_00140013 -->

    <owl:Class rdf:about="http://openenergy-platform.org/ontology/oeo/OEO_00140013">
        <rdfs:subClassOf rdf:resource="http://openenergy-platform.org/ontology/oeo/OEO_00140012"/>
        <oeo:OEO_00040001 rdf:datatype="http://www.w3.org/2001/XMLSchema#string">http://openenergy-platform.org/ontology/oeo/oeo-social</oeo:OEO_00040001>
        <obo:IAO_0000115>A gross domestic product is an economic value that represents the broadest measure of aggregate economic activity, measuring the total unduplicated market value of all final goods and services produced within a statistical area in a period.</obo:IAO_0000115>
        <obo:IAO_0000118>GDP</obo:IAO_0000118>
        <obo:IAO_0000233>issue: https://github.com/OpenEnergyPlatform/ontology/issues/454
pull request: https://github.com/OpenEnergyPlatform/ontology/pull/559
alternative term:
https://github.com/OpenEnergyPlatform/ontology/issues/675
https://github.com/OpenEnergyPlatform/ontology/pull/676</obo:IAO_0000233>
        <rdfs:label xml:lang="en">gross domestic product</rdfs:label>
    </owl:Class>
    


    <!-- http://openenergy-platform.org/ontology/oeo/OEO_00140023 -->

    <owl:Class rdf:about="http://openenergy-platform.org/ontology/oeo/OEO_00140023">
        <rdfs:subClassOf rdf:resource="http://openenergy-platform.org/ontology/oeo/OEO_00140012"/>
        <oeo:OEO_00040001 rdf:datatype="http://www.w3.org/2001/XMLSchema#string">http://openenergy-platform.org/ontology/oeo/oeo-social</oeo:OEO_00040001>
        <obo:IAO_0000115>Gross value added is an economic value that is the value of goods and services produced in a sector of an economy, measuring that sector&apos;s contribution to gross domestic product (GDP). It is calculated as the monetary value of products and services produced, less the value of intermediate consumption.</obo:IAO_0000115>
        <obo:IAO_0000118>GVA</obo:IAO_0000118>
        <obo:IAO_0000233>issue: https://github.com/OpenEnergyPlatform/ontology/issues/455
pull request: https://github.com/OpenEnergyPlatform/ontology/pull/563
alternative term:
https://github.com/OpenEnergyPlatform/ontology/issues/675
https://github.com/OpenEnergyPlatform/ontology/pull/676</obo:IAO_0000233>
        <rdfs:label xml:lang="en">gross value added</rdfs:label>
    </owl:Class>
    


    <!-- http://openenergy-platform.org/ontology/oeo/OEO_00140040 -->

    <owl:Class rdf:about="http://openenergy-platform.org/ontology/oeo/OEO_00140040"/>
    


    <!-- http://openenergy-platform.org/ontology/oeo/OEO_00140081 -->

    <owl:Class rdf:about="http://openenergy-platform.org/ontology/oeo/OEO_00140081"/>
    


    <!-- http://openenergy-platform.org/ontology/oeo/OEO_00140109 -->

    <owl:Class rdf:about="http://openenergy-platform.org/ontology/oeo/OEO_00140109">
        <rdfs:subClassOf rdf:resource="http://purl.obolibrary.org/obo/IAO_0000310"/>
        <oeo:OEO_00040001 rdf:datatype="http://www.w3.org/2001/XMLSchema#string">http://openenergy-platform.org/ontology/oeo/oeo-social</oeo:OEO_00040001>
        <obo:IAO_0000115>A contract is a document that contains an agreement between two or more competent agents to which those agents agree to be legally bound.</obo:IAO_0000115>
        <obo:IAO_0000119>https://spec.edmcouncil.org/fibo/ontology/FND/Agreements/Contracts/Contract</obo:IAO_0000119>
        <obo:IAO_0000233>issue: https://github.com/OpenEnergyPlatform/ontology/issues/376
pull request: https://github.com/OpenEnergyPlatform/ontology/pull/756</obo:IAO_0000233>
        <rdfs:label xml:lang="en">contract</rdfs:label>
    </owl:Class>
    


    <!-- http://openenergy-platform.org/ontology/oeo/OEO_00140117 -->

    <owl:Class rdf:about="http://openenergy-platform.org/ontology/oeo/OEO_00140117">
        <rdfs:subClassOf rdf:resource="http://purl.obolibrary.org/obo/BFO_0000038"/>
        <oeo:OEO_00040001 rdf:datatype="http://www.w3.org/2001/XMLSchema#string">http://openenergy-platform.org/ontology/oeo/oeo-social</oeo:OEO_00040001>
        <obo:IAO_0000115>Delivery time is a one-dimensional temporal region expressing the amount of time that it takes for goods that have been bought to arrive at the place where they are wanted.</obo:IAO_0000115>
        <obo:IAO_0000233>issue: https://github.com/OpenEnergyPlatform/ontology/issues/376
pull request: https://github.com/OpenEnergyPlatform/ontology/pull/778</obo:IAO_0000233>
        <rdfs:label xml:lang="en">delivery time</rdfs:label>
    </owl:Class>
    


    <!-- http://openenergy-platform.org/ontology/oeo/OEO_00140118 -->

    <owl:Class rdf:about="http://openenergy-platform.org/ontology/oeo/OEO_00140118">
        <rdfs:subClassOf rdf:resource="http://purl.obolibrary.org/obo/BFO_0000148"/>
        <oeo:OEO_00040001 rdf:datatype="http://www.w3.org/2001/XMLSchema#string">http://openenergy-platform.org/ontology/oeo/oeo-social</oeo:OEO_00040001>
        <obo:IAO_0000115>A delivery time point is a zero-dimensional temporal region expressing the point in time when goods that have been bought arrive at the place where they are wanted.</obo:IAO_0000115>
        <obo:IAO_0000233>issue: https://github.com/OpenEnergyPlatform/ontology/issues/376
pull request: https://github.com/OpenEnergyPlatform/ontology/pull/778</obo:IAO_0000233>
        <rdfs:label xml:lang="en">delivery time point</rdfs:label>
    </owl:Class>
    


    <!-- http://openenergy-platform.org/ontology/oeo/OEO_00140119 -->

    <owl:Class rdf:about="http://openenergy-platform.org/ontology/oeo/OEO_00140119">
        <rdfs:subClassOf rdf:resource="http://openenergy-platform.org/ontology/oeo/OEO_00000051"/>
        <oeo:OEO_00040001 rdf:datatype="http://www.w3.org/2001/XMLSchema#string">http://openenergy-platform.org/ontology/oeo/oeo-social</oeo:OEO_00040001>
        <obo:IAO_0000115>A sender is an agent who initiates a communication.</obo:IAO_0000115>
        <obo:IAO_0000233>issue: https://github.com/OpenEnergyPlatform/ontology/issues/376
pull request: https://github.com/OpenEnergyPlatform/ontology/pull/778</obo:IAO_0000233>
        <rdfs:label xml:lang="en">sender</rdfs:label>
    </owl:Class>
    


    <!-- http://openenergy-platform.org/ontology/oeo/OEO_00140120 -->

    <owl:Class rdf:about="http://openenergy-platform.org/ontology/oeo/OEO_00140120">
        <rdfs:subClassOf rdf:resource="http://openenergy-platform.org/ontology/oeo/OEO_00000051"/>
        <oeo:OEO_00040001 rdf:datatype="http://www.w3.org/2001/XMLSchema#string">http://openenergy-platform.org/ontology/oeo/oeo-social</oeo:OEO_00040001>
        <obo:IAO_0000115>A receiver is an agent who obtains information from a sender.</obo:IAO_0000115>
        <obo:IAO_0000233>issue: https://github.com/OpenEnergyPlatform/ontology/issues/376
pull request: https://github.com/OpenEnergyPlatform/ontology/pull/778</obo:IAO_0000233>
        <rdfs:label xml:lang="en">receiver</rdfs:label>
    </owl:Class>
    


    <!-- http://openenergy-platform.org/ontology/oeo/OEO_00140121 -->

    <owl:Class rdf:about="http://openenergy-platform.org/ontology/oeo/OEO_00140121">
        <rdfs:subClassOf rdf:resource="http://purl.obolibrary.org/obo/IAO_0000310"/>
        <oeo:OEO_00040001 rdf:datatype="http://www.w3.org/2001/XMLSchema#string">http://openenergy-platform.org/ontology/oeo/oeo-social</oeo:OEO_00040001>
        <obo:IAO_0000115>A bid is a document describing an offer made by an agent to another agent in an effort to exchange commodities or services via terms relating to price and quantity which will be part of the resulting contract.</obo:IAO_0000115>
        <obo:IAO_0000233>issue: https://github.com/OpenEnergyPlatform/ontology/issues/376
pull request: https://github.com/OpenEnergyPlatform/ontology/pull/778</obo:IAO_0000233>
        <rdfs:label xml:lang="en">bid</rdfs:label>
    </owl:Class>
    


    <!-- http://openenergy-platform.org/ontology/oeo/OEO_00140122 -->

    <owl:Class rdf:about="http://openenergy-platform.org/ontology/oeo/OEO_00140122">
        <rdfs:subClassOf rdf:resource="http://purl.obolibrary.org/obo/IAO_0000310"/>
        <oeo:OEO_00040001 rdf:datatype="http://www.w3.org/2001/XMLSchema#string">http://openenergy-platform.org/ontology/oeo/oeo-social</oeo:OEO_00040001>
        <obo:IAO_0000115>An award is a document that signifies that a supplier for a particular commodity or service specified in a bid has been accepted.</obo:IAO_0000115>
        <obo:IAO_0000233>issue: https://github.com/OpenEnergyPlatform/ontology/issues/376
pull request: https://github.com/OpenEnergyPlatform/ontology/pull/778</obo:IAO_0000233>
        <rdfs:label xml:lang="en">award</rdfs:label>
    </owl:Class>
    


    <!-- http://openenergy-platform.org/ontology/oeo/OEO_00140123 -->

    <owl:Class rdf:about="http://openenergy-platform.org/ontology/oeo/OEO_00140123">
        <rdfs:subClassOf rdf:resource="http://openenergy-platform.org/ontology/oeo/OEO_00000051"/>
        <oeo:OEO_00040001 rdf:datatype="http://www.w3.org/2001/XMLSchema#string">http://openenergy-platform.org/ontology/oeo/oeo-social</oeo:OEO_00040001>
        <obo:IAO_0000115>A provider is an agent that transfers commodities or services to other agents.</obo:IAO_0000115>
        <obo:IAO_0000119>https://spec.edmcouncil.org/fibo/ontology/FND/ProductsAndServices/ProductsAndServices/ServiceProvider (adapted)</obo:IAO_0000119>
        <obo:IAO_0000233>issue: https://github.com/OpenEnergyPlatform/ontology/issues/376
pull request: https://github.com/OpenEnergyPlatform/ontology/pull/778</obo:IAO_0000233>
        <rdfs:comment>The transfer is typically defined in a contract.</rdfs:comment>
        <rdfs:label xml:lang="en">provider</rdfs:label>
    </owl:Class>
    


    <!-- http://openenergy-platform.org/ontology/oeo/OEO_00140124 -->

    <owl:Class rdf:about="http://openenergy-platform.org/ontology/oeo/OEO_00140124">
        <rdfs:subClassOf rdf:resource="http://purl.obolibrary.org/obo/BFO_0000015"/>
        <oeo:OEO_00040001 rdf:datatype="http://www.w3.org/2001/XMLSchema#string">http://openenergy-platform.org/ontology/oeo/oeo-social</oeo:OEO_00040001>
        <obo:IAO_0000115>A service is a process that is an intangible actitvity performed by some agent for the benefit of another agent.</obo:IAO_0000115>
        <obo:IAO_0000119>https://spec.edmcouncil.org/fibo/ontology/FND/ProductsAndServices/ProductsAndServices/Service (adapted)</obo:IAO_0000119>
        <obo:IAO_0000233>issue: https://github.com/OpenEnergyPlatform/ontology/issues/376
pull request: https://github.com/OpenEnergyPlatform/ontology/pull/778</obo:IAO_0000233>
        <rdfs:label xml:lang="en">service</rdfs:label>
    </owl:Class>
    


    <!-- http://openenergy-platform.org/ontology/oeo/OEO_00140125 -->

    <owl:Class rdf:about="http://openenergy-platform.org/ontology/oeo/OEO_00140125">
        <rdfs:subClassOf rdf:resource="http://openenergy-platform.org/ontology/oeo/OEO_00030035"/>
        <oeo:OEO_00040001 rdf:datatype="http://www.w3.org/2001/XMLSchema#string">http://openenergy-platform.org/ontology/oeo/oeo-social</oeo:OEO_00040001>
        <obo:IAO_0000115>A delivery interval is the duration between repeated deliveries of services or commodities.</obo:IAO_0000115>
        <obo:IAO_0000233>issue: https://github.com/OpenEnergyPlatform/ontology/issues/256
pull request: https://github.com/OpenEnergyPlatform/ontology/pull/779</obo:IAO_0000233>
        <rdfs:comment>This duration is often contractually fixed and regular.</rdfs:comment>
        <rdfs:label xml:lang="en">delivery interval</rdfs:label>
    </owl:Class>
    


    <!-- http://openenergy-platform.org/ontology/oeo/OEO_00140130 -->

    <owl:Class rdf:about="http://openenergy-platform.org/ontology/oeo/OEO_00140130">
        <rdfs:subClassOf rdf:resource="http://openenergy-platform.org/ontology/oeo/OEO_00000051"/>
        <oeo:OEO_00040001 rdf:datatype="http://www.w3.org/2001/XMLSchema#string">http://openenergy-platform.org/ontology/oeo/oeo-social</oeo:OEO_00040001>
        <obo:IAO_0000115>A power plant operator is an agent that operates an electric utility generation station.</obo:IAO_0000115>
        <obo:IAO_0000233>issue: https://github.com/OpenEnergyPlatform/ontology/issues/256
pull request: https://github.com/OpenEnergyPlatform/ontology/pull/779</obo:IAO_0000233>
        <rdfs:label xml:lang="en">power plant operator</rdfs:label>
    </owl:Class>
    


    <!-- http://openenergy-platform.org/ontology/oeo/OEO_00140131 -->

    <owl:Class rdf:about="http://openenergy-platform.org/ontology/oeo/OEO_00140131">
        <rdfs:subClassOf rdf:resource="http://openenergy-platform.org/ontology/oeo/OEO_00040005"/>
        <oeo:OEO_00040001 rdf:datatype="http://www.w3.org/2001/XMLSchema#string">http://openenergy-platform.org/ontology/oeo/oeo-social</oeo:OEO_00040001>
        <obo:IAO_0000115>A trader that trades the power of fossil fuel power plants.</obo:IAO_0000115>
        <obo:IAO_0000233>issue: https://github.com/OpenEnergyPlatform/ontology/issues/256
pull request: https://github.com/OpenEnergyPlatform/ontology/pull/779</obo:IAO_0000233>
        <rdfs:label xml:lang="en">conventional trader</rdfs:label>
    </owl:Class>
    


    <!-- http://openenergy-platform.org/ontology/oeo/OEO_00140136 -->

    <owl:Class rdf:about="http://openenergy-platform.org/ontology/oeo/OEO_00140136">
        <rdfs:subClassOf rdf:resource="http://purl.obolibrary.org/obo/IAO_0000104"/>
        <oeo:OEO_00040001 rdf:datatype="http://www.w3.org/2001/XMLSchema#string">http://openenergy-platform.org/ontology/oeo/oeo-social</oeo:OEO_00040001>
        <obo:IAO_0000115>Dispatch assignment is a plan specification that refers to resource planning at a power plant (usually by the plant’s operator).</obo:IAO_0000115>
        <obo:IAO_0000233>issue: https://github.com/OpenEnergyPlatform/ontology/issues/376
pull request: https://github.com/OpenEnergyPlatform/ontology/pull/792</obo:IAO_0000233>
        <rdfs:label xml:lang="en">dispatch assignment</rdfs:label>
    </owl:Class>
    


    <!-- http://openenergy-platform.org/ontology/oeo/OEO_00140137 -->

    <owl:Class rdf:about="http://openenergy-platform.org/ontology/oeo/OEO_00140137">
        <rdfs:subClassOf rdf:resource="http://purl.obolibrary.org/obo/IAO_0000030"/>
        <oeo:OEO_00040001 rdf:datatype="http://www.w3.org/2001/XMLSchema#string">http://openenergy-platform.org/ontology/oeo/oeo-social</oeo:OEO_00040001>
        <obo:IAO_0000115>A power plant portfolio is an information content entity that describes a particular combination or mix of different power plants, e.g. renewables and fossil plants within one business unit or company or trader.</obo:IAO_0000115>
        <obo:IAO_0000233>issue: https://github.com/OpenEnergyPlatform/ontology/issues/376
pull request: https://github.com/OpenEnergyPlatform/ontology/pull/792</obo:IAO_0000233>
        <rdfs:label xml:lang="en">power plant portfolio</rdfs:label>
    </owl:Class>
    


    <!-- http://openenergy-platform.org/ontology/oeo/OEO_00140140 -->

    <owl:Class rdf:about="http://openenergy-platform.org/ontology/oeo/OEO_00140140">
        <rdfs:subClassOf rdf:resource="http://openenergy-platform.org/ontology/oeo/OEO_00040005"/>
        <oeo:OEO_00040001 rdf:datatype="http://www.w3.org/2001/XMLSchema#string">http://openenergy-platform.org/ontology/oeo/oeo-social</oeo:OEO_00040001>
        <obo:IAO_0000115>A demand trader is a trader that deals specifically with energy demand.</obo:IAO_0000115>
        <obo:IAO_0000233>issue: https://github.com/OpenEnergyPlatform/ontology/issues/256
pull request: https://github.com/OpenEnergyPlatform/ontology/pull/793</obo:IAO_0000233>
        <rdfs:label xml:lang="en">demand trader</rdfs:label>
    </owl:Class>
    


    <!-- http://openenergy-platform.org/ontology/oeo/OEO_00140141 -->

    <owl:Class rdf:about="http://openenergy-platform.org/ontology/oeo/OEO_00140141">
        <rdfs:subClassOf rdf:resource="http://purl.obolibrary.org/obo/IAO_0000104"/>
        <oeo:OEO_00040001 rdf:datatype="http://www.w3.org/2001/XMLSchema#string">http://openenergy-platform.org/ontology/oeo/oeo-social</oeo:OEO_00040001>
        <obo:IAO_0000115>A merit order is a plan specification that describes the dispatch ranking of power plants (electrical generation) based on ascending order of price.</obo:IAO_0000115>
        <obo:IAO_0000233>issue: https://github.com/OpenEnergyPlatform/ontology/issues/256
pull request: https://github.com/OpenEnergyPlatform/ontology/pull/793</obo:IAO_0000233>
        <rdfs:label xml:lang="en">merit order</rdfs:label>
    </owl:Class>
    


    <!-- http://openenergy-platform.org/ontology/oeo/OEO_00140143 -->

    <owl:Class rdf:about="http://openenergy-platform.org/ontology/oeo/OEO_00140143">
        <rdfs:subClassOf rdf:resource="http://openenergy-platform.org/ontology/oeo/OEO_00040005"/>
        <oeo:OEO_00040001 rdf:datatype="http://www.w3.org/2001/XMLSchema#string">http://openenergy-platform.org/ontology/oeo/oeo-social</oeo:OEO_00040001>
        <obo:IAO_0000115>A direct marketer is a trader who is the relay between the energy exchange and power plant operators.</obo:IAO_0000115>
        <obo:IAO_0000233>issue: https://github.com/OpenEnergyPlatform/ontology/issues/256
pull request: https://github.com/OpenEnergyPlatform/ontology/pull/793</obo:IAO_0000233>
        <rdfs:label xml:lang="en">direct marketer</rdfs:label>
    </owl:Class>
    


    <!-- http://openenergy-platform.org/ontology/oeo/OEO_00140146 -->

    <owl:Class rdf:about="http://openenergy-platform.org/ontology/oeo/OEO_00140146">
        <rdfs:subClassOf rdf:resource="http://openenergy-platform.org/ontology/oeo/OEO_00140040"/>
        <oeo:OEO_00040001 rdf:datatype="http://www.w3.org/2001/XMLSchema#string">http://openenergy-platform.org/ontology/oeo/oeo-social</oeo:OEO_00040001>
        <obo:IAO_0000115>Energy demand is a demand for energy.</obo:IAO_0000115>
        <obo:IAO_0000233>issue: https://github.com/OpenEnergyPlatform/ontology/issues/794
pull request: https://github.com/OpenEnergyPlatform/ontology/pull/796</obo:IAO_0000233>
        <rdfs:label xml:lang="en">energy demand</rdfs:label>
    </owl:Class>
    


    <!-- http://openenergy-platform.org/ontology/oeo/OEO_00140149 -->

    <owl:Class rdf:about="http://openenergy-platform.org/ontology/oeo/OEO_00140149">
        <rdfs:subClassOf rdf:resource="http://purl.obolibrary.org/obo/BFO_0000015"/>
        <oeo:OEO_00040001 rdf:datatype="http://www.w3.org/2001/XMLSchema#string">http://openenergy-platform.org/ontology/oeo/oeo-social</oeo:OEO_00040001>
        <obo:IAO_0000115>A transformative measure is a process that is an activity that has a direct impact on a specific variable in question.</obo:IAO_0000115>
        <obo:IAO_0000233>issue: https://github.com/OpenEnergyPlatform/ontology/issues/444
pull request: https://github.com/OpenEnergyPlatform/ontology/pull/797</obo:IAO_0000233>
        <rdfs:label xml:lang="en">transformative measure</rdfs:label>
    </owl:Class>
    


    <!-- http://openenergy-platform.org/ontology/oeo/OEO_00140150 -->

    <owl:Class rdf:about="http://openenergy-platform.org/ontology/oeo/OEO_00140150">
        <rdfs:subClassOf rdf:resource="http://purl.obolibrary.org/obo/BFO_0000020"/>
        <rdfs:subClassOf>
            <owl:Restriction>
                <owl:onProperty rdf:resource="http://openenergy-platform.org/ontology/oeo/OEO_00010121"/>
                <owl:someValuesFrom rdf:resource="http://openenergy-platform.org/ontology/oeo/OEO_00030022"/>
            </owl:Restriction>
        </rdfs:subClassOf>
        <rdfs:subClassOf>
            <owl:Restriction>
                <owl:onProperty rdf:resource="http://purl.obolibrary.org/obo/BFO_0000051"/>
                <owl:someValuesFrom rdf:resource="http://openenergy-platform.org/ontology/oeo/OEO_00140151"/>
            </owl:Restriction>
        </rdfs:subClassOf>
        <oeo:OEO_00040001 rdf:datatype="http://www.w3.org/2001/XMLSchema#string">http://openenergy-platform.org/ontology/oeo/oeo-social</oeo:OEO_00040001>
        <obo:IAO_0000115>A policy is a specifically dependent continuant that is a deliberate system of principles, rules and guidelines, adopted by an organisation to guide decision making with respect to particular situations and implemented to achieve stated goals.</obo:IAO_0000115>
        <obo:IAO_0000233>issue: https://github.com/OpenEnergyPlatform/ontology/issues/444
pull request: https://github.com/OpenEnergyPlatform/ontology/pull/797

relations:
issue: https://github.com/OpenEnergyPlatform/ontology/issues/444
pull request: https://github.com/OpenEnergyPlatform/ontology/pull/853</obo:IAO_0000233>
        <rdfs:label xml:lang="en">policy</rdfs:label>
    </owl:Class>
    


    <!-- http://openenergy-platform.org/ontology/oeo/OEO_00140151 -->

    <owl:Class rdf:about="http://openenergy-platform.org/ontology/oeo/OEO_00140151">
        <rdfs:subClassOf rdf:resource="http://purl.obolibrary.org/obo/BFO_0000020"/>
        <rdfs:subClassOf>
            <owl:Restriction>
                <owl:onProperty rdf:resource="http://openenergy-platform.org/ontology/oeo/OEO_00010119"/>
                <owl:someValuesFrom rdf:resource="http://openenergy-platform.org/ontology/oeo/OEO_00140149"/>
            </owl:Restriction>
        </rdfs:subClassOf>
        <oeo:OEO_00040001 rdf:datatype="http://www.w3.org/2001/XMLSchema#string">http://openenergy-platform.org/ontology/oeo/oeo-social</oeo:OEO_00040001>
        <obo:IAO_0000115>A policy instrument is a specifically dependent continuant that is an action by the government that is intended to promote the adoption of a (transformative) measure.</obo:IAO_0000115>
        <obo:IAO_0000233>issue: https://github.com/OpenEnergyPlatform/ontology/issues/444
pull request: https://github.com/OpenEnergyPlatform/ontology/pull/797</obo:IAO_0000233>
        <rdfs:label xml:lang="en">policy instrument</rdfs:label>
    </owl:Class>
    <owl:Axiom>
        <owl:annotatedSource rdf:resource="http://openenergy-platform.org/ontology/oeo/OEO_00140151"/>
        <owl:annotatedProperty rdf:resource="http://www.w3.org/2000/01/rdf-schema#subClassOf"/>
        <owl:annotatedTarget>
            <owl:Restriction>
                <owl:onProperty rdf:resource="http://openenergy-platform.org/ontology/oeo/OEO_00010119"/>
                <owl:someValuesFrom rdf:resource="http://openenergy-platform.org/ontology/oeo/OEO_00140149"/>
            </owl:Restriction>
        </owl:annotatedTarget>
        <obo:IAO_0000233>issue: https://github.com/OpenEnergyPlatform/ontology/issues/444
pull request: https://github.com/OpenEnergyPlatform/ontology/pull/853</obo:IAO_0000233>
    </owl:Axiom>
    


    <!-- http://openenergy-platform.org/ontology/oeo/OEO_00140171 -->

    <owl:Class rdf:about="http://openenergy-platform.org/ontology/oeo/OEO_00140171">
        <rdfs:subClassOf rdf:resource="http://purl.obolibrary.org/obo/IAO_0000030"/>
        <oeo:OEO_00040001 rdf:datatype="http://www.w3.org/2001/XMLSchema#string">http://openenergy-platform.org/ontology/oeo/oeo-social</oeo:OEO_00040001>
        <obo:IAO_0000115>An email address is an information content entity that identifies an email box to which messages are delivered.</obo:IAO_0000115>
        <obo:IAO_0000233>issue: https://github.com/OpenEnergyPlatform/ontology/issues/818
pull request: https://github.com/OpenEnergyPlatform/ontology/pull/827</obo:IAO_0000233>
        <rdfs:label xml:lang="en">email address</rdfs:label>
    </owl:Class>
    


    <!-- http://openenergy-platform.org/ontology/oeo/OEO_00160005 -->

    <owl:Class rdf:about="http://openenergy-platform.org/ontology/oeo/OEO_00160005">
        <rdfs:subClassOf rdf:resource="http://openenergy-platform.org/ontology/oeo/OEO_00020145"/>
        <obo:IAO_0000115>A fuel cost is a variable cost that depends on the type and amount of fuel.</obo:IAO_0000115>
        <obo:IAO_0000233>issue: https://github.com/OpenEnergyPlatform/ontology/issues/1257
pull request: https://github.com/OpenEnergyPlatform/ontology/pull/1260</obo:IAO_0000233>
        <rdfs:label xml:lang="en">fuel cost</rdfs:label>
    </owl:Class>
    


    <!-- http://openenergy-platform.org/ontology/oeo/OEO_00230013 -->

    <owl:Class rdf:about="http://openenergy-platform.org/ontology/oeo/OEO_00230013">
        <rdfs:subClassOf rdf:resource="http://purl.obolibrary.org/obo/BFO_0000027"/>
        <oeo:OEO_00040001 rdf:datatype="http://www.w3.org/2001/XMLSchema#string">http://openenergy-platform.org/ontology/oeo/oeo-social</oeo:OEO_00040001>
        <obo:IAO_0000115 xml:lang="en">A population is an aggregate of people in a spatial region.</obo:IAO_0000115>
        <obo:IAO_0000233 xml:lang="en">issue: https://github.com/OpenEnergyPlatform/ontology/issues/479
https://github.com/OpenEnergyPlatform/ontology/issues/301
pull request: https://github.com/OpenEnergyPlatform/ontology/pull/491</obo:IAO_0000233>
        <rdfs:label xml:lang="en">population</rdfs:label>
    </owl:Class>
    


    <!-- http://openenergy-platform.org/ontology/oeo/OEO_00230014 -->

    <owl:Class rdf:about="http://openenergy-platform.org/ontology/oeo/OEO_00230014">
        <rdfs:subClassOf rdf:resource="http://openenergy-platform.org/ontology/oeo/OEO_00230013"/>
        <owl:disjointWith rdf:resource="http://openenergy-platform.org/ontology/oeo/OEO_00230015"/>
        <oeo:OEO_00040001 rdf:datatype="http://www.w3.org/2001/XMLSchema#string">http://openenergy-platform.org/ontology/oeo/oeo-social</oeo:OEO_00040001>
        <obo:IAO_0000115 xml:lang="en">An urban population is a population living in urban areas, as defined by national statistical offices.</obo:IAO_0000115>
        <obo:IAO_0000119 xml:lang="en">United Nations Population Division. World Urbanization Prospects: 2018 Revision.</obo:IAO_0000119>
        <obo:IAO_0000233 xml:lang="en">issue: https://github.com/OpenEnergyPlatform/ontology/issues/479
https://github.com/OpenEnergyPlatform/ontology/issues/301
pull request: https://github.com/OpenEnergyPlatform/ontology/pull/491</obo:IAO_0000233>
        <rdfs:label xml:lang="en">urban population</rdfs:label>
    </owl:Class>
    


    <!-- http://openenergy-platform.org/ontology/oeo/OEO_00230015 -->

    <owl:Class rdf:about="http://openenergy-platform.org/ontology/oeo/OEO_00230015">
        <rdfs:subClassOf rdf:resource="http://openenergy-platform.org/ontology/oeo/OEO_00230013"/>
        <oeo:OEO_00040001 rdf:datatype="http://www.w3.org/2001/XMLSchema#string">http://openenergy-platform.org/ontology/oeo/oeo-social</oeo:OEO_00040001>
        <obo:IAO_0000115 xml:lang="en">A rural population is a population living in rural areas, as defined by national statistical offices.</obo:IAO_0000115>
        <obo:IAO_0000119 xml:lang="en">United Nations Population Division. World Urbanization Prospects: 2018 Revision.</obo:IAO_0000119>
        <obo:IAO_0000233 xml:lang="en">issue: https://github.com/OpenEnergyPlatform/ontology/issues/301
https://github.com/OpenEnergyPlatform/ontology/issues/479
pull request: https://github.com/OpenEnergyPlatform/ontology/pull/491</obo:IAO_0000233>
        <rdfs:label xml:lang="en">rural population</rdfs:label>
    </owl:Class>
    


    <!-- http://openenergy-platform.org/ontology/oeo/OEO_00230016 -->

    <owl:Class rdf:about="http://openenergy-platform.org/ontology/oeo/OEO_00230016">
        <rdfs:subClassOf rdf:resource="http://openenergy-platform.org/ontology/oeo/OEO_00230013"/>
        <oeo:OEO_00040001 rdf:datatype="http://www.w3.org/2001/XMLSchema#string">http://openenergy-platform.org/ontology/oeo/oeo-social</oeo:OEO_00040001>
        <obo:IAO_0000115 xml:lang="en">The labour force is the population of people ages 15 and older who supply labour to the production of goods and services.  It includes people who are currently employed and people who are unemployed but seeking work as well as first-time job-seekers.</obo:IAO_0000115>
        <obo:IAO_0000118>labor force</obo:IAO_0000118>
        <obo:IAO_0000119 xml:lang="en">https://databank.worldbank.org/reports.aspx?source=2&amp;type=metadata&amp;series=SL.TLF.TOTL.IN</obo:IAO_0000119>
        <obo:IAO_0000233 xml:lang="en">issue: https://github.com/OpenEnergyPlatform/ontology/issues/479
https://github.com/OpenEnergyPlatform/ontology/issues/301
pull request: https://github.com/OpenEnergyPlatform/ontology/pull/491</obo:IAO_0000233>
        <rdfs:label xml:lang="en">labour force</rdfs:label>
    </owl:Class>
    


    <!-- http://openenergy-platform.org/ontology/oeo/OEO_00230017 -->

    <owl:Class rdf:about="http://openenergy-platform.org/ontology/oeo/OEO_00230017">
        <rdfs:subClassOf rdf:resource="http://openenergy-platform.org/ontology/oeo/OEO_00230013"/>
        <oeo:OEO_00040001 rdf:datatype="http://www.w3.org/2001/XMLSchema#string">http://openenergy-platform.org/ontology/oeo/oeo-social</oeo:OEO_00040001>
        <obo:IAO_0000115 xml:lang="en">The working age population is the population of people aged 15 to 65.</obo:IAO_0000115>
        <obo:IAO_0000233 xml:lang="en">issue: https://github.com/OpenEnergyPlatform/ontology/issues/301
https://github.com/OpenEnergyPlatform/ontology/issues/479
pull request: https://github.com/OpenEnergyPlatform/ontology/pull/491</obo:IAO_0000233>
        <rdfs:label xml:lang="en">working age population</rdfs:label>
    </owl:Class>
    


    <!-- http://openenergy-platform.org/ontology/oeo/OEO_00240003 -->

    <owl:Class rdf:about="http://openenergy-platform.org/ontology/oeo/OEO_00240003"/>
    


    <!-- http://openenergy-platform.org/ontology/oeo/OEO_00240021 -->

    <owl:Class rdf:about="http://openenergy-platform.org/ontology/oeo/OEO_00240021">
        <rdfs:subClassOf rdf:resource="http://openenergy-platform.org/ontology/oeo/OEO_00140012"/>
        <rdfs:subClassOf>
            <owl:Restriction>
                <owl:onProperty rdf:resource="http://openenergy-platform.org/ontology/oeo/OEO_00040010"/>
                <owl:someValuesFrom rdf:resource="http://purl.obolibrary.org/obo/UO_0000187"/>
            </owl:Restriction>
        </rdfs:subClassOf>
        <oeo:OEO_00040001 rdf:datatype="http://www.w3.org/2001/XMLSchema#string">http://openenergy-platform.org/ontology/oeo/oeo-social</oeo:OEO_00040001>
        <obo:IAO_0000115 xml:lang="en">A discount rate is an economic value with the unit percent that refers to the interest rate used in discounted cash flow (DCF) analysis to determine the present value of future cash flows.</obo:IAO_0000115>
        <obo:IAO_0000233 xml:lang="en">issue: https://github.com/OpenEnergyPlatform/ontology/issues/1049
pull request: https://github.com/OpenEnergyPlatform/ontology/pull/1077</obo:IAO_0000233>
        <rdfs:label>discount rate</rdfs:label>
    </owl:Class>
    


    <!-- http://openenergy-platform.org/ontology/oeo/OEO_00240036 -->

    <owl:Class rdf:about="http://openenergy-platform.org/ontology/oeo/OEO_00240036">
        <rdfs:subClassOf rdf:resource="http://openenergy-platform.org/ontology/oeo/OEO_00040003"/>
        <oeo:OEO_00040001 rdf:datatype="http://www.w3.org/2001/XMLSchema#string">http://openenergy-platform.org/ontology/oeo/oeo-social</oeo:OEO_00040001>
        <obo:IAO_0000115 xml:lang="en">An import price is the monetary price for the import of a material entity.</obo:IAO_0000115>
        <obo:IAO_0000233>issue: https://github.com/OpenEnergyPlatform/ontology/issues/1050
pull request: https://github.com/OpenEnergyPlatform/ontology/pull/1083</obo:IAO_0000233>
        <rdfs:label>import price</rdfs:label>
    </owl:Class>
    


    <!-- http://openenergy-platform.org/ontology/oeo/OEO_00240037 -->

    <owl:Class rdf:about="http://openenergy-platform.org/ontology/oeo/OEO_00240037">
        <rdfs:subClassOf rdf:resource="http://openenergy-platform.org/ontology/oeo/OEO_00040003"/>
        <oeo:OEO_00040001 rdf:datatype="http://www.w3.org/2001/XMLSchema#string">http://openenergy-platform.org/ontology/oeo/oeo-social</oeo:OEO_00040001>
        <obo:IAO_0000115 xml:lang="en">An export price is the monetary price for the export of a material entity.</obo:IAO_0000115>
        <obo:IAO_0000233>issue: https://github.com/OpenEnergyPlatform/ontology/issues/1050
pull request: https://github.com/OpenEnergyPlatform/ontology/pull/1083</obo:IAO_0000233>
        <rdfs:label>export price</rdfs:label>
    </owl:Class>
    


    <!-- http://openenergy-platform.org/ontology/oeo/OEO_00260007 -->

    <owl:Class rdf:about="http://openenergy-platform.org/ontology/oeo/OEO_00260007">
        <owl:equivalentClass>
            <owl:Class>
                <owl:intersectionOf rdf:parseType="Collection">
                    <rdf:Description rdf:about="http://openenergy-platform.org/ontology/oeo/OEO_00000147"/>
                    <owl:Restriction>
                        <owl:onProperty rdf:resource="http://purl.obolibrary.org/obo/RO_0000057"/>
                        <owl:someValuesFrom rdf:resource="http://openenergy-platform.org/ontology/oeo/OEO_00000006"/>
                    </owl:Restriction>
                </owl:intersectionOf>
            </owl:Class>
        </owl:equivalentClass>
        <rdfs:subClassOf rdf:resource="http://openenergy-platform.org/ontology/oeo/OEO_00000147"/>
        <obo:IAO_0000115 xml:lang="en">A CO2 emission is an emission that releases carbon dioxide.</obo:IAO_0000115>
        <obo:IAO_0000233 xml:lang="en">issue: https://github.com/OpenEnergyPlatform/ontology/issues/866
pull request: https://github.com/OpenEnergyPlatform/ontology/pull/1253/</obo:IAO_0000233>
        <rdfs:label xml:lang="en">CO2 emission</rdfs:label>
        <rdfs:label xml:lang="en">carbon dioxide emission</rdfs:label>
    </owl:Class>
    


    <!-- http://openenergy-platform.org/ontology/oeo/OEO_00260008 -->

    <owl:Class rdf:about="http://openenergy-platform.org/ontology/oeo/OEO_00260008">
        <rdfs:subClassOf rdf:resource="http://openenergy-platform.org/ontology/oeo/OEO_00140081"/>
        <obo:IAO_0000115 xml:lang="en">A CO2 emission value is greenhouse gas emission value that quantifies the output of a CO2 emission process.</obo:IAO_0000115>
        <obo:IAO_0000233 xml:lang="en">issue: https://github.com/OpenEnergyPlatform/ontology/issues/866
pull request: https://github.com/OpenEnergyPlatform/ontology/pull/1253/</obo:IAO_0000233>
        <rdfs:label xml:lang="en">CO2 emission value</rdfs:label>
        <rdfs:label xml:lang="en">carbon dioxide emission value</rdfs:label>
    </owl:Class>
    


    <!-- http://purl.obolibrary.org/obo/BFO_0000002 -->

    <owl:Class rdf:about="http://purl.obolibrary.org/obo/BFO_0000002"/>
    


    <!-- http://purl.obolibrary.org/obo/BFO_0000003 -->

    <owl:Class rdf:about="http://purl.obolibrary.org/obo/BFO_0000003"/>
    


    <!-- http://purl.obolibrary.org/obo/BFO_0000004 -->

    <owl:Class rdf:about="http://purl.obolibrary.org/obo/BFO_0000004"/>
    


    <!-- http://purl.obolibrary.org/obo/BFO_0000006 -->

    <owl:Class rdf:about="http://purl.obolibrary.org/obo/BFO_0000006"/>
    


    <!-- http://purl.obolibrary.org/obo/BFO_0000009 -->

    <owl:Class rdf:about="http://purl.obolibrary.org/obo/BFO_0000009"/>
    


    <!-- http://purl.obolibrary.org/obo/BFO_0000015 -->

    <owl:Class rdf:about="http://purl.obolibrary.org/obo/BFO_0000015"/>
    


    <!-- http://purl.obolibrary.org/obo/BFO_0000016 -->

    <owl:Class rdf:about="http://purl.obolibrary.org/obo/BFO_0000016"/>
    


    <!-- http://purl.obolibrary.org/obo/BFO_0000017 -->

    <owl:Class rdf:about="http://purl.obolibrary.org/obo/BFO_0000017"/>
    


    <!-- http://purl.obolibrary.org/obo/BFO_0000019 -->

    <owl:Class rdf:about="http://purl.obolibrary.org/obo/BFO_0000019"/>
    


    <!-- http://purl.obolibrary.org/obo/BFO_0000020 -->

    <owl:Class rdf:about="http://purl.obolibrary.org/obo/BFO_0000020"/>
    


    <!-- http://purl.obolibrary.org/obo/BFO_0000023 -->

    <owl:Class rdf:about="http://purl.obolibrary.org/obo/BFO_0000023"/>
    


    <!-- http://purl.obolibrary.org/obo/BFO_0000024 -->

    <owl:Class rdf:about="http://purl.obolibrary.org/obo/BFO_0000024"/>
    


    <!-- http://purl.obolibrary.org/obo/BFO_0000027 -->

    <owl:Class rdf:about="http://purl.obolibrary.org/obo/BFO_0000027"/>
    


    <!-- http://purl.obolibrary.org/obo/BFO_0000029 -->

    <owl:Class rdf:about="http://purl.obolibrary.org/obo/BFO_0000029"/>
    


    <!-- http://purl.obolibrary.org/obo/BFO_0000030 -->

    <owl:Class rdf:about="http://purl.obolibrary.org/obo/BFO_0000030"/>
    


    <!-- http://purl.obolibrary.org/obo/BFO_0000031 -->

    <owl:Class rdf:about="http://purl.obolibrary.org/obo/BFO_0000031"/>
    


    <!-- http://purl.obolibrary.org/obo/BFO_0000038 -->

    <owl:Class rdf:about="http://purl.obolibrary.org/obo/BFO_0000038"/>
    


    <!-- http://purl.obolibrary.org/obo/BFO_0000040 -->

    <owl:Class rdf:about="http://purl.obolibrary.org/obo/BFO_0000040"/>
    


    <!-- http://purl.obolibrary.org/obo/BFO_0000141 -->

    <owl:Class rdf:about="http://purl.obolibrary.org/obo/BFO_0000141"/>
    


    <!-- http://purl.obolibrary.org/obo/BFO_0000148 -->

    <owl:Class rdf:about="http://purl.obolibrary.org/obo/BFO_0000148"/>
    


    <!-- http://purl.obolibrary.org/obo/IAO_0000030 -->

    <owl:Class rdf:about="http://purl.obolibrary.org/obo/IAO_0000030"/>
    


    <!-- http://purl.obolibrary.org/obo/IAO_0000104 -->

    <owl:Class rdf:about="http://purl.obolibrary.org/obo/IAO_0000104"/>
    


    <!-- http://purl.obolibrary.org/obo/IAO_0000310 -->

    <owl:Class rdf:about="http://purl.obolibrary.org/obo/IAO_0000310"/>
    


    <!-- http://purl.obolibrary.org/obo/RO_0002577 -->

    <owl:Class rdf:about="http://purl.obolibrary.org/obo/RO_0002577"/>
    


    <!-- http://purl.obolibrary.org/obo/UO_0000000 -->

    <owl:Class rdf:about="http://purl.obolibrary.org/obo/UO_0000000"/>
    


    <!-- http://purl.obolibrary.org/obo/UO_0000187 -->

    <owl:Class rdf:about="http://purl.obolibrary.org/obo/UO_0000187"/>
    


    <!-- http://purl.obolibrary.org/obo/UO_0000190 -->

    <owl:Class rdf:about="http://purl.obolibrary.org/obo/UO_0000190"/>
    


    <!-- http://purl.obolibrary.org/obo/UO_0010006 -->

    <owl:Class rdf:about="http://purl.obolibrary.org/obo/UO_0010006"/>
    


    <!-- 
    ///////////////////////////////////////////////////////////////////////////////////////
    //
    // Individuals
    //
    ///////////////////////////////////////////////////////////////////////////////////////
     -->

    


    <!-- http://openenergy-platform.org/ontology/oeo/OEO_00000160 -->

    <owl:NamedIndividual rdf:about="http://openenergy-platform.org/ontology/oeo/OEO_00000160">
        <rdf:type rdf:resource="http://openenergy-platform.org/ontology/oeo/OEO_00000368"/>
        <oeo:OEO_00040001 rdf:datatype="http://www.w3.org/2001/XMLSchema#string">http://openenergy-platform.org/ontology/oeo/oeo-social</oeo:OEO_00040001>
        <obo:IAO_0000115>The concept of &quot;energy balance&quot; is an accounting framework for the compilation and understanding of data on all energy products entering, exiting and being used in a country. The energy balance is the most complete statistical accounting of energy products and their flow in the economy. Columns of the energy balance represent energy products (fuels). Rows represent energy flows.

The energy balance expresses all forms of energy in a common accounting unit. The balance shows the relationships between supply, inputs to the energy transformation processes and their outputs as well as the actual energy consumption by different sectors of end-use.</obo:IAO_0000115>
        <obo:IAO_0000116>This is a general description of an energy balance. A link to a complete Eurostat energy balance is provided under the URL for &apos;definition source&apos;</obo:IAO_0000116>
        <obo:IAO_0000119>https://ec.europa.eu/eurostat/statistics-explained/index.php/Energy_balance#What_is_an_energy_balance.3F</obo:IAO_0000119>
        <rdfs:label>eurostat energy balances</rdfs:label>
    </owl:NamedIndividual>
    


    <!-- http://openenergy-platform.org/ontology/oeo/OEO_00000193 -->

    <owl:NamedIndividual rdf:about="http://openenergy-platform.org/ontology/oeo/OEO_00000193">
        <rdf:type rdf:resource="http://openenergy-platform.org/ontology/oeo/OEO_00000368"/>
        <oeo:OEO_00040001 rdf:datatype="http://www.w3.org/2001/XMLSchema#string">http://openenergy-platform.org/ontology/oeo/oeo-social</oeo:OEO_00040001>
        <obo:IAO_0000115>Das Schema der Energiebilanzen umfasst eine Matrix von 33 Spalten und 68 Zeilen (einschließlich der Summenspalten und -zeilen). In der horizontalen Gliederung (Spalten) werden die Energieträger ausgewiesen, die der energetischen und nichtenergetischen Nutzung dienen. In der vertikalen Gliederung (Zeilen) werden für die jeweiligen Energieträger Aufkommen, Umwandlung und Verwendung erfasst.

Als Energieträger werden alle Quellen oder Stoffe bezeichnet, in denen Energie mechanisch, thermisch, chemisch oder physikalisch gespeichert ist. Fünf Kerngruppe werden bei der Energiebilanz unterschieden:

    Fossile Brennstoffe
    Erneuerbare Energien
    Strom
    Kernbrennstoffe
    Fernwärme

Bilanzebenen
Schematische Darstellung des Bilanzraums der deutschen Arbeitsgemeinschaft Energiebilanzen
Primär- und Endenergie sowie Umwandlungsverluste

Die Abgrenzung erfolgt in drei Bilanzbereichen:

    die Primärenergiebilanz,
    die Umwandlungsbilanz und
    der Endenergieverbrauch.

In der Primärenergiebilanz werden die Energieträger mit ihrem Mengenaufkommen bei der Gewinnung und Anlieferung nach folgenden Kriterien erfasst:

    inländische Gewinnung von Energieträgern,
    Außenhandel mit Energieträgern, unterteilt nach Einfuhr und Ausfuhr,
    Hochseebunkerungen (Heizöl, Dieselkraftstoff und Schmierstoffe für die nationale und internationale Seeschifffahrt in deutschen Häfen. Ohne Lieferungen an Binnen- und Küstenmotorschiffe und Fischerei, die zum Sektor Verkehr (Endenergieverbrauch) zählen.)
    Bestandsveränderungen, getrennt erfasst nach Bestandsentnahmen und -aufstockungen</obo:IAO_0000115>
        <obo:IAO_0000116>The German Energy Balance is managed by the &apos;AG Energiebilanzen&apos;, where aso the energy balances can be found: https://ag-energiebilanzen.de/</obo:IAO_0000116>
        <obo:IAO_0000119>https://de.wikipedia.org/w/index.php?title=Energiebilanz_(Energiewirtschaft)&amp;oldid=176259115</obo:IAO_0000119>
        <rdfs:label>german energy balances</rdfs:label>
    </owl:NamedIndividual>
    


    <!-- http://openenergy-platform.org/ontology/oeo/OEO_00000242 -->

    <owl:NamedIndividual rdf:about="http://openenergy-platform.org/ontology/oeo/OEO_00000242">
        <rdf:type rdf:resource="http://openenergy-platform.org/ontology/oeo/OEO_00010055"/>
        <oeo:OEO_00000504 rdf:resource="http://openenergy-platform.org/ontology/oeo/OEO_00000242"/>
        <oeo:OEO_00040001 rdf:datatype="http://www.w3.org/2001/XMLSchema#string">http://openenergy-platform.org/ontology/oeo/oeo-social</oeo:OEO_00040001>
        <obo:IAO_0000115>CRF sectors (IPCC 2006) is a version of the common reporting format that was used for national greenhouse gas inventories since the year 2015. It implements the 2006 IPCC Guidelines for National Greenhouse Gas Inventories (with some deviations).</obo:IAO_0000115>
        <obo:IAO_0000233>issue: https://github.com/OpenEnergyPlatform/ontology/issues/461
pull request: https://github.com/OpenEnergyPlatform/ontology/pull/578</obo:IAO_0000233>
        <rdfs:label>CRF sectors (IPCC 2006)</rdfs:label>
    </owl:NamedIndividual>
    


    <!-- http://openenergy-platform.org/ontology/oeo/OEO_00000243 -->

    <owl:NamedIndividual rdf:about="http://openenergy-platform.org/ontology/oeo/OEO_00000243">
        <rdf:type rdf:resource="http://openenergy-platform.org/ontology/oeo/OEO_00010055"/>
        <oeo:OEO_00040001 rdf:datatype="http://www.w3.org/2001/XMLSchema#string">http://openenergy-platform.org/ontology/oeo/oeo-social</oeo:OEO_00040001>
        <obo:IAO_0000115>CRF sectors (IPCC 1996) is a version of the common reporting format that was used for national greenhouse gas inventories until the year 2014. It implements the Revised 1996 IPCC Guidelines for National Greenhouse Gas Inventories (with some deviations).</obo:IAO_0000115>
        <obo:IAO_0000233>issue: https://github.com/OpenEnergyPlatform/ontology/issues/461
pull request: https://github.com/OpenEnergyPlatform/ontology/pull/578</obo:IAO_0000233>
        <rdfs:label>CRF sectors (IPCC 1996)</rdfs:label>
    </owl:NamedIndividual>
    


    <!-- http://openenergy-platform.org/ontology/oeo/OEO_00000291 -->

    <owl:NamedIndividual rdf:about="http://openenergy-platform.org/ontology/oeo/OEO_00000291">
        <rdf:type rdf:resource="http://openenergy-platform.org/ontology/oeo/OEO_00000368"/>
        <oeo:OEO_00040001 rdf:datatype="http://www.w3.org/2001/XMLSchema#string">http://openenergy-platform.org/ontology/oeo/oeo-social</oeo:OEO_00040001>
        <obo:IAO_0000115>The Statistical classification of economic activities in the European Community, abbreviated as NACE, is the classification of economic activities in the European Union (EU); the term NACE is derived from the French Nomenclature statistique des activités économiques dans la Communauté européenne. Various NACE versions have been developed since 1970.

NACE is a four-digit classification providing the framework for collecting and presenting a large range of statistical data according to economic activity in the fields of economic statistics (e.g. production, employment and national accounts) and in other statistical domains developed within the European statistical system (ESS).</obo:IAO_0000115>
        <obo:IAO_0000119>https://ec.europa.eu/eurostat/statistics-explained/index.php?title=Glossary:Statistical_classification_of_economic_activities_in_the_European_Community_(NACE)</obo:IAO_0000119>
        <rdfs:label>nace_ sectors</rdfs:label>
    </owl:NamedIndividual>
    


    <!-- http://openenergy-platform.org/ontology/oeo/OEO_00000355 -->

    <owl:NamedIndividual rdf:about="http://openenergy-platform.org/ontology/oeo/OEO_00000355">
        <rdf:type rdf:resource="http://openenergy-platform.org/ontology/oeo/OEO_00000368"/>
        <oeo:OEO_00040001 rdf:datatype="http://www.w3.org/2001/XMLSchema#string">http://openenergy-platform.org/ontology/oeo/oeo-social</oeo:OEO_00040001>
        <obo:IAO_0000116>The Renewable energy Directive has been revised, but this should have had no impacts on the sectoral definitions. Factsheet on revision: https://ec.europa.eu/energy/sites/ener/files/documents/directive_renewable_factsheet.pdf</obo:IAO_0000116>
        <obo:IAO_0000119>https://eur-lex.europa.eu/legal-content/EN/ALL/?uri=CELEX:32009L0028</obo:IAO_0000119>
        <rdfs:label>renewable_ energy_ directive_ sectors</rdfs:label>
    </owl:NamedIndividual>
    


    <!-- http://openenergy-platform.org/ontology/oeo/OEO_00010038 -->

    <owl:NamedIndividual rdf:about="http://openenergy-platform.org/ontology/oeo/OEO_00010038">
        <rdf:type rdf:resource="http://openenergy-platform.org/ontology/oeo/OEO_00000367"/>
        <oeo:OEO_00000504 rdf:resource="http://openenergy-platform.org/ontology/oeo/OEO_00000242"/>
        <obo:BFO_0000051 rdf:resource="http://openenergy-platform.org/ontology/oeo/OEO_00010040"/>
        <obo:BFO_0000051 rdf:resource="http://openenergy-platform.org/ontology/oeo/OEO_00010041"/>
        <obo:BFO_0000051 rdf:resource="http://openenergy-platform.org/ontology/oeo/OEO_00010042"/>
        <obo:BFO_0000051 rdf:resource="http://openenergy-platform.org/ontology/oeo/OEO_00010043"/>
        <obo:BFO_0000051 rdf:resource="http://openenergy-platform.org/ontology/oeo/OEO_00010044"/>
        <oeo:OEO_00010037>CRF 1</oeo:OEO_00010037>
        <oeo:OEO_00040001 rdf:datatype="http://www.w3.org/2001/XMLSchema#string">http://openenergy-platform.org/ontology/oeo/oeo-social</oeo:OEO_00040001>
        <obo:IAO_0000115>The CRF sector (IPCC 2006) energy is a sector defined by the 2006 IPCC Guidelines for National Greenhouse Gas Inventories:
All GHG emissions arising from combustion and fugitive releases of fuels. Emissions from the non-energy uses of fuels are generally not included here, but reported under Industrial Processes and Product Use.</obo:IAO_0000115>
        <obo:IAO_0000119>2006 IPCC Guidelines for National Greenhouse Gas Inventories, Volume 2, Chapter 2.2, https://www.ipcc-nggip.iges.or.jp/public/2006gl/</obo:IAO_0000119>
        <obo:IAO_0000233>issue: https://github.com/OpenEnergyPlatform/ontology/issues/461
pull request: https://github.com/OpenEnergyPlatform/ontology/pull/523</obo:IAO_0000233>
        <rdfs:label>CRF sector (IPCC 2006): energy</rdfs:label>
    </owl:NamedIndividual>
    


    <!-- http://openenergy-platform.org/ontology/oeo/OEO_00010039 -->

    <owl:NamedIndividual rdf:about="http://openenergy-platform.org/ontology/oeo/OEO_00010039">
        <rdf:type rdf:resource="http://openenergy-platform.org/ontology/oeo/OEO_00000367"/>
        <oeo:OEO_00000504 rdf:resource="http://openenergy-platform.org/ontology/oeo/OEO_00000242"/>
        <obo:BFO_0000050 rdf:resource="http://openenergy-platform.org/ontology/oeo/OEO_00010038"/>
        <oeo:OEO_00010037>CRF 1.A</oeo:OEO_00010037>
        <oeo:OEO_00040001 rdf:datatype="http://www.w3.org/2001/XMLSchema#string">http://openenergy-platform.org/ontology/oeo/oeo-social</oeo:OEO_00040001>
        <obo:IAO_0000115>The CRF sector (IPCC 2006) &apos;fuel combustion&apos; is a sector defined by the 2006 IPCC Guidelines for National Greenhouse Gas Inventories:
Emissions from the intentional oxidation of materials within an apparatus that is designed to raise heat and provide it either as heat or as mechanical work to a process or for use away from the apparatus.</obo:IAO_0000115>
        <obo:IAO_0000119>2006 IPCC Guidelines for National Greenhouse Gas Inventories, Volume 2, Chapter 2.2, https://www.ipcc-nggip.iges.or.jp/public/2006gl/</obo:IAO_0000119>
        <obo:IAO_0000233>issue: https://github.com/OpenEnergyPlatform/ontology/issues/461
pull request: https://github.com/OpenEnergyPlatform/ontology/pull/523</obo:IAO_0000233>
        <rdfs:label>CRF sector (IPCC 2006): fuel combustion</rdfs:label>
    </owl:NamedIndividual>
    


    <!-- http://openenergy-platform.org/ontology/oeo/OEO_00010040 -->

    <owl:NamedIndividual rdf:about="http://openenergy-platform.org/ontology/oeo/OEO_00010040">
        <rdf:type rdf:resource="http://openenergy-platform.org/ontology/oeo/OEO_00000158"/>
        <oeo:OEO_00000504 rdf:resource="http://openenergy-platform.org/ontology/oeo/OEO_00000242"/>
        <obo:BFO_0000050 rdf:resource="http://openenergy-platform.org/ontology/oeo/OEO_00010039"/>
        <obo:BFO_0000051 rdf:resource="http://openenergy-platform.org/ontology/oeo/OEO_00010158"/>
        <obo:BFO_0000051 rdf:resource="http://openenergy-platform.org/ontology/oeo/OEO_00010159"/>
        <obo:BFO_0000051 rdf:resource="http://openenergy-platform.org/ontology/oeo/OEO_00010160"/>
        <oeo:OEO_00010037>CRF 1.A.1</oeo:OEO_00010037>
        <oeo:OEO_00040001 rdf:datatype="http://www.w3.org/2001/XMLSchema#string">http://openenergy-platform.org/ontology/oeo/oeo-social</oeo:OEO_00040001>
        <obo:IAO_0000115>The CRF sector (IPCC 2006) &apos;energy industry&apos; is an energy transformation sector defined by the 2006 IPCC Guidelines for National Greenhouse Gas Inventories:
Comprises emissions from fuels combusted by the fuel extraction or energy-producing industries.</obo:IAO_0000115>
        <obo:IAO_0000119>2006 IPCC Guidelines for National Greenhouse Gas Inventories, Volume 2, Chapter 2.2, https://www.ipcc-nggip.iges.or.jp/public/2006gl/</obo:IAO_0000119>
        <obo:IAO_0000233>issue: https://github.com/OpenEnergyPlatform/ontology/issues/461
pull request: https://github.com/OpenEnergyPlatform/ontology/pull/523

add has part relations:
issue: https://github.com/OpenEnergyPlatform/ontology/issues/858
pull request: https://github.com/OpenEnergyPlatform/ontology/pull/941</obo:IAO_0000233>
        <rdfs:label>CRF sector (IPCC 2006): energy industry</rdfs:label>
    </owl:NamedIndividual>
    


    <!-- http://openenergy-platform.org/ontology/oeo/OEO_00010041 -->

    <owl:NamedIndividual rdf:about="http://openenergy-platform.org/ontology/oeo/OEO_00010041">
        <rdf:type rdf:resource="http://openenergy-platform.org/ontology/oeo/OEO_00000227"/>
        <oeo:OEO_00000504 rdf:resource="http://openenergy-platform.org/ontology/oeo/OEO_00000242"/>
        <obo:BFO_0000050 rdf:resource="http://openenergy-platform.org/ontology/oeo/OEO_00010039"/>
        <oeo:OEO_00010037>CRF 1.A.2</oeo:OEO_00010037>
        <oeo:OEO_00040001 rdf:datatype="http://www.w3.org/2001/XMLSchema#string">http://openenergy-platform.org/ontology/oeo/oeo-social</oeo:OEO_00040001>
        <obo:IAO_0000115>The CRF sector (IPCC 2006) &apos;manufacturing industries and construction&apos; is an industry sector defined by the 2006 IPCC Guidelines for National Greenhouse Gas Inventories:
Emissions from combustion of fuels in industry. Also includes combustion for the generation of electricity and heat for own use in these industries.</obo:IAO_0000115>
        <obo:IAO_0000119>2006 IPCC Guidelines for National Greenhouse Gas Inventories, Volume 2, Chapter 2.2, https://www.ipcc-nggip.iges.or.jp/public/2006gl/</obo:IAO_0000119>
        <obo:IAO_0000233>issue: https://github.com/OpenEnergyPlatform/ontology/issues/461
pull request: https://github.com/OpenEnergyPlatform/ontology/pull/523</obo:IAO_0000233>
        <rdfs:label>CRF sector (IPCC 2006): manufacturing industries and construction</rdfs:label>
    </owl:NamedIndividual>
    


    <!-- http://openenergy-platform.org/ontology/oeo/OEO_00010042 -->

    <owl:NamedIndividual rdf:about="http://openenergy-platform.org/ontology/oeo/OEO_00010042">
        <rdf:type rdf:resource="http://openenergy-platform.org/ontology/oeo/OEO_00000422"/>
        <owl:sameAs rdf:resource="http://openenergy-platform.org/ontology/oeo/OEO_00010306"/>
        <oeo:OEO_00000504 rdf:resource="http://openenergy-platform.org/ontology/oeo/OEO_00000242"/>
        <obo:BFO_0000050 rdf:resource="http://openenergy-platform.org/ontology/oeo/OEO_00010039"/>
        <oeo:OEO_00010037>CRF 1.A.3</oeo:OEO_00010037>
        <oeo:OEO_00040001 rdf:datatype="http://www.w3.org/2001/XMLSchema#string">http://openenergy-platform.org/ontology/oeo/oeo-social</oeo:OEO_00040001>
        <obo:IAO_0000115>The CRF sector (IPCC 2006) &apos;transport&apos; is a transport sector defined by the 2006 IPCC Guidelines for National Greenhouse Gas Inventories:
Emissions from the combustion and evaporation of fuel for all transport activity (excluding military transport), regardless of the sector, specifiedby sub-categories below. Emissions from fuel sold to any air or marine vessel engaged in international transport (1 A 3 a i and 1 A 3 d i) should as far as possible be excluded from the totals and subtotals in this category and should be reported separately.</obo:IAO_0000115>
        <obo:IAO_0000119>2006 IPCC Guidelines for National Greenhouse Gas Inventories, Volume 2, Chapter 3.1, https://www.ipcc-nggip.iges.or.jp/public/2006gl/</obo:IAO_0000119>
        <obo:IAO_0000233>issue: https://github.com/OpenEnergyPlatform/ontology/issues/461
pull request: https://github.com/OpenEnergyPlatform/ontology/pull/523</obo:IAO_0000233>
        <rdfs:label>CRF sector (IPCC 2006): transport</rdfs:label>
    </owl:NamedIndividual>
    


    <!-- http://openenergy-platform.org/ontology/oeo/OEO_00010043 -->

    <owl:NamedIndividual rdf:about="http://openenergy-platform.org/ontology/oeo/OEO_00010043">
        <rdf:type rdf:resource="http://openenergy-platform.org/ontology/oeo/OEO_00000128"/>
        <oeo:OEO_00000504 rdf:resource="http://openenergy-platform.org/ontology/oeo/OEO_00000242"/>
        <obo:BFO_0000050 rdf:resource="http://openenergy-platform.org/ontology/oeo/OEO_00010039"/>
        <obo:BFO_0000051 rdf:resource="http://openenergy-platform.org/ontology/oeo/OEO_00010052"/>
        <obo:BFO_0000051 rdf:resource="http://openenergy-platform.org/ontology/oeo/OEO_00010053"/>
        <oeo:OEO_00010037>CRF 1.A.4</oeo:OEO_00010037>
        <oeo:OEO_00040001 rdf:datatype="http://www.w3.org/2001/XMLSchema#string">http://openenergy-platform.org/ontology/oeo/oeo-social</oeo:OEO_00040001>
        <obo:IAO_0000115>The CRF sector (IPCC 2006) &apos;fuel combustion - other sectors&apos; is an energy demand sector defined by the 2006 IPCC Guidelines for National Greenhouse Gas Inventories:
Emissions from combustion activities as described below, including combustion for the generation of electricity and heat for own use in these sectors.</obo:IAO_0000115>
        <obo:IAO_0000119>2006 IPCC Guidelines for National Greenhouse Gas Inventories, Volume 2, Chapter 2.2, https://www.ipcc-nggip.iges.or.jp/public/2006gl/</obo:IAO_0000119>
        <obo:IAO_0000233>issue: https://github.com/OpenEnergyPlatform/ontology/issues/461
pull request: https://github.com/OpenEnergyPlatform/ontology/pull/523</obo:IAO_0000233>
        <rdfs:label>CRF sector (IPCC 2006): fuel combustion - other sectors</rdfs:label>
    </owl:NamedIndividual>
    


    <!-- http://openenergy-platform.org/ontology/oeo/OEO_00010044 -->

    <owl:NamedIndividual rdf:about="http://openenergy-platform.org/ontology/oeo/OEO_00010044">
        <rdf:type rdf:resource="http://openenergy-platform.org/ontology/oeo/OEO_00000367"/>
        <oeo:OEO_00000504 rdf:resource="http://openenergy-platform.org/ontology/oeo/OEO_00000242"/>
        <obo:BFO_0000050 rdf:resource="http://openenergy-platform.org/ontology/oeo/OEO_00010039"/>
        <oeo:OEO_00010037>CRF 1.A.5</oeo:OEO_00010037>
        <oeo:OEO_00040001 rdf:datatype="http://www.w3.org/2001/XMLSchema#string">http://openenergy-platform.org/ontology/oeo/oeo-social</oeo:OEO_00040001>
        <obo:IAO_0000115>The CRF sector (IPCC 2006) &apos;fuel combustion&apos; is a sector defined by the 2006 IPCC Guidelines for National Greenhouse Gas Inventories:
All remaining emissions from fuel combustion that are not specified elsewhere. Include emissions from fuel delivered to the military in the country and delivered to the military of other countries that are not engaged in multilateral operations.</obo:IAO_0000115>
        <obo:IAO_0000119>2006 IPCC Guidelines for National Greenhouse Gas Inventories, Volume 2, Chapter 2.2, https://www.ipcc-nggip.iges.or.jp/public/2006gl/</obo:IAO_0000119>
        <obo:IAO_0000233>issue: https://github.com/OpenEnergyPlatform/ontology/issues/461
pull request: https://github.com/OpenEnergyPlatform/ontology/pull/523</obo:IAO_0000233>
        <rdfs:label>CRF sector (IPCC 2006): fuel combustion - other</rdfs:label>
    </owl:NamedIndividual>
    


    <!-- http://openenergy-platform.org/ontology/oeo/OEO_00010046 -->

    <owl:NamedIndividual rdf:about="http://openenergy-platform.org/ontology/oeo/OEO_00010046">
        <rdf:type rdf:resource="http://openenergy-platform.org/ontology/oeo/OEO_00000227"/>
        <oeo:OEO_00000504 rdf:resource="http://openenergy-platform.org/ontology/oeo/OEO_00000242"/>
        <obo:BFO_0000051 rdf:resource="http://openenergy-platform.org/ontology/oeo/OEO_00010164"/>
        <obo:BFO_0000051 rdf:resource="http://openenergy-platform.org/ontology/oeo/OEO_00010166"/>
        <obo:BFO_0000051 rdf:resource="http://openenergy-platform.org/ontology/oeo/OEO_00010167"/>
        <obo:BFO_0000051 rdf:resource="http://openenergy-platform.org/ontology/oeo/OEO_00010169"/>
        <obo:BFO_0000051 rdf:resource="http://openenergy-platform.org/ontology/oeo/OEO_00010170"/>
        <obo:BFO_0000051 rdf:resource="http://openenergy-platform.org/ontology/oeo/OEO_00010171"/>
        <obo:BFO_0000051 rdf:resource="http://openenergy-platform.org/ontology/oeo/OEO_00010172"/>
        <obo:BFO_0000051 rdf:resource="http://openenergy-platform.org/ontology/oeo/OEO_00010173"/>
        <oeo:OEO_00010037>CRF 2</oeo:OEO_00010037>
        <oeo:OEO_00040001 rdf:datatype="http://www.w3.org/2001/XMLSchema#string">http://openenergy-platform.org/ontology/oeo/oeo-social</oeo:OEO_00040001>
        <obo:IAO_0000115>The CRF sector (IPCC 2006) &apos;energy industrial processes and product use&apos; (IPPU) is an industry sector defined by the 2006 IPCC Guidelines for National Greenhouse Gas Inventories:
It covers greenhouse gas emissions occurring from industrial processes, from the use of greenhouse gases in products, and from non-energy uses of fossil fuel carbon.</obo:IAO_0000115>
        <obo:IAO_0000118>IPPU</obo:IAO_0000118>
        <obo:IAO_0000119>2006 IPCC Guidelines for National Greenhouse Gas Inventories, Volume 3, Chapter 1.1, https://www.ipcc-nggip.iges.or.jp/public/2006gl/</obo:IAO_0000119>
        <obo:IAO_0000233>issue: https://github.com/OpenEnergyPlatform/ontology/issues/461
pull request: https://github.com/OpenEnergyPlatform/ontology/pull/578

add has part relations:
issue: https://github.com/OpenEnergyPlatform/ontology/issues/858
pull request: https://github.com/OpenEnergyPlatform/ontology/pull/941</obo:IAO_0000233>
        <rdfs:label>CRF sector (IPCC 2006): industrial processes and product use</rdfs:label>
    </owl:NamedIndividual>
    


    <!-- http://openenergy-platform.org/ontology/oeo/OEO_00010047 -->

    <owl:NamedIndividual rdf:about="http://openenergy-platform.org/ontology/oeo/OEO_00010047">
        <rdf:type rdf:resource="http://openenergy-platform.org/ontology/oeo/OEO_00010035"/>
        <owl:sameAs rdf:resource="http://openenergy-platform.org/ontology/oeo/OEO_00010308"/>
        <oeo:OEO_00000504 rdf:resource="http://openenergy-platform.org/ontology/oeo/OEO_00000242"/>
        <obo:BFO_0000051 rdf:resource="http://openenergy-platform.org/ontology/oeo/OEO_00010179"/>
        <obo:BFO_0000051 rdf:resource="http://openenergy-platform.org/ontology/oeo/OEO_00010180"/>
        <obo:BFO_0000051 rdf:resource="http://openenergy-platform.org/ontology/oeo/OEO_00010181"/>
        <obo:BFO_0000051 rdf:resource="http://openenergy-platform.org/ontology/oeo/OEO_00010182"/>
        <obo:BFO_0000051 rdf:resource="http://openenergy-platform.org/ontology/oeo/OEO_00010183"/>
        <obo:BFO_0000051 rdf:resource="http://openenergy-platform.org/ontology/oeo/OEO_00010184"/>
        <obo:BFO_0000051 rdf:resource="http://openenergy-platform.org/ontology/oeo/OEO_00010185"/>
        <obo:BFO_0000051 rdf:resource="http://openenergy-platform.org/ontology/oeo/OEO_00010186"/>
        <obo:BFO_0000051 rdf:resource="http://openenergy-platform.org/ontology/oeo/OEO_00010187"/>
        <obo:BFO_0000051 rdf:resource="http://openenergy-platform.org/ontology/oeo/OEO_00010188"/>
        <oeo:OEO_00010037>CRF 3</oeo:OEO_00010037>
        <oeo:OEO_00040001 rdf:datatype="http://www.w3.org/2001/XMLSchema#string">http://openenergy-platform.org/ontology/oeo/oeo-social</oeo:OEO_00040001>
        <obo:IAO_0000233>issue: https://github.com/OpenEnergyPlatform/ontology/issues/461
pull request: https://github.com/OpenEnergyPlatform/ontology/pull/578

add has part axioms:
issue: https://github.com/OpenEnergyPlatform/ontology/issues/858
pull request: https://github.com/OpenEnergyPlatform/ontology/pull/941</obo:IAO_0000233>
        <rdfs:comment>The CRF sector (IPCC 2006) &apos;agriculture&apos; is an agriculture, forestry and land use sector defined by the 2006 IPCC Guidelines for National Greenhouse Gas Inventories</rdfs:comment>
        <rdfs:label>CRF sector (IPCC 2006): agriculture</rdfs:label>
    </owl:NamedIndividual>
    


    <!-- http://openenergy-platform.org/ontology/oeo/OEO_00010048 -->

    <owl:NamedIndividual rdf:about="http://openenergy-platform.org/ontology/oeo/OEO_00010048">
        <rdf:type rdf:resource="http://openenergy-platform.org/ontology/oeo/OEO_00010035"/>
        <owl:sameAs rdf:resource="http://openenergy-platform.org/ontology/oeo/OEO_00010071"/>
        <owl:sameAs rdf:resource="http://openenergy-platform.org/ontology/oeo/OEO_00010135"/>
        <owl:sameAs rdf:resource="http://openenergy-platform.org/ontology/oeo/OEO_00010309"/>
        <oeo:OEO_00000504 rdf:resource="http://openenergy-platform.org/ontology/oeo/OEO_00000242"/>
        <obo:BFO_0000051 rdf:resource="http://openenergy-platform.org/ontology/oeo/OEO_00010189"/>
        <obo:BFO_0000051 rdf:resource="http://openenergy-platform.org/ontology/oeo/OEO_00010190"/>
        <obo:BFO_0000051 rdf:resource="http://openenergy-platform.org/ontology/oeo/OEO_00010192"/>
        <obo:BFO_0000051 rdf:resource="http://openenergy-platform.org/ontology/oeo/OEO_00010193"/>
        <obo:BFO_0000051 rdf:resource="http://openenergy-platform.org/ontology/oeo/OEO_00010194"/>
        <obo:BFO_0000051 rdf:resource="http://openenergy-platform.org/ontology/oeo/OEO_00010195"/>
        <obo:BFO_0000051 rdf:resource="http://openenergy-platform.org/ontology/oeo/OEO_00010196"/>
        <oeo:OEO_00010037>CRF 4</oeo:OEO_00010037>
        <oeo:OEO_00040001 rdf:datatype="http://www.w3.org/2001/XMLSchema#string">http://openenergy-platform.org/ontology/oeo/oeo-social</oeo:OEO_00040001>
        <obo:IAO_0000115>The CRF sector (IPCC 2006) &apos;land use, land-use change and forestry&apos; (LULUCF) is an agriculture, forestry and land use sector defined by the 2006 IPCC Guidelines for National Greenhouse Gas Inventories</obo:IAO_0000115>
        <obo:IAO_0000118>LULUCF</obo:IAO_0000118>
        <obo:IAO_0000233>issue: https://github.com/OpenEnergyPlatform/ontology/issues/461
pull request: https://github.com/OpenEnergyPlatform/ontology/pull/578

add has part axioms:
issue: https://github.com/OpenEnergyPlatform/ontology/issues/858
pull request: https://github.com/OpenEnergyPlatform/ontology/pull/941</obo:IAO_0000233>
        <rdfs:label>CRF sector (IPCC 2006): land use, land-use change and forestry</rdfs:label>
    </owl:NamedIndividual>
    


    <!-- http://openenergy-platform.org/ontology/oeo/OEO_00010049 -->

    <owl:NamedIndividual rdf:about="http://openenergy-platform.org/ontology/oeo/OEO_00010049">
        <rdf:type rdf:resource="http://openenergy-platform.org/ontology/oeo/OEO_00010036"/>
        <owl:sameAs rdf:resource="http://openenergy-platform.org/ontology/oeo/OEO_00010310"/>
        <oeo:OEO_00000504 rdf:resource="http://openenergy-platform.org/ontology/oeo/OEO_00000242"/>
        <obo:BFO_0000051 rdf:resource="http://openenergy-platform.org/ontology/oeo/OEO_00010174"/>
        <obo:BFO_0000051 rdf:resource="http://openenergy-platform.org/ontology/oeo/OEO_00010175"/>
        <obo:BFO_0000051 rdf:resource="http://openenergy-platform.org/ontology/oeo/OEO_00010176"/>
        <obo:BFO_0000051 rdf:resource="http://openenergy-platform.org/ontology/oeo/OEO_00010177"/>
        <obo:BFO_0000051 rdf:resource="http://openenergy-platform.org/ontology/oeo/OEO_00010178"/>
        <oeo:OEO_00010037>CRF 5</oeo:OEO_00010037>
        <oeo:OEO_00040001 rdf:datatype="http://www.w3.org/2001/XMLSchema#string">http://openenergy-platform.org/ontology/oeo/oeo-social</oeo:OEO_00040001>
        <obo:IAO_0000115>The CRF sector (IPCC 2006) &apos;waste&apos; is a waste and wastewater sector defined by the 2006 IPCC Guidelines for National Greenhouse Gas Inventories:
Carbon dioxide (CO2), methane (CH4) and nitrous oxide (N2O) emissions from following categories: Solid waste disposal, Biological treatment of solid waste,
Incineration and open burning of waste, Wastewater treatment and discharge.</obo:IAO_0000115>
        <obo:IAO_0000119>2006 IPCC Guidelines for National Greenhouse Gas Inventories, Volume 5, Chapter 1.1, https://www.ipcc-nggip.iges.or.jp/public/2006gl/</obo:IAO_0000119>
        <obo:IAO_0000233>issue: https://github.com/OpenEnergyPlatform/ontology/issues/461
pull request: https://github.com/OpenEnergyPlatform/ontology/pull/578

add has part axioms and improve definition:
issue: https://github.com/OpenEnergyPlatform/ontology/issues/858
pull request: https://github.com/OpenEnergyPlatform/ontology/pull/941</obo:IAO_0000233>
        <rdfs:label>CRF sector (IPCC 2006): waste</rdfs:label>
    </owl:NamedIndividual>
    


    <!-- http://openenergy-platform.org/ontology/oeo/OEO_00010050 -->

    <owl:NamedIndividual rdf:about="http://openenergy-platform.org/ontology/oeo/OEO_00010050">
        <rdf:type rdf:resource="http://openenergy-platform.org/ontology/oeo/OEO_00000367"/>
        <owl:sameAs rdf:resource="http://openenergy-platform.org/ontology/oeo/OEO_00010311"/>
        <oeo:OEO_00000504 rdf:resource="http://openenergy-platform.org/ontology/oeo/OEO_00000242"/>
        <oeo:OEO_00010037>CRF 6</oeo:OEO_00010037>
        <oeo:OEO_00040001 rdf:datatype="http://www.w3.org/2001/XMLSchema#string">http://openenergy-platform.org/ontology/oeo/oeo-social</oeo:OEO_00040001>
        <obo:IAO_0000115>The CRF sector (IPCC 2006) &apos;other&apos; is a sector defined by the 2006 IPCC Guidelines for National Greenhouse Gas Inventories</obo:IAO_0000115>
        <obo:IAO_0000233>issue: https://github.com/OpenEnergyPlatform/ontology/issues/461
pull request: https://github.com/OpenEnergyPlatform/ontology/pull/578</obo:IAO_0000233>
        <rdfs:label>CRF sector (IPCC 2006): other</rdfs:label>
    </owl:NamedIndividual>
    


    <!-- http://openenergy-platform.org/ontology/oeo/OEO_00010052 -->

    <owl:NamedIndividual rdf:about="http://openenergy-platform.org/ontology/oeo/OEO_00010052">
        <rdf:type rdf:resource="http://openenergy-platform.org/ontology/oeo/OEO_00000405"/>
        <oeo:OEO_00000504 rdf:resource="http://openenergy-platform.org/ontology/oeo/OEO_00000242"/>
        <obo:BFO_0000050 rdf:resource="http://openenergy-platform.org/ontology/oeo/OEO_00010043"/>
        <oeo:OEO_00010037>CRF 1.A.4.a</oeo:OEO_00010037>
        <oeo:OEO_00040001 rdf:datatype="http://www.w3.org/2001/XMLSchema#string">http://openenergy-platform.org/ontology/oeo/oeo-social</oeo:OEO_00040001>
        <obo:IAO_0000115>The CRF sector (IPCC 2006) &apos;commercial and institutional&apos; is a commercial sector defined by the 2006 IPCC Guidelines for National Greenhouse Gas Inventories:
Emissions from fuel combustion in commercial and institutional buildings.</obo:IAO_0000115>
        <obo:IAO_0000119>2006 IPCC Guidelines for National Greenhouse Gas Inventories, Volume 3, Chapter 1.1, https://www.ipcc-nggip.iges.or.jp/public/2006gl/</obo:IAO_0000119>
        <obo:IAO_0000233>issue: https://github.com/OpenEnergyPlatform/ontology/issues/461
pull request: https://github.com/OpenEnergyPlatform/ontology/pull/578</obo:IAO_0000233>
        <rdfs:label>CRF sector (IPCC 2006): commercial and institutional</rdfs:label>
    </owl:NamedIndividual>
    


    <!-- http://openenergy-platform.org/ontology/oeo/OEO_00010053 -->

    <owl:NamedIndividual rdf:about="http://openenergy-platform.org/ontology/oeo/OEO_00010053">
        <rdf:type rdf:resource="http://openenergy-platform.org/ontology/oeo/OEO_00000214"/>
        <oeo:OEO_00000504 rdf:resource="http://openenergy-platform.org/ontology/oeo/OEO_00000242"/>
        <obo:BFO_0000050 rdf:resource="http://openenergy-platform.org/ontology/oeo/OEO_00010043"/>
        <oeo:OEO_00010037>CRF 1.A.4.b</oeo:OEO_00010037>
        <oeo:OEO_00040001 rdf:datatype="http://www.w3.org/2001/XMLSchema#string">http://openenergy-platform.org/ontology/oeo/oeo-social</oeo:OEO_00040001>
        <obo:IAO_0000115>The CRF sector (IPCC 2006) &apos;residential&apos; is a household sector defined by the 2006 IPCC Guidelines for National Greenhouse Gas Inventories:
All emissions from fuel combustion in households.</obo:IAO_0000115>
        <obo:IAO_0000119>2006 IPCC Guidelines for National Greenhouse Gas Inventories, Volume 2, Chapter 2.2, https://www.ipcc-nggip.iges.or.jp/public/2006gl/</obo:IAO_0000119>
        <obo:IAO_0000233>issue: https://github.com/OpenEnergyPlatform/ontology/issues/461
pull request: https://github.com/OpenEnergyPlatform/ontology/pull/578</obo:IAO_0000233>
        <rdfs:label>CRF sector (IPCC 2006): residential</rdfs:label>
    </owl:NamedIndividual>
    


    <!-- http://openenergy-platform.org/ontology/oeo/OEO_00010054 -->

    <owl:NamedIndividual rdf:about="http://openenergy-platform.org/ontology/oeo/OEO_00010054">
        <rdf:type rdf:resource="http://openenergy-platform.org/ontology/oeo/OEO_00000128"/>
        <oeo:OEO_00000504 rdf:resource="http://openenergy-platform.org/ontology/oeo/OEO_00000242"/>
        <obo:BFO_0000050 rdf:resource="http://openenergy-platform.org/ontology/oeo/OEO_00010043"/>
        <oeo:OEO_00010037>CRF 1.A.4.c</oeo:OEO_00010037>
        <oeo:OEO_00040001 rdf:datatype="http://www.w3.org/2001/XMLSchema#string">http://openenergy-platform.org/ontology/oeo/oeo-social</oeo:OEO_00040001>
        <obo:IAO_0000115>The CRF sector (IPCC 2006) &apos;agriculture, forestry and fishing&apos; is an energy demand sector defined by the 2006 IPCC Guidelines for National Greenhouse Gas Inventories:
Emissions from fuel combustion in agriculture, forestry, fishing and fishing industries such as fish farms.</obo:IAO_0000115>
        <obo:IAO_0000119>2006 IPCC Guidelines for National Greenhouse Gas Inventories, Volume 2, Chapter 2.2, https://www.ipcc-nggip.iges.or.jp/public/2006gl/</obo:IAO_0000119>
        <obo:IAO_0000233>issue: https://github.com/OpenEnergyPlatform/ontology/issues/461
pull request: https://github.com/OpenEnergyPlatform/ontology/pull/578</obo:IAO_0000233>
        <rdfs:label>CRF sector (IPCC 2006): agriculture, forestry and fishing</rdfs:label>
    </owl:NamedIndividual>
    


    <!-- http://openenergy-platform.org/ontology/oeo/OEO_00010056 -->

    <owl:NamedIndividual rdf:about="http://openenergy-platform.org/ontology/oeo/OEO_00010056">
        <rdf:type rdf:resource="http://openenergy-platform.org/ontology/oeo/OEO_00000368"/>
        <oeo:OEO_00040001 rdf:datatype="http://www.w3.org/2001/XMLSchema#string">http://openenergy-platform.org/ontology/oeo/oeo-social</oeo:OEO_00040001>
        <obo:IAO_0000115>The KSG sector division is a sector division defined in annex 1 of the Bundes-Klimaschutzgesetz (KSG).</obo:IAO_0000115>
        <obo:IAO_0000233>issue: https://github.com/OpenEnergyPlatform/ontology/issues/580
pull request: https://github.com/OpenEnergyPlatform/ontology/pull/595</obo:IAO_0000233>
        <rdfs:label>KSG sector division</rdfs:label>
    </owl:NamedIndividual>
    


    <!-- http://openenergy-platform.org/ontology/oeo/OEO_00010057 -->

    <owl:NamedIndividual rdf:about="http://openenergy-platform.org/ontology/oeo/OEO_00010057">
        <rdf:type rdf:resource="http://openenergy-platform.org/ontology/oeo/OEO_00000367"/>
        <oeo:OEO_00000504 rdf:resource="http://openenergy-platform.org/ontology/oeo/OEO_00000242"/>
        <obo:BFO_0000050 rdf:resource="http://openenergy-platform.org/ontology/oeo/OEO_00010038"/>
        <obo:BFO_0000051 rdf:resource="http://openenergy-platform.org/ontology/oeo/OEO_00010161"/>
        <obo:BFO_0000051 rdf:resource="http://openenergy-platform.org/ontology/oeo/OEO_00010162"/>
        <oeo:OEO_00010037>CRF 1.B</oeo:OEO_00010037>
        <oeo:OEO_00040001 rdf:datatype="http://www.w3.org/2001/XMLSchema#string">http://openenergy-platform.org/ontology/oeo/oeo-social</oeo:OEO_00040001>
        <obo:IAO_0000115>The CRF sector (IPCC 2006) &apos;fugitive emissions from fuels&apos; is a sector defined by the 2006 IPCC Guidelines for National Greenhouse Gas Inventories:
Includes all intentional and unintentional emissions from the extraction, processing, storage and transport of solid fuel to the point of final use.</obo:IAO_0000115>
        <obo:IAO_0000119>2006 IPCC Guidelines for National Greenhouse Gas Inventories, Volume 1, Chapter 8.5, https://www.ipcc-nggip.iges.or.jp/public/2006gl/</obo:IAO_0000119>
        <obo:IAO_0000233>issue: https://github.com/OpenEnergyPlatform/ontology/issues/580
pull request: https://github.com/OpenEnergyPlatform/ontology/pull/595</obo:IAO_0000233>
        <rdfs:label>CRF sector (IPCC 2006): fugitive emissions from fuels</rdfs:label>
    </owl:NamedIndividual>
    


    <!-- http://openenergy-platform.org/ontology/oeo/OEO_00010058 -->

    <owl:NamedIndividual rdf:about="http://openenergy-platform.org/ontology/oeo/OEO_00010058">
        <rdf:type rdf:resource="http://openenergy-platform.org/ontology/oeo/OEO_00000367"/>
        <oeo:OEO_00000504 rdf:resource="http://openenergy-platform.org/ontology/oeo/OEO_00000242"/>
        <obo:BFO_0000050 rdf:resource="http://openenergy-platform.org/ontology/oeo/OEO_00010038"/>
        <oeo:OEO_00010037>CRF 1.C</oeo:OEO_00010037>
        <oeo:OEO_00040001 rdf:datatype="http://www.w3.org/2001/XMLSchema#string">http://openenergy-platform.org/ontology/oeo/oeo-social</oeo:OEO_00040001>
        <obo:IAO_0000115>The CRF sector (IPCC 2006) &apos;CO2 transport and storage&apos; is a sector defined by the 2006 IPCC Guidelines for National Greenhouse Gas Inventories:
Carbon dioxide (CO2) capture and storage (CCS) involves the capture of CO2 from anthropogenic sources, its transport to a storage location and its long-term isolation from the atmosphere. Emissions associated with CO2 transport, injection and storage are covered under category 1C. Emissions (and reductions) associated with CO2 capture should be reported under the IPCC Sector in which capture takes place (e.g. Fuel Combustion or Industrial Activities).</obo:IAO_0000115>
        <obo:IAO_0000119>2006 IPCC Guidelines for National Greenhouse Gas Inventories, Volume 1, Chapter 8.5, https://www.ipcc-nggip.iges.or.jp/public/2006gl/</obo:IAO_0000119>
        <obo:IAO_0000233>issue: https://github.com/OpenEnergyPlatform/ontology/issues/580
pull request: https://github.com/OpenEnergyPlatform/ontology/pull/595</obo:IAO_0000233>
        <rdfs:label>CRF sector (IPCC 2006): CO2 transport and storage</rdfs:label>
    </owl:NamedIndividual>
    


    <!-- http://openenergy-platform.org/ontology/oeo/OEO_00010059 -->

    <owl:NamedIndividual rdf:about="http://openenergy-platform.org/ontology/oeo/OEO_00010059">
        <rdf:type rdf:resource="http://openenergy-platform.org/ontology/oeo/OEO_00000422"/>
        <oeo:OEO_00000504 rdf:resource="http://openenergy-platform.org/ontology/oeo/OEO_00000242"/>
        <obo:BFO_0000050 rdf:resource="http://openenergy-platform.org/ontology/oeo/OEO_00010042"/>
        <oeo:OEO_00010037>CRF 1.A.3.a</oeo:OEO_00010037>
        <oeo:OEO_00040001 rdf:datatype="http://www.w3.org/2001/XMLSchema#string">http://openenergy-platform.org/ontology/oeo/oeo-social</oeo:OEO_00040001>
        <obo:IAO_0000115>The CRF sector (IPCC 2006) &apos;domestic aviation&apos; is a transport sector defined by the 2006 IPCC Guidelines for National Greenhouse Gas Inventories:
Emissions from civil domestic passenger and freight traffic that departs and arrives in the same country (commercial, private, agriculture, etc.), including take-offs and landings for these flight stages. Note that this may include journeys of considerable length between two airports in a country (e.g. San Francisco to Honolulu). Exclude military, which should be reported under 1 A 5 b.</obo:IAO_0000115>
        <obo:IAO_0000119>2006 IPCC Guidelines for National Greenhouse Gas Inventories, Volume 1, Chapter 8.5, https://www.ipcc-nggip.iges.or.jp/public/2006gl/</obo:IAO_0000119>
        <obo:IAO_0000233>issue: https://github.com/OpenEnergyPlatform/ontology/issues/580
pull request: https://github.com/OpenEnergyPlatform/ontology/pull/595</obo:IAO_0000233>
        <rdfs:label>CRF sector (IPCC 2006): domestic aviation</rdfs:label>
    </owl:NamedIndividual>
    


    <!-- http://openenergy-platform.org/ontology/oeo/OEO_00010060 -->

    <owl:NamedIndividual rdf:about="http://openenergy-platform.org/ontology/oeo/OEO_00010060">
        <rdf:type rdf:resource="http://openenergy-platform.org/ontology/oeo/OEO_00000422"/>
        <oeo:OEO_00000504 rdf:resource="http://openenergy-platform.org/ontology/oeo/OEO_00000242"/>
        <obo:BFO_0000050 rdf:resource="http://openenergy-platform.org/ontology/oeo/OEO_00010042"/>
        <oeo:OEO_00010037>CRF 1.A.3.b</oeo:OEO_00010037>
        <oeo:OEO_00040001 rdf:datatype="http://www.w3.org/2001/XMLSchema#string">http://openenergy-platform.org/ontology/oeo/oeo-social</oeo:OEO_00040001>
        <obo:IAO_0000115>The CRF sector (IPCC 2006) &apos;road transport&apos; is a transport sector defined by the 2006 IPCC Guidelines for National Greenhouse Gas Inventories:
All combustion and evaporative emissions arising from fuel use in road vehicles, including the use of agricultural vehicles on paved roads.</obo:IAO_0000115>
        <obo:IAO_0000119>2006 IPCC Guidelines for National Greenhouse Gas Inventories, Volume 1, Chapter 8.5, https://www.ipcc-nggip.iges.or.jp/public/2006gl/</obo:IAO_0000119>
        <obo:IAO_0000233>issue: https://github.com/OpenEnergyPlatform/ontology/issues/580
pull request: https://github.com/OpenEnergyPlatform/ontology/pull/595</obo:IAO_0000233>
        <rdfs:label>CRF sector (IPCC 2006): road transportation</rdfs:label>
    </owl:NamedIndividual>
    


    <!-- http://openenergy-platform.org/ontology/oeo/OEO_00010061 -->

    <owl:NamedIndividual rdf:about="http://openenergy-platform.org/ontology/oeo/OEO_00010061">
        <rdf:type rdf:resource="http://openenergy-platform.org/ontology/oeo/OEO_00000422"/>
        <oeo:OEO_00000504 rdf:resource="http://openenergy-platform.org/ontology/oeo/OEO_00000242"/>
        <obo:BFO_0000050 rdf:resource="http://openenergy-platform.org/ontology/oeo/OEO_00010042"/>
        <oeo:OEO_00010037>CRF 1.A.3.c</oeo:OEO_00010037>
        <oeo:OEO_00040001 rdf:datatype="http://www.w3.org/2001/XMLSchema#string">http://openenergy-platform.org/ontology/oeo/oeo-social</oeo:OEO_00040001>
        <obo:IAO_0000115>2006 IPCC Guidelines for National Greenhouse Gas Inventories, Volume 1, Chapter 8.5, https://www.ipcc-nggip.iges.or.jp/public/2006gl/</obo:IAO_0000115>
        <obo:IAO_0000115>The CRF sector (IPCC 2006) &apos;railways&apos; is a transport sector defined by the 2006 IPCC Guidelines for National Greenhouse Gas Inventories:
Emissions from railway transport for both freight and passenger traffic routes.</obo:IAO_0000115>
        <obo:IAO_0000115>issue: https://github.com/OpenEnergyPlatform/ontology/issues/580
pull request: https://github.com/OpenEnergyPlatform/ontology/pull/595</obo:IAO_0000115>
        <rdfs:label>CRF sector (IPCC 2006): railways</rdfs:label>
    </owl:NamedIndividual>
    


    <!-- http://openenergy-platform.org/ontology/oeo/OEO_00010062 -->

    <owl:NamedIndividual rdf:about="http://openenergy-platform.org/ontology/oeo/OEO_00010062">
        <rdf:type rdf:resource="http://openenergy-platform.org/ontology/oeo/OEO_00000422"/>
        <oeo:OEO_00000504 rdf:resource="http://openenergy-platform.org/ontology/oeo/OEO_00000242"/>
        <obo:BFO_0000050 rdf:resource="http://openenergy-platform.org/ontology/oeo/OEO_00010042"/>
        <oeo:OEO_00010037>CRF 1.A.3.d</oeo:OEO_00010037>
        <oeo:OEO_00040001 rdf:datatype="http://www.w3.org/2001/XMLSchema#string">http://openenergy-platform.org/ontology/oeo/oeo-social</oeo:OEO_00040001>
        <obo:IAO_0000115>The CRF sector (IPCC 2006) &apos;domestic navigation&apos; is a transport sector defined by the 2006 IPCC Guidelines for National Greenhouse Gas Inventories:
Emissions from fuels used by vessels of all flags that depart and arrive in the same country (exclude fishing, which should be reported under 1 A 4 c iii, and military, which should be reported under 1 A 5 b). Note that this may include journeys of considerable length between two ports in a country (e.g. San Francisco to Honolulu).</obo:IAO_0000115>
        <obo:IAO_0000119>2006 IPCC Guidelines for National Greenhouse Gas Inventories, Volume 1, Chapter 8.5, https://www.ipcc-nggip.iges.or.jp/public/2006gl/</obo:IAO_0000119>
        <obo:IAO_0000233>issue: https://github.com/OpenEnergyPlatform/ontology/issues/580
pull request: https://github.com/OpenEnergyPlatform/ontology/pull/595</obo:IAO_0000233>
        <rdfs:label>CRF sector (IPCC 2006): domestic navigation</rdfs:label>
    </owl:NamedIndividual>
    


    <!-- http://openenergy-platform.org/ontology/oeo/OEO_00010063 -->

    <owl:NamedIndividual rdf:about="http://openenergy-platform.org/ontology/oeo/OEO_00010063">
        <rdf:type rdf:resource="http://openenergy-platform.org/ontology/oeo/OEO_00000422"/>
        <oeo:OEO_00000504 rdf:resource="http://openenergy-platform.org/ontology/oeo/OEO_00000242"/>
        <obo:BFO_0000050 rdf:resource="http://openenergy-platform.org/ontology/oeo/OEO_00010042"/>
        <oeo:OEO_00010037>CRF 1.A.3.e</oeo:OEO_00010037>
        <oeo:OEO_00040001 rdf:datatype="http://www.w3.org/2001/XMLSchema#string">http://openenergy-platform.org/ontology/oeo/oeo-social</oeo:OEO_00040001>
        <obo:IAO_0000115>The CRF sector (IPCC 2006) &apos;other transportation&apos; is a transport sector defined by the 2006 IPCC Guidelines for National Greenhouse Gas Inventories:
Combustion emissions from all remaining transport activities including pipeline transportation, ground activities in airports and harbours, and off-road activities not otherwise reported under 1 A 4 c Agriculture or 1 A 2. Manufacturing Industries and Construction. Military transport should be reported under 1 A 5.</obo:IAO_0000115>
        <obo:IAO_0000119>2006 IPCC Guidelines for National Greenhouse Gas Inventories, Volume 1, Chapter 8.5, https://www.ipcc-nggip.iges.or.jp/public/2006gl/</obo:IAO_0000119>
        <obo:IAO_0000233>issue: https://github.com/OpenEnergyPlatform/ontology/issues/580
pull request: https://github.com/OpenEnergyPlatform/ontology/pull/595</obo:IAO_0000233>
        <rdfs:label>CRF sector (IPCC 2006): other transportation</rdfs:label>
    </owl:NamedIndividual>
    


    <!-- http://openenergy-platform.org/ontology/oeo/OEO_00010064 -->

    <owl:NamedIndividual rdf:about="http://openenergy-platform.org/ontology/oeo/OEO_00010064">
        <rdf:type rdf:resource="http://openenergy-platform.org/ontology/oeo/OEO_00000422"/>
        <oeo:OEO_00000504 rdf:resource="http://openenergy-platform.org/ontology/oeo/OEO_00000242"/>
        <obo:BFO_0000050 rdf:resource="http://openenergy-platform.org/ontology/oeo/OEO_00010063"/>
        <oeo:OEO_00010037>CRF 1.A.3.e.i</oeo:OEO_00010037>
        <oeo:OEO_00040001 rdf:datatype="http://www.w3.org/2001/XMLSchema#string">http://openenergy-platform.org/ontology/oeo/oeo-social</oeo:OEO_00040001>
        <obo:IAO_0000115>The CRF sector (IPCC 2006) &apos;pipeline transport&apos; is a transport sector defined by the 2006 IPCC Guidelines for National Greenhouse Gas Inventories:
Combustion related emissions from the operation of pump stations and maintenance of pipelines. Transport via pipelines includes transport of gases  liquids, slurry and other commodities via pipelines. Distribution of natural or manufactured gas, water or steam from the distributor to final users is excluded and should be reported in 1 A 1 c ii or 1 A 4 a.</obo:IAO_0000115>
        <obo:IAO_0000119>2006 IPCC Guidelines for National Greenhouse Gas Inventories, Volume 1, Chapter 8.5, https://www.ipcc-nggip.iges.or.jp/public/2006gl/</obo:IAO_0000119>
        <obo:IAO_0000233>issue: https://github.com/OpenEnergyPlatform/ontology/issues/580
pull request: https://github.com/OpenEnergyPlatform/ontology/pull/595

fix unique individual identfier
issue: https://github.com/OpenEnergyPlatform/ontology/issues/1121
pull request: https://github.com/OpenEnergyPlatform/ontology/pull/1122</obo:IAO_0000233>
        <rdfs:label>CRF sector (IPCC 2006): pipeline transport</rdfs:label>
    </owl:NamedIndividual>
    


    <!-- http://openenergy-platform.org/ontology/oeo/OEO_00010065 -->

    <owl:NamedIndividual rdf:about="http://openenergy-platform.org/ontology/oeo/OEO_00010065">
        <rdf:type rdf:resource="http://openenergy-platform.org/ontology/oeo/OEO_00000158"/>
        <oeo:OEO_00000504 rdf:resource="http://openenergy-platform.org/ontology/oeo/OEO_00010056"/>
        <obo:BFO_0000051 rdf:resource="http://openenergy-platform.org/ontology/oeo/OEO_00010040"/>
        <obo:BFO_0000051 rdf:resource="http://openenergy-platform.org/ontology/oeo/OEO_00010057"/>
        <obo:BFO_0000051 rdf:resource="http://openenergy-platform.org/ontology/oeo/OEO_00010064"/>
        <oeo:OEO_00040001 rdf:datatype="http://www.w3.org/2001/XMLSchema#string">http://openenergy-platform.org/ontology/oeo/oeo-social</oeo:OEO_00040001>
        <obo:IAO_0000115>The KSG sector energy industry is an energy transformation sector defined by the KSG sector division. It is an aggregate of the following three sectors:
- CRF sector (IPCC 2006): energy industry (CRF 1.A.1.a)
- CRF sector (IPCC 2006): other transportation (CRF 1.A.3.e)
- CRF sector (IPCC 2006): fugitive emissions from fuels (CRF 1.B)</obo:IAO_0000115>
        <obo:IAO_0000119>Bundes-Klimaschutzgesetz (KSG), Anlage 1 (zu den §§ 4 und 5) https://www.gesetze-im-internet.de/ksg/anlage_1.html</obo:IAO_0000119>
        <obo:IAO_0000233>issue: https://github.com/OpenEnergyPlatform/ontology/issues/580
pull request: https://github.com/OpenEnergyPlatform/ontology/pull/595</obo:IAO_0000233>
        <rdfs:label>KSG sector energy industry</rdfs:label>
    </owl:NamedIndividual>
    


    <!-- http://openenergy-platform.org/ontology/oeo/OEO_00010066 -->

    <owl:NamedIndividual rdf:about="http://openenergy-platform.org/ontology/oeo/OEO_00010066">
        <rdf:type rdf:resource="http://openenergy-platform.org/ontology/oeo/OEO_00000227"/>
        <oeo:OEO_00000504 rdf:resource="http://openenergy-platform.org/ontology/oeo/OEO_00010056"/>
        <obo:BFO_0000051 rdf:resource="http://openenergy-platform.org/ontology/oeo/OEO_00010041"/>
        <obo:BFO_0000051 rdf:resource="http://openenergy-platform.org/ontology/oeo/OEO_00010046"/>
        <obo:BFO_0000051 rdf:resource="http://openenergy-platform.org/ontology/oeo/OEO_00010058"/>
        <oeo:OEO_00040001 rdf:datatype="http://www.w3.org/2001/XMLSchema#string">http://openenergy-platform.org/ontology/oeo/oeo-social</oeo:OEO_00040001>
        <obo:IAO_0000115>The KSG sector industry is an industry sector defined by the KSG sector division. It is an aggregate of the following three sectors:
- CRF sector (IPCC 2006): manufacturing industries and construction (CRF 1.A.2)
- CRF sector (IPCC 2006): CO2 transport and storage (CRF 1.C)
- CRF sector (IPCC 2006): industrial processes and product use (CRF 2)</obo:IAO_0000115>
        <obo:IAO_0000119>Bundes-Klimaschutzgesetz (KSG), Anlage 1 (zu den §§ 4 und 5) https://www.gesetze-im-internet.de/ksg/anlage_1.html</obo:IAO_0000119>
        <obo:IAO_0000233>issue: https://github.com/OpenEnergyPlatform/ontology/issues/580
pull request: https://github.com/OpenEnergyPlatform/ontology/pull/595</obo:IAO_0000233>
        <rdfs:label>KSG sector industry</rdfs:label>
    </owl:NamedIndividual>
    


    <!-- http://openenergy-platform.org/ontology/oeo/OEO_00010067 -->

    <owl:NamedIndividual rdf:about="http://openenergy-platform.org/ontology/oeo/OEO_00010067">
        <rdf:type rdf:resource="http://openenergy-platform.org/ontology/oeo/OEO_00010034"/>
        <oeo:OEO_00000504 rdf:resource="http://openenergy-platform.org/ontology/oeo/OEO_00010056"/>
        <obo:BFO_0000051 rdf:resource="http://openenergy-platform.org/ontology/oeo/OEO_00010044"/>
        <obo:BFO_0000051 rdf:resource="http://openenergy-platform.org/ontology/oeo/OEO_00010052"/>
        <obo:BFO_0000051 rdf:resource="http://openenergy-platform.org/ontology/oeo/OEO_00010053"/>
        <oeo:OEO_00040001 rdf:datatype="http://www.w3.org/2001/XMLSchema#string">http://openenergy-platform.org/ontology/oeo/oeo-social</oeo:OEO_00040001>
        <obo:IAO_0000115>The KSG sector buildings is a building sector defined by the KSG sector division. It is an aggregate of the following two sectors:
- CRF sector (IPCC 2006): commercial and institutional (CRF 1.A.4.a)
- CRF sector (IPCC 2006): residential (CRF 1.A.4.b)
- CRF sector (IPCC 2006): fuel combustion - other</obo:IAO_0000115>
        <obo:IAO_0000119>Bundes-Klimaschutzgesetz (KSG), Anlage 1 (zu den §§ 4 und 5) https://www.gesetze-im-internet.de/ksg/anlage_1.html</obo:IAO_0000119>
        <obo:IAO_0000233>issue: https://github.com/OpenEnergyPlatform/ontology/issues/580
pull request: https://github.com/OpenEnergyPlatform/ontology/pull/595

Add axiom to 1.A.5 and extend definition:
issue: https://github.com/OpenEnergyPlatform/ontology/issues/1194
pull request: https://github.com/OpenEnergyPlatform/ontology/pull/1198</obo:IAO_0000233>
        <rdfs:label>KSG sector buildings</rdfs:label>
    </owl:NamedIndividual>
    


    <!-- http://openenergy-platform.org/ontology/oeo/OEO_00010068 -->

    <owl:NamedIndividual rdf:about="http://openenergy-platform.org/ontology/oeo/OEO_00010068">
        <rdf:type rdf:resource="http://openenergy-platform.org/ontology/oeo/OEO_00000422"/>
        <oeo:OEO_00000504 rdf:resource="http://openenergy-platform.org/ontology/oeo/OEO_00010056"/>
        <obo:BFO_0000051 rdf:resource="http://openenergy-platform.org/ontology/oeo/OEO_00010059"/>
        <obo:BFO_0000051 rdf:resource="http://openenergy-platform.org/ontology/oeo/OEO_00010060"/>
        <obo:BFO_0000051 rdf:resource="http://openenergy-platform.org/ontology/oeo/OEO_00010061"/>
        <obo:BFO_0000051 rdf:resource="http://openenergy-platform.org/ontology/oeo/OEO_00010062"/>
        <oeo:OEO_00040001 rdf:datatype="http://www.w3.org/2001/XMLSchema#string">http://openenergy-platform.org/ontology/oeo/oeo-social</oeo:OEO_00040001>
        <obo:IAO_0000115>The KSG sector transport is a transport sector defined by the KSG sector division. It is an aggregate of the following four sectors:
- CRF sector (IPCC 2006): domestic aviation (CRF 1.A.3.a)
- CRF sector (IPCC 2006): road transportation (CRF 1.A.3.b)
- CRF sector (IPCC 2006): railways (CRF 1.A.3.c)
- CRF sector (IPCC 2006): domestic navigation (CRF 1.A.3.d)</obo:IAO_0000115>
        <obo:IAO_0000119>Bundes-Klimaschutzgesetz (KSG), Anlage 1 (zu den §§ 4 und 5) https://www.gesetze-im-internet.de/ksg/anlage_1.html</obo:IAO_0000119>
        <obo:IAO_0000233>issue: https://github.com/OpenEnergyPlatform/ontology/issues/580
pull request: https://github.com/OpenEnergyPlatform/ontology/pull/595</obo:IAO_0000233>
        <rdfs:label>KSG sector transport</rdfs:label>
    </owl:NamedIndividual>
    


    <!-- http://openenergy-platform.org/ontology/oeo/OEO_00010069 -->

    <owl:NamedIndividual rdf:about="http://openenergy-platform.org/ontology/oeo/OEO_00010069">
        <rdf:type rdf:resource="http://openenergy-platform.org/ontology/oeo/OEO_00010035"/>
        <oeo:OEO_00000504 rdf:resource="http://openenergy-platform.org/ontology/oeo/OEO_00010056"/>
        <obo:BFO_0000051 rdf:resource="http://openenergy-platform.org/ontology/oeo/OEO_00010047"/>
        <obo:BFO_0000051 rdf:resource="http://openenergy-platform.org/ontology/oeo/OEO_00010054"/>
        <oeo:OEO_00040001 rdf:datatype="http://www.w3.org/2001/XMLSchema#string">http://openenergy-platform.org/ontology/oeo/oeo-social</oeo:OEO_00040001>
        <obo:IAO_0000115>The KSG sector agriculture is an agriculture, forestry and land use sector defined by the KSG sector division. It is an aggregate of the following two sectors:
- CRF sector (IPCC 2006): agriculture, forestry and fishing (CRF 1.A.4.c)
- CRF sector (IPCC 2006): agriculture (CRF 3)</obo:IAO_0000115>
        <obo:IAO_0000119>Bundes-Klimaschutzgesetz (KSG), Anlage 1 (zu den §§ 4 und 5) https://www.gesetze-im-internet.de/ksg/anlage_1.html</obo:IAO_0000119>
        <obo:IAO_0000233>issue: https://github.com/OpenEnergyPlatform/ontology/issues/580
pull request: https://github.com/OpenEnergyPlatform/ontology/pull/595</obo:IAO_0000233>
        <rdfs:label>KSG sector agriculture</rdfs:label>
    </owl:NamedIndividual>
    


    <!-- http://openenergy-platform.org/ontology/oeo/OEO_00010070 -->

    <owl:NamedIndividual rdf:about="http://openenergy-platform.org/ontology/oeo/OEO_00010070">
        <rdf:type rdf:resource="http://openenergy-platform.org/ontology/oeo/OEO_00010036"/>
        <oeo:OEO_00000504 rdf:resource="http://openenergy-platform.org/ontology/oeo/OEO_00010056"/>
        <obo:BFO_0000051 rdf:resource="http://openenergy-platform.org/ontology/oeo/OEO_00010049"/>
        <obo:BFO_0000051 rdf:resource="http://openenergy-platform.org/ontology/oeo/OEO_00010050"/>
        <oeo:OEO_00040001 rdf:datatype="http://www.w3.org/2001/XMLSchema#string">http://openenergy-platform.org/ontology/oeo/oeo-social</oeo:OEO_00040001>
        <obo:IAO_0000115>The KSG sector waste management and other is a sector defined by the KSG sector division. It is an aggregate of the following two sectors:
- CRF sector (IPCC 2006): waste (CRF 5)
- CRF sector (IPCC 2006): other (CRF 6)</obo:IAO_0000115>
        <obo:IAO_0000119>Bundes-Klimaschutzgesetz (KSG), Anlage 1 (zu den §§ 4 und 5) https://www.gesetze-im-internet.de/ksg/anlage_1.html</obo:IAO_0000119>
        <obo:IAO_0000233>issue: https://github.com/OpenEnergyPlatform/ontology/issues/580
pull request: https://github.com/OpenEnergyPlatform/ontology/pull/595</obo:IAO_0000233>
        <rdfs:label>KSG sector waste management and other</rdfs:label>
    </owl:NamedIndividual>
    


    <!-- http://openenergy-platform.org/ontology/oeo/OEO_00010071 -->

    <owl:NamedIndividual rdf:about="http://openenergy-platform.org/ontology/oeo/OEO_00010071">
        <rdf:type rdf:resource="http://openenergy-platform.org/ontology/oeo/OEO_00010035"/>
        <oeo:OEO_00000504 rdf:resource="http://openenergy-platform.org/ontology/oeo/OEO_00010056"/>
        <oeo:OEO_00040001 rdf:datatype="http://www.w3.org/2001/XMLSchema#string">http://openenergy-platform.org/ontology/oeo/oeo-social</oeo:OEO_00040001>
        <obo:IAO_0000115>The KSG sector land use, land-use change and forestry is an agriculture, forestry and land use sector defined by the KSG sector division.
It is equivalent to the CRF sector (IPCC 2006): land use, land-use change and forestry (CRF 4).</obo:IAO_0000115>
        <obo:IAO_0000119>Bundes-Klimaschutzgesetz (KSG), Anlage 1 (zu den §§ 4 und 5) https://www.gesetze-im-internet.de/ksg/anlage_1.html</obo:IAO_0000119>
        <obo:IAO_0000233>issue: https://github.com/OpenEnergyPlatform/ontology/issues/580
pull request: https://github.com/OpenEnergyPlatform/ontology/pull/595</obo:IAO_0000233>
        <rdfs:label>KSG sector land use, land-use change and forestry</rdfs:label>
    </owl:NamedIndividual>
    


    <!-- http://openenergy-platform.org/ontology/oeo/OEO_00010122 -->

    <owl:NamedIndividual rdf:about="http://openenergy-platform.org/ontology/oeo/OEO_00010122">
        <rdf:type rdf:resource="http://openenergy-platform.org/ontology/oeo/OEO_00140151"/>
        <rdf:type>
            <owl:Restriction>
                <owl:onProperty rdf:resource="http://openenergy-platform.org/ontology/oeo/OEO_00000503"/>
                <owl:someValuesFrom rdf:resource="http://openenergy-platform.org/ontology/oeo/OEO_00020064"/>
            </owl:Restriction>
        </rdf:type>
        <oeo:OEO_00010128 rdf:resource="http://openenergy-platform.org/ontology/oeo/OEO_00010131"/>
        <oeo:OEO_00010128 rdf:resource="http://openenergy-platform.org/ontology/oeo/OEO_00010132"/>
        <oeo:OEO_00010128 rdf:resource="http://openenergy-platform.org/ontology/oeo/OEO_00010133"/>
        <oeo:OEO_00010128 rdf:resource="http://openenergy-platform.org/ontology/oeo/OEO_00010205"/>
        <obo:BFO_0000050 rdf:resource="http://openenergy-platform.org/ontology/oeo/OEO_00010129"/>
        <oeo:OEO_00040001 rdf:datatype="http://www.w3.org/2001/XMLSchema#string">http://openenergy-platform.org/ontology/oeo/oeo-social</oeo:OEO_00040001>
        <obo:IAO_0000115>The European Union Emissions Trading System (EU ETS) is a policy instrument that implements an emissions trading system covering the European Union, Norway, Iceland and Liechtenstein.</obo:IAO_0000115>
        <obo:IAO_0000118>EU ETS</obo:IAO_0000118>
        <obo:IAO_0000233>issue: https://github.com/OpenEnergyPlatform/ontology/issues/834
pull request: https://github.com/OpenEnergyPlatform/ontology/pull/857

add axioms:
issue: https://github.com/OpenEnergyPlatform/ontology/issues/928
pull request: https://github.com/OpenEnergyPlatform/ontology/pull/944</obo:IAO_0000233>
        <rdfs:label xml:lang="en">European Union Emissions Trading System</rdfs:label>
    </owl:NamedIndividual>
    


    <!-- http://openenergy-platform.org/ontology/oeo/OEO_00010124 -->

    <owl:NamedIndividual rdf:about="http://openenergy-platform.org/ontology/oeo/OEO_00010124">
        <rdf:type rdf:resource="http://openenergy-platform.org/ontology/oeo/OEO_00010123"/>
        <rdf:type>
            <owl:Restriction>
                <owl:onProperty rdf:resource="http://openenergy-platform.org/ontology/oeo/OEO_00000503"/>
                <owl:someValuesFrom rdf:resource="http://openenergy-platform.org/ontology/oeo/OEO_00010126"/>
            </owl:Restriction>
        </rdf:type>
        <obo:BFO_0000050 rdf:resource="http://openenergy-platform.org/ontology/oeo/OEO_00010129"/>
        <oeo:OEO_00040001 rdf:datatype="http://www.w3.org/2001/XMLSchema#string">http://openenergy-platform.org/ontology/oeo/oeo-social</oeo:OEO_00040001>
        <obo:IAO_0000115>The Effort Sharing Decision (ESD) is the European effort sharing for the years 2013-2020. It covers the European Union, Norway, Iceland and Liechtenstein and the following greenhouse gases: carbon dioxide, methane, nitrous oxide, hydrofluorocarbons, perfluorocarbons and sulphur hexafluoride. Emission quantities under the ESD are calculated using global warming potentials from the Fourth IPCC Assessment Report.</obo:IAO_0000115>
        <obo:IAO_0000118>ESD</obo:IAO_0000118>
        <obo:IAO_0000233>issue: https://github.com/OpenEnergyPlatform/ontology/issues/834
pull request: https://github.com/OpenEnergyPlatform/ontology/pull/857</obo:IAO_0000233>
        <rdfs:label xml:lang="en">Effort Sharing Decision</rdfs:label>
    </owl:NamedIndividual>
    


    <!-- http://openenergy-platform.org/ontology/oeo/OEO_00010125 -->

    <owl:NamedIndividual rdf:about="http://openenergy-platform.org/ontology/oeo/OEO_00010125">
        <rdf:type rdf:resource="http://openenergy-platform.org/ontology/oeo/OEO_00010123"/>
        <rdf:type>
            <owl:Restriction>
                <owl:onProperty rdf:resource="http://openenergy-platform.org/ontology/oeo/OEO_00000503"/>
                <owl:someValuesFrom rdf:resource="http://openenergy-platform.org/ontology/oeo/OEO_00010126"/>
            </owl:Restriction>
        </rdf:type>
        <obo:BFO_0000050 rdf:resource="http://openenergy-platform.org/ontology/oeo/OEO_00010129"/>
        <oeo:OEO_00040001 rdf:datatype="http://www.w3.org/2001/XMLSchema#string">http://openenergy-platform.org/ontology/oeo/oeo-social</oeo:OEO_00040001>
        <obo:IAO_0000115>The Effort Sharing Regulation (ESR) is the European effort sharing for the years 2021-2030. It covers the European Union, Norway, Iceland and Liechtenstein and the following greenhouse gases: carbon dioxide, methane, nitrous oxide, hydrofluorocarbons, perfluorocarbons, sulphur hexafluoride and nitrogen trifluoride. Emission quantities under the ESR are calculated using global warming potentials from the Fifth IPCC Assessment Report.</obo:IAO_0000115>
        <obo:IAO_0000118>ESR</obo:IAO_0000118>
        <obo:IAO_0000233>issue: https://github.com/OpenEnergyPlatform/ontology/issues/834
pull request: https://github.com/OpenEnergyPlatform/ontology/pull/857</obo:IAO_0000233>
        <rdfs:label xml:lang="en">Effort Sharing Regulation</rdfs:label>
    </owl:NamedIndividual>
    


    <!-- http://openenergy-platform.org/ontology/oeo/OEO_00010129 -->

    <owl:NamedIndividual rdf:about="http://openenergy-platform.org/ontology/oeo/OEO_00010129">
        <rdf:type rdf:resource="http://openenergy-platform.org/ontology/oeo/OEO_00140150"/>
        <oeo:OEO_00000503 rdf:resource="http://openenergy-platform.org/ontology/oeo/OEO_00010130"/>
        <oeo:OEO_00040001 rdf:datatype="http://www.w3.org/2001/XMLSchema#string">http://openenergy-platform.org/ontology/oeo/oeo-social</oeo:OEO_00040001>
        <obo:IAO_0000115>The EU climate policy is the policy of the European Union for reducing greenhouse gas emissions. It uses the EU emission sector division.</obo:IAO_0000115>
        <obo:IAO_0000233>issue: https://github.com/OpenEnergyPlatform/ontology/issues/834
pull request: https://github.com/OpenEnergyPlatform/ontology/pull/857</obo:IAO_0000233>
        <rdfs:label xml:lang="en">EU climate policy</rdfs:label>
    </owl:NamedIndividual>
    


    <!-- http://openenergy-platform.org/ontology/oeo/OEO_00010130 -->

    <owl:NamedIndividual rdf:about="http://openenergy-platform.org/ontology/oeo/OEO_00010130">
        <rdf:type rdf:resource="http://openenergy-platform.org/ontology/oeo/OEO_00000368"/>
        <oeo:OEO_00000504 rdf:resource="http://openenergy-platform.org/ontology/oeo/OEO_00010129"/>
        <oeo:OEO_00040001 rdf:datatype="http://www.w3.org/2001/XMLSchema#string">http://openenergy-platform.org/ontology/oeo/oeo-social</oeo:OEO_00040001>
        <obo:IAO_0000115>The EU emission sector division is used in the EU climate policy.</obo:IAO_0000115>
        <obo:IAO_0000233>issue: https://github.com/OpenEnergyPlatform/ontology/issues/834
pull request: https://github.com/OpenEnergyPlatform/ontology/pull/857</obo:IAO_0000233>
        <rdfs:label xml:lang="en">EU emission sector division</rdfs:label>
    </owl:NamedIndividual>
    


    <!-- http://openenergy-platform.org/ontology/oeo/OEO_00010131 -->

    <owl:NamedIndividual rdf:about="http://openenergy-platform.org/ontology/oeo/OEO_00010131">
        <rdf:type rdf:resource="http://openenergy-platform.org/ontology/oeo/OEO_00000367"/>
        <oeo:OEO_00000504 rdf:resource="http://openenergy-platform.org/ontology/oeo/OEO_00010130"/>
        <oeo:OEO_00040001 rdf:datatype="http://www.w3.org/2001/XMLSchema#string">http://openenergy-platform.org/ontology/oeo/oeo-social</oeo:OEO_00040001>
        <obo:IAO_0000115>The EU emission sector ETS is a sector defined by the EU emission sector division that covers greenhouse gas emissions that are regulated by the European Union Emissions Trading System.</obo:IAO_0000115>
        <obo:IAO_0000233>issue: https://github.com/OpenEnergyPlatform/ontology/issues/834
pull request: https://github.com/OpenEnergyPlatform/ontology/pull/857</obo:IAO_0000233>
        <rdfs:label xml:lang="en">EU emission sector: ETS</rdfs:label>
    </owl:NamedIndividual>
    


    <!-- http://openenergy-platform.org/ontology/oeo/OEO_00010132 -->

    <owl:NamedIndividual rdf:about="http://openenergy-platform.org/ontology/oeo/OEO_00010132">
        <rdf:type rdf:resource="http://openenergy-platform.org/ontology/oeo/OEO_00000367"/>
        <oeo:OEO_00000504 rdf:resource="http://openenergy-platform.org/ontology/oeo/OEO_00010130"/>
        <obo:BFO_0000050 rdf:resource="http://openenergy-platform.org/ontology/oeo/OEO_00010131"/>
        <oeo:OEO_00040001 rdf:datatype="http://www.w3.org/2001/XMLSchema#string">http://openenergy-platform.org/ontology/oeo/oeo-social</oeo:OEO_00040001>
        <obo:IAO_0000115>The EU emission sector ETS stationary is a sector defined by the EU emission sector division that covers greenhouse gas emissions regulated by the European Union Emissions Trading System and that are emitted by stationary installations.</obo:IAO_0000115>
        <obo:IAO_0000233>issue: https://github.com/OpenEnergyPlatform/ontology/issues/834
pull request: https://github.com/OpenEnergyPlatform/ontology/pull/857</obo:IAO_0000233>
        <rdfs:label xml:lang="en">EU emission sector: ETS stationary</rdfs:label>
    </owl:NamedIndividual>
    


    <!-- http://openenergy-platform.org/ontology/oeo/OEO_00010133 -->

    <owl:NamedIndividual rdf:about="http://openenergy-platform.org/ontology/oeo/OEO_00010133">
        <rdf:type rdf:resource="http://openenergy-platform.org/ontology/oeo/OEO_00000422"/>
        <oeo:OEO_00000504 rdf:resource="http://openenergy-platform.org/ontology/oeo/OEO_00010130"/>
        <obo:BFO_0000050 rdf:resource="http://openenergy-platform.org/ontology/oeo/OEO_00010131"/>
        <oeo:OEO_00040001 rdf:datatype="http://www.w3.org/2001/XMLSchema#string">http://openenergy-platform.org/ontology/oeo/oeo-social</oeo:OEO_00040001>
        <obo:IAO_0000115>The EU emission sector ETS aviation is a transport sector defined by the EU emission sector division that covers greenhouse gas emissions regulated by the European Union Emissions Trading System and that are emitted by stationary installations.</obo:IAO_0000115>
        <obo:IAO_0000233>issue: https://github.com/OpenEnergyPlatform/ontology/issues/834
pull request: https://github.com/OpenEnergyPlatform/ontology/pull/857</obo:IAO_0000233>
        <rdfs:label xml:lang="en">EU emission sector: ETS aviation</rdfs:label>
    </owl:NamedIndividual>
    


    <!-- http://openenergy-platform.org/ontology/oeo/OEO_00010134 -->

    <owl:NamedIndividual rdf:about="http://openenergy-platform.org/ontology/oeo/OEO_00010134">
        <rdf:type rdf:resource="http://openenergy-platform.org/ontology/oeo/OEO_00000367"/>
        <oeo:OEO_00000504 rdf:resource="http://openenergy-platform.org/ontology/oeo/OEO_00010130"/>
        <oeo:OEO_00040001 rdf:datatype="http://www.w3.org/2001/XMLSchema#string">http://openenergy-platform.org/ontology/oeo/oeo-social</oeo:OEO_00040001>
        <obo:IAO_0000115>The EU emission sector effort sharing is a sector defined by the EU emission sector division that covers greenhouse gas emissions regulated by the Effort Sharing Decision and the Effort Sharing Regulation.</obo:IAO_0000115>
        <obo:IAO_0000233>issue: https://github.com/OpenEnergyPlatform/ontology/issues/834
pull request: https://github.com/OpenEnergyPlatform/ontology/pull/857</obo:IAO_0000233>
        <rdfs:label xml:lang="en">EU emission sector: effort sharing</rdfs:label>
    </owl:NamedIndividual>
    


    <!-- http://openenergy-platform.org/ontology/oeo/OEO_00010135 -->

    <owl:NamedIndividual rdf:about="http://openenergy-platform.org/ontology/oeo/OEO_00010135">
        <rdf:type rdf:resource="http://openenergy-platform.org/ontology/oeo/OEO_00010035"/>
        <oeo:OEO_00000504 rdf:resource="http://openenergy-platform.org/ontology/oeo/OEO_00010130"/>
        <oeo:OEO_00040001 rdf:datatype="http://www.w3.org/2001/XMLSchema#string">http://openenergy-platform.org/ontology/oeo/oeo-social</oeo:OEO_00040001>
        <obo:IAO_0000115>The EU emission sector ETS stationary is a sector defined by the EU emission sector division that covers greenhouse gas emissions regulated by the European Union Emissions Trading System and that are emitted by stationary installations.</obo:IAO_0000115>
        <obo:IAO_0000233>issue: https://github.com/OpenEnergyPlatform/ontology/issues/834
pull request: https://github.com/OpenEnergyPlatform/ontology/pull/857</obo:IAO_0000233>
        <rdfs:label xml:lang="en">EU emission sector: LULUCF</rdfs:label>
    </owl:NamedIndividual>
    


    <!-- http://openenergy-platform.org/ontology/oeo/OEO_00010158 -->

    <owl:NamedIndividual rdf:about="http://openenergy-platform.org/ontology/oeo/OEO_00010158">
        <rdf:type rdf:resource="http://openenergy-platform.org/ontology/oeo/OEO_00000158"/>
        <oeo:OEO_00000504 rdf:resource="http://openenergy-platform.org/ontology/oeo/OEO_00000242"/>
        <obo:BFO_0000050 rdf:resource="http://openenergy-platform.org/ontology/oeo/OEO_00010040"/>
        <oeo:OEO_00010037>CRF 1.A.1.a</oeo:OEO_00010037>
        <oeo:OEO_00040001 rdf:datatype="http://www.w3.org/2001/XMLSchema#string">http://openenergy-platform.org/ontology/oeo/oeo-social</oeo:OEO_00040001>
        <obo:IAO_0000115>The CRF sector (IPCC 2006) &apos;public electricity and heat production&apos; is an energy transformation sector defined by the 2006 IPCC Guidelines for National Greenhouse Gas Inventories:
Sum of emissions from main activity producers of electricity generation, combined heat and power generation, and heat plants.</obo:IAO_0000115>
        <obo:IAO_0000119>2006 IPCC Guidelines for National Greenhouse Gas Inventories, Volume 2, Chapter 2.2, https://www.ipcc-nggip.iges.or.jp/public/2006gl/</obo:IAO_0000119>
        <obo:IAO_0000233>issue: https://github.com/OpenEnergyPlatform/ontology/issues/858
pull request: https://github.com/OpenEnergyPlatform/ontology/pull/941</obo:IAO_0000233>
        <rdfs:label xml:lang="en">CRF sector (IPCC 2006): public electricity and heat production</rdfs:label>
    </owl:NamedIndividual>
    


    <!-- http://openenergy-platform.org/ontology/oeo/OEO_00010159 -->

    <owl:NamedIndividual rdf:about="http://openenergy-platform.org/ontology/oeo/OEO_00010159">
        <rdf:type rdf:resource="http://openenergy-platform.org/ontology/oeo/OEO_00010319"/>
        <oeo:OEO_00000504 rdf:resource="http://openenergy-platform.org/ontology/oeo/OEO_00000242"/>
        <obo:BFO_0000050 rdf:resource="http://openenergy-platform.org/ontology/oeo/OEO_00010040"/>
        <oeo:OEO_00010037>CRF 1.A.1.b</oeo:OEO_00010037>
        <oeo:OEO_00040001 rdf:datatype="http://www.w3.org/2001/XMLSchema#string">http://openenergy-platform.org/ontology/oeo/oeo-social</oeo:OEO_00040001>
        <obo:IAO_0000115>The CRF sector (IPCC 2006) &apos;petroleum refining&apos; is an energy transformation sector defined by the 2006 IPCC Guidelines for National Greenhouse Gas Inventories:
All combustion activities supporting the refining of petroleum products including on-site combustion for the generation of electricity and heat for own use.</obo:IAO_0000115>
        <obo:IAO_0000119>2006 IPCC Guidelines for National Greenhouse Gas Inventories, Volume 2, Chapter 2.2, https://www.ipcc-nggip.iges.or.jp/public/2006gl/</obo:IAO_0000119>
        <obo:IAO_0000233>issue: https://github.com/OpenEnergyPlatform/ontology/issues/858
pull request: https://github.com/OpenEnergyPlatform/ontology/pull/941

Make individual of &apos;mineral oil refining sector&apos;:
issue: https://github.com/OpenEnergyPlatform/ontology/issues/1318
pull request: https://github.com/OpenEnergyPlatform/ontology/pull/1331</obo:IAO_0000233>
        <rdfs:label>CRF sector (IPCC 2006): petroleum refining</rdfs:label>
    </owl:NamedIndividual>
    


    <!-- http://openenergy-platform.org/ontology/oeo/OEO_00010160 -->

    <owl:NamedIndividual rdf:about="http://openenergy-platform.org/ontology/oeo/OEO_00010160">
        <rdf:type rdf:resource="http://openenergy-platform.org/ontology/oeo/OEO_00000158"/>
        <oeo:OEO_00000504 rdf:resource="http://openenergy-platform.org/ontology/oeo/OEO_00000242"/>
        <obo:BFO_0000050 rdf:resource="http://openenergy-platform.org/ontology/oeo/OEO_00010040"/>
        <oeo:OEO_00010037>CRF 1.A.1.c</oeo:OEO_00010037>
        <oeo:OEO_00040001 rdf:datatype="http://www.w3.org/2001/XMLSchema#string">http://openenergy-platform.org/ontology/oeo/oeo-social</oeo:OEO_00040001>
        <obo:IAO_0000115>The CRF sector (IPCC 2006) &apos;manufacture of solid fuels and other energy industries&apos; is an energy transformation sector defined by the 2006 IPCC Guidelines for National Greenhouse Gas Inventories:
Combustion emissions from fuel use during the manufacture of secondary and tertiary products from solid fuels including production of charcoal.</obo:IAO_0000115>
        <obo:IAO_0000119>2006 IPCC Guidelines for National Greenhouse Gas Inventories, Volume 2, Chapter 2.2, https://www.ipcc-nggip.iges.or.jp/public/2006gl/</obo:IAO_0000119>
        <obo:IAO_0000233>issue: https://github.com/OpenEnergyPlatform/ontology/issues/858
pull request: https://github.com/OpenEnergyPlatform/ontology/pull/941</obo:IAO_0000233>
        <rdfs:label xml:lang="en">CRF sector (IPCC 2006): manufacture of solid fuels and other energy industries</rdfs:label>
    </owl:NamedIndividual>
    


    <!-- http://openenergy-platform.org/ontology/oeo/OEO_00010161 -->

    <owl:NamedIndividual rdf:about="http://openenergy-platform.org/ontology/oeo/OEO_00010161">
        <rdf:type rdf:resource="http://openenergy-platform.org/ontology/oeo/OEO_00000367"/>
        <oeo:OEO_00000504 rdf:resource="http://openenergy-platform.org/ontology/oeo/OEO_00000242"/>
        <obo:BFO_0000050 rdf:resource="http://openenergy-platform.org/ontology/oeo/OEO_00010057"/>
        <oeo:OEO_00010037>CRF 1.B.1</oeo:OEO_00010037>
        <oeo:OEO_00040001 rdf:datatype="http://www.w3.org/2001/XMLSchema#string">http://openenergy-platform.org/ontology/oeo/oeo-social</oeo:OEO_00040001>
        <obo:IAO_0000115>The CRF sector (IPCC 2006) &apos;solid fuels&apos; is a sector defined by the 2006 IPCC Guidelines for National Greenhouse Gas Inventories:
Includes all intentional and unintentional emissions from the extraction, processing, storage and transport of fuel to the point of final use.</obo:IAO_0000115>
        <obo:IAO_0000119>2006 IPCC Guidelines for National Greenhouse Gas Inventories, Volume 1, Chapter 8.5, https://www.ipcc-nggip.iges.or.jp/public/2006gl/</obo:IAO_0000119>
        <obo:IAO_0000233>issue: https://github.com/OpenEnergyPlatform/ontology/issues/858
pull request: https://github.com/OpenEnergyPlatform/ontology/pull/941</obo:IAO_0000233>
        <rdfs:label xml:lang="en">CRF sector (IPCC 2006): solid fuels</rdfs:label>
    </owl:NamedIndividual>
    


    <!-- http://openenergy-platform.org/ontology/oeo/OEO_00010162 -->

    <owl:NamedIndividual rdf:about="http://openenergy-platform.org/ontology/oeo/OEO_00010162">
        <rdf:type rdf:resource="http://openenergy-platform.org/ontology/oeo/OEO_00000367"/>
        <oeo:OEO_00000504 rdf:resource="http://openenergy-platform.org/ontology/oeo/OEO_00000242"/>
        <obo:BFO_0000050 rdf:resource="http://openenergy-platform.org/ontology/oeo/OEO_00010057"/>
        <oeo:OEO_00010037>CRF 1.B.2</oeo:OEO_00010037>
        <oeo:OEO_00040001 rdf:datatype="http://www.w3.org/2001/XMLSchema#string">http://openenergy-platform.org/ontology/oeo/oeo-social</oeo:OEO_00040001>
        <obo:IAO_0000115>The CRF sector (IPCC 2006) &apos;oil and natural gas&apos; is a sector defined by the 2006 IPCC Guidelines for National Greenhouse Gas Inventories:
Comprises fugitive emissions from all oil and natural gas activities.</obo:IAO_0000115>
        <obo:IAO_0000119>2006 IPCC Guidelines for National Greenhouse Gas Inventories, Volume 1, Chapter 8.5, https://www.ipcc-nggip.iges.or.jp/public/2006gl/</obo:IAO_0000119>
        <obo:IAO_0000233>issue: https://github.com/OpenEnergyPlatform/ontology/issues/858
pull request: https://github.com/OpenEnergyPlatform/ontology/pull/941</obo:IAO_0000233>
        <rdfs:label xml:lang="en">CRF sector (IPCC 2006): oil and natural gas</rdfs:label>
    </owl:NamedIndividual>
    


    <!-- http://openenergy-platform.org/ontology/oeo/OEO_00010163 -->

    <owl:NamedIndividual rdf:about="http://openenergy-platform.org/ontology/oeo/OEO_00010163">
        <rdf:type rdf:resource="http://openenergy-platform.org/ontology/oeo/OEO_00000368"/>
        <oeo:OEO_00000503 rdf:resource="http://openenergy-platform.org/ontology/oeo/OEO_00000242"/>
        <oeo:OEO_00040001 rdf:datatype="http://www.w3.org/2001/XMLSchema#string">http://openenergy-platform.org/ontology/oeo/oeo-social</oeo:OEO_00040001>
        <obo:IAO_0000115>The GovReg sector division is a sector division defined in Annex XXV, Table 1a of Commission Implementing Regulation (EU) 2020/1208. It uses CRF sectors (IPCC 2006) and adds further sectors.</obo:IAO_0000115>
        <obo:IAO_0000116>Annex XXV, Table 1a of Commission Implementing Regulation (EU) 2020/1208: https://eur-lex.europa.eu/legal-content/EN/TXT/HTML/?uri=CELEX:32020R1208&amp;from=EN#d1e32-98-1</obo:IAO_0000116>
        <obo:IAO_0000233>issue: https://github.com/OpenEnergyPlatform/ontology/issues/858
pull request: https://github.com/OpenEnergyPlatform/ontology/pull/941

relabel:
issue: https://github.com/OpenEnergyPlatform/ontology/issues/928
pull request: https://github.com/OpenEnergyPlatform/ontology/pull/944</obo:IAO_0000233>
        <rdfs:label xml:lang="en">GovReg sector division</rdfs:label>
    </owl:NamedIndividual>
    


    <!-- http://openenergy-platform.org/ontology/oeo/OEO_00010164 -->

    <owl:NamedIndividual rdf:about="http://openenergy-platform.org/ontology/oeo/OEO_00010164">
        <rdf:type rdf:resource="http://openenergy-platform.org/ontology/oeo/OEO_00000227"/>
        <oeo:OEO_00000504 rdf:resource="http://openenergy-platform.org/ontology/oeo/OEO_00000242"/>
        <obo:BFO_0000050 rdf:resource="http://openenergy-platform.org/ontology/oeo/OEO_00010046"/>
        <oeo:OEO_00010037>CRF 2.A</oeo:OEO_00010037>
        <oeo:OEO_00040001 rdf:datatype="http://www.w3.org/2001/XMLSchema#string">http://openenergy-platform.org/ontology/oeo/oeo-social</oeo:OEO_00040001>
        <obo:IAO_0000115>The CRF sector (IPCC 2006) &apos;mineral industry&apos; is an industry sector defined by the 2006 IPCC Guidelines for National Greenhouse Gas Inventories:
Process-related carbon dioxide (CO2) emissions resulting from the use of carbonate raw materials in the production and use of a variety of mineral industry products.</obo:IAO_0000115>
        <obo:IAO_0000119>2006 IPCC Guidelines for National Greenhouse Gas Inventories, Volume 3, Chapter 2.1, https://www.ipcc-nggip.iges.or.jp/public/2006gl/</obo:IAO_0000119>
        <obo:IAO_0000233>issue: https://github.com/OpenEnergyPlatform/ontology/issues/858
pull request: https://github.com/OpenEnergyPlatform/ontology/pull/941</obo:IAO_0000233>
        <rdfs:label xml:lang="en">CRF sector (IPCC 2006): mineral industry</rdfs:label>
    </owl:NamedIndividual>
    


    <!-- http://openenergy-platform.org/ontology/oeo/OEO_00010165 -->

    <owl:NamedIndividual rdf:about="http://openenergy-platform.org/ontology/oeo/OEO_00010165">
        <rdf:type rdf:resource="http://openenergy-platform.org/ontology/oeo/OEO_00000227"/>
        <oeo:OEO_00000504 rdf:resource="http://openenergy-platform.org/ontology/oeo/OEO_00000242"/>
        <obo:BFO_0000050 rdf:resource="http://openenergy-platform.org/ontology/oeo/OEO_00010164"/>
        <oeo:OEO_00010037>CRF 2.A.1</oeo:OEO_00010037>
        <oeo:OEO_00040001 rdf:datatype="http://www.w3.org/2001/XMLSchema#string">http://openenergy-platform.org/ontology/oeo/oeo-social</oeo:OEO_00040001>
        <obo:IAO_0000115>The CRF sector (IPCC 2006) &apos;cement production&apos; is an industry sector defined by the 2006 IPCC Guidelines for National Greenhouse Gas Inventories:
Process-related emissions from the production of various types of cement (ISIC: D2694).</obo:IAO_0000115>
        <obo:IAO_0000119>2006 IPCC Guidelines for National Greenhouse Gas Inventories, Volume 1, Chapter 8.5, https://www.ipcc-nggip.iges.or.jp/public/2006gl/</obo:IAO_0000119>
        <obo:IAO_0000233>issue: https://github.com/OpenEnergyPlatform/ontology/issues/858
pull request: https://github.com/OpenEnergyPlatform/ontology/pull/941</obo:IAO_0000233>
        <rdfs:label xml:lang="en">CRF sector (IPCC 2006): cement production</rdfs:label>
    </owl:NamedIndividual>
    


    <!-- http://openenergy-platform.org/ontology/oeo/OEO_00010166 -->

    <owl:NamedIndividual rdf:about="http://openenergy-platform.org/ontology/oeo/OEO_00010166">
        <rdf:type rdf:resource="http://openenergy-platform.org/ontology/oeo/OEO_00000227"/>
        <oeo:OEO_00000504 rdf:resource="http://openenergy-platform.org/ontology/oeo/OEO_00000242"/>
        <obo:BFO_0000050 rdf:resource="http://openenergy-platform.org/ontology/oeo/OEO_00010046"/>
        <oeo:OEO_00010037>CRF 2.B</oeo:OEO_00010037>
        <oeo:OEO_00040001 rdf:datatype="http://www.w3.org/2001/XMLSchema#string">http://openenergy-platform.org/ontology/oeo/oeo-social</oeo:OEO_00040001>
        <obo:IAO_0000115>The CRF sector (IPCC 2006) &apos;chemical industry&apos; is an industry sector defined by the 2006 IPCC Guidelines for National Greenhouse Gas Inventories:
Greenhouse gas emissions that result from the production of various inorganic and organic chemicals.</obo:IAO_0000115>
        <obo:IAO_0000119>2006 IPCC Guidelines for National Greenhouse Gas Inventories, Volume 3, Chapter 3.1, https://www.ipcc-nggip.iges.or.jp/public/2006gl/</obo:IAO_0000119>
        <obo:IAO_0000233>issue: https://github.com/OpenEnergyPlatform/ontology/issues/858
pull request: https://github.com/OpenEnergyPlatform/ontology/pull/941</obo:IAO_0000233>
        <rdfs:label xml:lang="en">CRF sector (IPCC 2006): chemical industry</rdfs:label>
    </owl:NamedIndividual>
    


    <!-- http://openenergy-platform.org/ontology/oeo/OEO_00010167 -->

    <owl:NamedIndividual rdf:about="http://openenergy-platform.org/ontology/oeo/OEO_00010167">
        <rdf:type rdf:resource="http://openenergy-platform.org/ontology/oeo/OEO_00000227"/>
        <oeo:OEO_00000504 rdf:resource="http://openenergy-platform.org/ontology/oeo/OEO_00000242"/>
        <obo:BFO_0000050 rdf:resource="http://openenergy-platform.org/ontology/oeo/OEO_00010046"/>
        <oeo:OEO_00010037>CRF 2.C</oeo:OEO_00010037>
        <oeo:OEO_00040001 rdf:datatype="http://www.w3.org/2001/XMLSchema#string">http://openenergy-platform.org/ontology/oeo/oeo-social</oeo:OEO_00040001>
        <obo:IAO_0000115>The CRF sector (IPCC 2006) &apos;metal industry&apos; is an industry sector defined by the 2006 IPCC Guidelines for National Greenhouse Gas Inventories:
Greenhouse gas emissions that result from the production of metals.</obo:IAO_0000115>
        <obo:IAO_0000119>2006 IPCC Guidelines for National Greenhouse Gas Inventories, Volume 3, Chapter 4.1, https://www.ipcc-nggip.iges.or.jp/public/2006gl/</obo:IAO_0000119>
        <obo:IAO_0000233>issue: https://github.com/OpenEnergyPlatform/ontology/issues/858
pull request: https://github.com/OpenEnergyPlatform/ontology/pull/941</obo:IAO_0000233>
        <rdfs:label xml:lang="en">CRF sector (IPCC 2006): metal industry</rdfs:label>
    </owl:NamedIndividual>
    


    <!-- http://openenergy-platform.org/ontology/oeo/OEO_00010168 -->

    <owl:NamedIndividual rdf:about="http://openenergy-platform.org/ontology/oeo/OEO_00010168">
        <rdf:type rdf:resource="http://openenergy-platform.org/ontology/oeo/OEO_00000227"/>
        <oeo:OEO_00000504 rdf:resource="http://openenergy-platform.org/ontology/oeo/OEO_00000242"/>
        <obo:BFO_0000050 rdf:resource="http://openenergy-platform.org/ontology/oeo/OEO_00010167"/>
        <oeo:OEO_00010037>CRF 2.C.1</oeo:OEO_00010037>
        <oeo:OEO_00040001 rdf:datatype="http://www.w3.org/2001/XMLSchema#string">http://openenergy-platform.org/ontology/oeo/oeo-social</oeo:OEO_00040001>
        <obo:IAO_0000115>The CRF sector (IPCC 2006) &apos;cement production&apos; is an industry sector defined by the 2006 IPCC Guidelines for National Greenhouse Gas Inventories:
Carbon dioxide is the predominant gas emitted from the production of iron and steel. The sources of the carbon dioxide emissions include that from carbon-containing reducing agents such as coke and pulverized coal, and, from minerals such as limestone and dolomite added.</obo:IAO_0000115>
        <obo:IAO_0000119>2006 IPCC Guidelines for National Greenhouse Gas Inventories, Volume 1, Chapter 8.5, https://www.ipcc-nggip.iges.or.jp/public/2006gl/</obo:IAO_0000119>
        <obo:IAO_0000233>issue: https://github.com/OpenEnergyPlatform/ontology/issues/858
pull request: https://github.com/OpenEnergyPlatform/ontology/pull/941</obo:IAO_0000233>
        <rdfs:label xml:lang="en">CRF sector (IPCC 2006): iron and steel production</rdfs:label>
    </owl:NamedIndividual>
    


    <!-- http://openenergy-platform.org/ontology/oeo/OEO_00010169 -->

    <owl:NamedIndividual rdf:about="http://openenergy-platform.org/ontology/oeo/OEO_00010169">
        <rdf:type rdf:resource="http://openenergy-platform.org/ontology/oeo/OEO_00000227"/>
        <oeo:OEO_00000504 rdf:resource="http://openenergy-platform.org/ontology/oeo/OEO_00000242"/>
        <obo:BFO_0000050 rdf:resource="http://openenergy-platform.org/ontology/oeo/OEO_00010046"/>
        <oeo:OEO_00010037>CRF 2.D</oeo:OEO_00010037>
        <oeo:OEO_00040001 rdf:datatype="http://www.w3.org/2001/XMLSchema#string">http://openenergy-platform.org/ontology/oeo/oeo-social</oeo:OEO_00040001>
        <obo:IAO_0000115>The CRF sector (IPCC 2006) &apos;non-energy products from fuels and solvent use&apos; is an industry sector defined by the 2006 IPCC Guidelines for National Greenhouse Gas Inventories:
The use of oil products and coal-derived oils primarily intended for purposes other than combustion</obo:IAO_0000115>
        <obo:IAO_0000119>2006 IPCC Guidelines for National Greenhouse Gas Inventories, Volume 1, Chapter 8.5, https://www.ipcc-nggip.iges.or.jp/public/2006gl/</obo:IAO_0000119>
        <obo:IAO_0000233>issue: https://github.com/OpenEnergyPlatform/ontology/issues/858
pull request: https://github.com/OpenEnergyPlatform/ontology/pull/941</obo:IAO_0000233>
        <rdfs:label xml:lang="en">CRF sector (IPCC 2006): non-energy products from fuels and solvent use</rdfs:label>
    </owl:NamedIndividual>
    


    <!-- http://openenergy-platform.org/ontology/oeo/OEO_00010170 -->

    <owl:NamedIndividual rdf:about="http://openenergy-platform.org/ontology/oeo/OEO_00010170">
        <rdf:type rdf:resource="http://openenergy-platform.org/ontology/oeo/OEO_00000227"/>
        <oeo:OEO_00000504 rdf:resource="http://openenergy-platform.org/ontology/oeo/OEO_00000242"/>
        <obo:BFO_0000050 rdf:resource="http://openenergy-platform.org/ontology/oeo/OEO_00010046"/>
        <oeo:OEO_00010037>CRF 2.E</oeo:OEO_00010037>
        <oeo:OEO_00040001 rdf:datatype="http://www.w3.org/2001/XMLSchema#string">http://openenergy-platform.org/ontology/oeo/oeo-social</oeo:OEO_00040001>
        <obo:IAO_0000115>The CRF sector (IPCC 2006) &apos;electronics industry&apos; is an industry sector defined by the 2006 IPCC Guidelines for National Greenhouse Gas Inventories:
Several advanced electronics manufacturing processes utilise fluorinated compounds (FCs) for plasma etching intricate patterns, cleaning reactor chambers, and temperature control. The specific electronic industry sectors include semiconductor, thin-film-transistor flat panel display (TFT-FPD), and photovoltaic (PV) manufacturing (collectively termed ‘electronics industry’).</obo:IAO_0000115>
        <obo:IAO_0000119>2006 IPCC Guidelines for National Greenhouse Gas Inventories, Volume 3, Chapter 6.1, https://www.ipcc-nggip.iges.or.jp/public/2006gl/</obo:IAO_0000119>
        <obo:IAO_0000233>issue: https://github.com/OpenEnergyPlatform/ontology/issues/858
pull request: https://github.com/OpenEnergyPlatform/ontology/pull/941</obo:IAO_0000233>
        <rdfs:label xml:lang="en">CRF sector (IPCC 2006): electronics industry</rdfs:label>
    </owl:NamedIndividual>
    


    <!-- http://openenergy-platform.org/ontology/oeo/OEO_00010171 -->

    <owl:NamedIndividual rdf:about="http://openenergy-platform.org/ontology/oeo/OEO_00010171">
        <rdf:type rdf:resource="http://openenergy-platform.org/ontology/oeo/OEO_00000227"/>
        <oeo:OEO_00000504 rdf:resource="http://openenergy-platform.org/ontology/oeo/OEO_00000242"/>
        <obo:BFO_0000050 rdf:resource="http://openenergy-platform.org/ontology/oeo/OEO_00010046"/>
        <oeo:OEO_00010037>CRF 2.F</oeo:OEO_00010037>
        <oeo:OEO_00040001 rdf:datatype="http://www.w3.org/2001/XMLSchema#string">http://openenergy-platform.org/ontology/oeo/oeo-social</oeo:OEO_00040001>
        <obo:IAO_0000115>The CRF sector (IPCC 2006) &apos;product uses as substitutes for ozone depleting substances&apos; is an industry sector defined by the 2006 IPCC Guidelines for National Greenhouse Gas Inventories:
Hydrofluorocarbons (HFCs) and, to a very limited extent, perfluorocarbons (PFCs), are serving as alternatives to ozone depleting substances (ODS) being phased out under the Montreal Protocol.</obo:IAO_0000115>
        <obo:IAO_0000119>2006 IPCC Guidelines for National Greenhouse Gas Inventories, Volume 3, Chapter 7.1, https://www.ipcc-nggip.iges.or.jp/public/2006gl/</obo:IAO_0000119>
        <obo:IAO_0000233>issue: https://github.com/OpenEnergyPlatform/ontology/issues/858
pull request: https://github.com/OpenEnergyPlatform/ontology/pull/941</obo:IAO_0000233>
        <rdfs:label xml:lang="en">CRF sector (IPCC 2006): product uses as substitutes for ozone depleting substances</rdfs:label>
    </owl:NamedIndividual>
    


    <!-- http://openenergy-platform.org/ontology/oeo/OEO_00010172 -->

    <owl:NamedIndividual rdf:about="http://openenergy-platform.org/ontology/oeo/OEO_00010172">
        <rdf:type rdf:resource="http://openenergy-platform.org/ontology/oeo/OEO_00000227"/>
        <oeo:OEO_00000504 rdf:resource="http://openenergy-platform.org/ontology/oeo/OEO_00000242"/>
        <obo:BFO_0000050 rdf:resource="http://openenergy-platform.org/ontology/oeo/OEO_00010046"/>
        <oeo:OEO_00010037>CRF 2.G</oeo:OEO_00010037>
        <oeo:OEO_00040001 rdf:datatype="http://www.w3.org/2001/XMLSchema#string">http://openenergy-platform.org/ontology/oeo/oeo-social</oeo:OEO_00040001>
        <obo:IAO_0000115>The CRF sector (IPCC 2006) &apos;other product manufacture and use&apos; is an industry sector defined by the 2006 IPCC Guidelines for National Greenhouse Gas Inventories:
Emissions of sulphur hexafluoride (SF6) and perfluorocarbons
(PFCs) from the manufacture and use of electrical equipment and a number of other products. It also includes emissions of nitrous oxide (N2O) from several products.</obo:IAO_0000115>
        <obo:IAO_0000119>2006 IPCC Guidelines for National Greenhouse Gas Inventories, Volume 3, Chapter 8.1, https://www.ipcc-nggip.iges.or.jp/public/2006gl/</obo:IAO_0000119>
        <rdfs:label xml:lang="en">CRF sector (IPCC 2006): other product manufacture and use</rdfs:label>
    </owl:NamedIndividual>
    


    <!-- http://openenergy-platform.org/ontology/oeo/OEO_00010173 -->

    <owl:NamedIndividual rdf:about="http://openenergy-platform.org/ontology/oeo/OEO_00010173">
        <rdf:type rdf:resource="http://openenergy-platform.org/ontology/oeo/OEO_00000227"/>
        <oeo:OEO_00000504 rdf:resource="http://openenergy-platform.org/ontology/oeo/OEO_00000242"/>
        <obo:BFO_0000050 rdf:resource="http://openenergy-platform.org/ontology/oeo/OEO_00010046"/>
        <oeo:OEO_00010037>CRF 2.H</oeo:OEO_00010037>
        <oeo:OEO_00040001 rdf:datatype="http://www.w3.org/2001/XMLSchema#string">http://openenergy-platform.org/ontology/oeo/oeo-social</oeo:OEO_00040001>
        <obo:IAO_0000115>The CRF sector (IPCC 2006) &apos;industrial processes and product use - other&apos; is an industry sector defined by the 2006 IPCC Guidelines for National Greenhouse Gas Inventories</obo:IAO_0000115>
        <obo:IAO_0000233>issue: https://github.com/OpenEnergyPlatform/ontology/issues/858
pull request: https://github.com/OpenEnergyPlatform/ontology/pull/941</obo:IAO_0000233>
        <rdfs:label xml:lang="en">CRF sector (IPCC 2006): industrial processes and product use - other</rdfs:label>
    </owl:NamedIndividual>
    


    <!-- http://openenergy-platform.org/ontology/oeo/OEO_00010174 -->

    <owl:NamedIndividual rdf:about="http://openenergy-platform.org/ontology/oeo/OEO_00010174">
        <rdf:type rdf:resource="http://openenergy-platform.org/ontology/oeo/OEO_00010036"/>
        <oeo:OEO_00000504 rdf:resource="http://openenergy-platform.org/ontology/oeo/OEO_00000242"/>
        <obo:BFO_0000050 rdf:resource="http://openenergy-platform.org/ontology/oeo/OEO_00010049"/>
        <oeo:OEO_00010037>CRF 5.A</oeo:OEO_00010037>
        <oeo:OEO_00040001 rdf:datatype="http://www.w3.org/2001/XMLSchema#string">http://openenergy-platform.org/ontology/oeo/oeo-social</oeo:OEO_00040001>
        <obo:IAO_0000115>The CRF sector (IPCC 2006) &apos;solid waste disposal&apos; is a waste and wastewater sector defined by the 2006 IPCC Guidelines for National Greenhouse Gas Inventories:
Methane is produced from anaerobic microbial decomposition of organic matter in solid waste disposal sites.</obo:IAO_0000115>
        <obo:IAO_0000119>2006 IPCC Guidelines for National Greenhouse Gas Inventories, Volume 1, Chapter 8.5, https://www.ipcc-nggip.iges.or.jp/public/2006gl/</obo:IAO_0000119>
        <obo:IAO_0000233>issue: https://github.com/OpenEnergyPlatform/ontology/issues/858
pull request: https://github.com/OpenEnergyPlatform/ontology/pull/941</obo:IAO_0000233>
        <rdfs:label xml:lang="en">CRF sector (IPCC 2006): solid waste disposal</rdfs:label>
    </owl:NamedIndividual>
    


    <!-- http://openenergy-platform.org/ontology/oeo/OEO_00010175 -->

    <owl:NamedIndividual rdf:about="http://openenergy-platform.org/ontology/oeo/OEO_00010175">
        <rdf:type rdf:resource="http://openenergy-platform.org/ontology/oeo/OEO_00010036"/>
        <oeo:OEO_00000504 rdf:resource="http://openenergy-platform.org/ontology/oeo/OEO_00000242"/>
        <obo:BFO_0000050 rdf:resource="http://openenergy-platform.org/ontology/oeo/OEO_00010049"/>
        <oeo:OEO_00010037>CRF 5.B</oeo:OEO_00010037>
        <oeo:OEO_00040001 rdf:datatype="http://www.w3.org/2001/XMLSchema#string">http://openenergy-platform.org/ontology/oeo/oeo-social</oeo:OEO_00040001>
        <obo:IAO_0000115>The CRF sector (IPCC 2006) &apos;biological treatment of solid waste&apos; is a waste and wastewater sector defined by the 2006 IPCC Guidelines for National Greenhouse Gas Inventories:
Solid waste composting and other biological treatment. Emissions from biogas facilities (anaerobic digestion) with energy production are reported in the Energy Sector (1A4).</obo:IAO_0000115>
        <obo:IAO_0000119>2006 IPCC Guidelines for National Greenhouse Gas Inventories, Volume 1, Chapter 8.5, https://www.ipcc-nggip.iges.or.jp/public/2006gl/</obo:IAO_0000119>
        <obo:IAO_0000233>issue: https://github.com/OpenEnergyPlatform/ontology/issues/858
pull request: https://github.com/OpenEnergyPlatform/ontology/pull/941</obo:IAO_0000233>
        <rdfs:label xml:lang="en">CRF sector (IPCC 2006): biological treatment of solid waste</rdfs:label>
    </owl:NamedIndividual>
    


    <!-- http://openenergy-platform.org/ontology/oeo/OEO_00010176 -->

    <owl:NamedIndividual rdf:about="http://openenergy-platform.org/ontology/oeo/OEO_00010176">
        <rdf:type rdf:resource="http://openenergy-platform.org/ontology/oeo/OEO_00010036"/>
        <oeo:OEO_00000504 rdf:resource="http://openenergy-platform.org/ontology/oeo/OEO_00000242"/>
        <obo:BFO_0000050 rdf:resource="http://openenergy-platform.org/ontology/oeo/OEO_00010049"/>
        <oeo:OEO_00010037>CRF 5.C</oeo:OEO_00010037>
        <oeo:OEO_00040001 rdf:datatype="http://www.w3.org/2001/XMLSchema#string">http://openenergy-platform.org/ontology/oeo/oeo-social</oeo:OEO_00040001>
        <obo:IAO_0000115>The CRF sector (IPCC 2006) &apos;incineration and open burning of waste&apos; is a waste and wastewater sector defined by the 2006 IPCC Guidelines for National Greenhouse Gas Inventories:
Incineration of waste and open burning waste, not including waste-to-energy facilities.</obo:IAO_0000115>
        <obo:IAO_0000119>2006 IPCC Guidelines for National Greenhouse Gas Inventories, Volume 1, Chapter 8.5, https://www.ipcc-nggip.iges.or.jp/public/2006gl/</obo:IAO_0000119>
        <obo:IAO_0000233>issue: https://github.com/OpenEnergyPlatform/ontology/issues/858
pull request: https://github.com/OpenEnergyPlatform/ontology/pull/941</obo:IAO_0000233>
        <rdfs:label xml:lang="en">CRF sector (IPCC 2006): incineration and open burning of waste</rdfs:label>
    </owl:NamedIndividual>
    


    <!-- http://openenergy-platform.org/ontology/oeo/OEO_00010177 -->

    <owl:NamedIndividual rdf:about="http://openenergy-platform.org/ontology/oeo/OEO_00010177">
        <rdf:type rdf:resource="http://openenergy-platform.org/ontology/oeo/OEO_00010036"/>
        <oeo:OEO_00000504 rdf:resource="http://openenergy-platform.org/ontology/oeo/OEO_00000242"/>
        <obo:BFO_0000050 rdf:resource="http://openenergy-platform.org/ontology/oeo/OEO_00010049"/>
        <oeo:OEO_00010037>CRF 5.D</oeo:OEO_00010037>
        <oeo:OEO_00040001 rdf:datatype="http://www.w3.org/2001/XMLSchema#string">http://openenergy-platform.org/ontology/oeo/oeo-social</oeo:OEO_00040001>
        <obo:IAO_0000115>The CRF sector (IPCC 2006) &apos;waste water treatment and discharge&apos; is a waste and wastewater sector defined by the 2006 IPCC Guidelines for National Greenhouse Gas Inventories:
Methane is produced from anaerobic decomposition of organic matter by bacteria in sewage facilities and from food processing and other industrial facilities during wastewater treatment. N2O is also produced by bacteria
(denitrification and nitrification) in wastewater treatment and discharge.</obo:IAO_0000115>
        <obo:IAO_0000119>2006 IPCC Guidelines for National Greenhouse Gas Inventories, Volume 1, Chapter 8.5, https://www.ipcc-nggip.iges.or.jp/public/2006gl/</obo:IAO_0000119>
        <obo:IAO_0000233>issue: https://github.com/OpenEnergyPlatform/ontology/issues/858
pull request: https://github.com/OpenEnergyPlatform/ontology/pull/941</obo:IAO_0000233>
        <rdfs:label xml:lang="en">CRF sector (IPCC 2006): waste water treatment and discharge</rdfs:label>
    </owl:NamedIndividual>
    


    <!-- http://openenergy-platform.org/ontology/oeo/OEO_00010178 -->

    <owl:NamedIndividual rdf:about="http://openenergy-platform.org/ontology/oeo/OEO_00010178">
        <rdf:type rdf:resource="http://openenergy-platform.org/ontology/oeo/OEO_00010036"/>
        <oeo:OEO_00000504 rdf:resource="http://openenergy-platform.org/ontology/oeo/OEO_00000242"/>
        <obo:BFO_0000050 rdf:resource="http://openenergy-platform.org/ontology/oeo/OEO_00010049"/>
        <oeo:OEO_00010037>CRF 5.E</oeo:OEO_00010037>
        <oeo:OEO_00040001 rdf:datatype="http://www.w3.org/2001/XMLSchema#string">http://openenergy-platform.org/ontology/oeo/oeo-social</oeo:OEO_00040001>
        <obo:IAO_0000115>The CRF sector (IPCC 2006) &apos;waste - other&apos; is a waste and wastewater sector defined by the 2006 IPCC Guidelines for National Greenhouse Gas Inventories</obo:IAO_0000115>
        <obo:IAO_0000119>2006 IPCC Guidelines for National Greenhouse Gas Inventories, Volume 1, Chapter 8.5, https://www.ipcc-nggip.iges.or.jp/public/2006gl/</obo:IAO_0000119>
        <obo:IAO_0000233>issue: https://github.com/OpenEnergyPlatform/ontology/issues/858
pull request: https://github.com/OpenEnergyPlatform/ontology/pull/941</obo:IAO_0000233>
        <rdfs:label xml:lang="en">CRF sector (IPCC 2006): waste - other</rdfs:label>
    </owl:NamedIndividual>
    


    <!-- http://openenergy-platform.org/ontology/oeo/OEO_00010179 -->

    <owl:NamedIndividual rdf:about="http://openenergy-platform.org/ontology/oeo/OEO_00010179">
        <rdf:type rdf:resource="http://openenergy-platform.org/ontology/oeo/OEO_00010035"/>
        <oeo:OEO_00000504 rdf:resource="http://openenergy-platform.org/ontology/oeo/OEO_00000242"/>
        <obo:BFO_0000050 rdf:resource="http://openenergy-platform.org/ontology/oeo/OEO_00010047"/>
        <oeo:OEO_00010037>CRF 3.A</oeo:OEO_00010037>
        <oeo:OEO_00040001 rdf:datatype="http://www.w3.org/2001/XMLSchema#string">http://openenergy-platform.org/ontology/oeo/oeo-social</oeo:OEO_00040001>
        <obo:IAO_0000115>The CRF sector (IPCC 2006) &apos;enteric fermentation&apos; is an agriculture, forestry and land use sector defined by the 2006 IPCC Guidelines for National Greenhouse Gas Inventories:
Methane emissions from herbivores as a by-product of enteric fermentation (a digestive process by which carbohydrates are broken down by micro-organisms into simple molecules for absorption into the bloodstream). Ruminant animals (e.g., cattle, sheep) are major sources with moderate amounts produced from non-ruminant animals (e.g., pigs, horses).</obo:IAO_0000115>
        <obo:IAO_0000119>2006 IPCC Guidelines for National Greenhouse Gas Inventories, Volume 1, Chapter 8.5, https://www.ipcc-nggip.iges.or.jp/public/2006gl/</obo:IAO_0000119>
        <obo:IAO_0000233>issue: https://github.com/OpenEnergyPlatform/ontology/issues/858
pull request: https://github.com/OpenEnergyPlatform/ontology/pull/941</obo:IAO_0000233>
        <rdfs:label xml:lang="en">CRF sector (IPCC 2006): enteric fermentation</rdfs:label>
    </owl:NamedIndividual>
    


    <!-- http://openenergy-platform.org/ontology/oeo/OEO_00010180 -->

    <owl:NamedIndividual rdf:about="http://openenergy-platform.org/ontology/oeo/OEO_00010180">
        <rdf:type rdf:resource="http://openenergy-platform.org/ontology/oeo/OEO_00010035"/>
        <oeo:OEO_00000504 rdf:resource="http://openenergy-platform.org/ontology/oeo/OEO_00000242"/>
        <obo:BFO_0000050 rdf:resource="http://openenergy-platform.org/ontology/oeo/OEO_00010047"/>
        <oeo:OEO_00010037>CRF 3.B</oeo:OEO_00010037>
        <oeo:OEO_00040001 rdf:datatype="http://www.w3.org/2001/XMLSchema#string">http://openenergy-platform.org/ontology/oeo/oeo-social</oeo:OEO_00040001>
        <obo:IAO_0000115>The CRF sector (IPCC 2006) &apos;manure management&apos; is an agriculture, forestry and land use sector defined by the 2006 IPCC Guidelines for National Greenhouse Gas Inventories:
Methane and nitrous oxide emissions from the decomposition of manure under low oxygen or anaerobic conditions.</obo:IAO_0000115>
        <obo:IAO_0000119>2006 IPCC Guidelines for National Greenhouse Gas Inventories, Volume 1, Chapter 8.5, https://www.ipcc-nggip.iges.or.jp/public/2006gl/</obo:IAO_0000119>
        <obo:IAO_0000233>issue: https://github.com/OpenEnergyPlatform/ontology/issues/858
pull request: https://github.com/OpenEnergyPlatform/ontology/pull/941</obo:IAO_0000233>
        <rdfs:label xml:lang="en">CRF sector (IPCC 2006): manure management</rdfs:label>
    </owl:NamedIndividual>
    


    <!-- http://openenergy-platform.org/ontology/oeo/OEO_00010181 -->

    <owl:NamedIndividual rdf:about="http://openenergy-platform.org/ontology/oeo/OEO_00010181">
        <rdf:type rdf:resource="http://openenergy-platform.org/ontology/oeo/OEO_00010035"/>
        <oeo:OEO_00000504 rdf:resource="http://openenergy-platform.org/ontology/oeo/OEO_00000242"/>
        <obo:BFO_0000050 rdf:resource="http://openenergy-platform.org/ontology/oeo/OEO_00010047"/>
        <oeo:OEO_00010037>CRF 3.C</oeo:OEO_00010037>
        <oeo:OEO_00040001 rdf:datatype="http://www.w3.org/2001/XMLSchema#string">http://openenergy-platform.org/ontology/oeo/oeo-social</oeo:OEO_00040001>
        <obo:IAO_0000115>The CRF sector (IPCC 2006) &apos;rice cultivation&apos; is an agriculture, forestry and land use sector defined by the 2006 IPCC Guidelines for National Greenhouse Gas Inventories:
Methane (CH4) emissions from anaerobic decomposition of organic material in flooded rice fields.</obo:IAO_0000115>
        <obo:IAO_0000119>2006 IPCC Guidelines for National Greenhouse Gas Inventories, Volume 1, Chapter 8.5, https://www.ipcc-nggip.iges.or.jp/public/2006gl/</obo:IAO_0000119>
        <obo:IAO_0000233>issue: https://github.com/OpenEnergyPlatform/ontology/issues/858
pull request: https://github.com/OpenEnergyPlatform/ontology/pull/941</obo:IAO_0000233>
        <rdfs:label xml:lang="en">CRF sector (IPCC 2006): rice cultivation</rdfs:label>
    </owl:NamedIndividual>
    


    <!-- http://openenergy-platform.org/ontology/oeo/OEO_00010182 -->

    <owl:NamedIndividual rdf:about="http://openenergy-platform.org/ontology/oeo/OEO_00010182">
        <rdf:type rdf:resource="http://openenergy-platform.org/ontology/oeo/OEO_00010035"/>
        <oeo:OEO_00000504 rdf:resource="http://openenergy-platform.org/ontology/oeo/OEO_00000242"/>
        <obo:BFO_0000050 rdf:resource="http://openenergy-platform.org/ontology/oeo/OEO_00010047"/>
        <oeo:OEO_00010037>CRF 3.D</oeo:OEO_00010037>
        <oeo:OEO_00040001 rdf:datatype="http://www.w3.org/2001/XMLSchema#string">http://openenergy-platform.org/ontology/oeo/oeo-social</oeo:OEO_00040001>
        <obo:IAO_0000115>The CRF sector (IPCC 2006) &apos;agricultural soils&apos; is an agriculture, forestry and land use sector defined by the 2006 IPCC Guidelines for National Greenhouse Gas Inventories</obo:IAO_0000115>
        <obo:IAO_0000233>issue: https://github.com/OpenEnergyPlatform/ontology/issues/858
pull request: https://github.com/OpenEnergyPlatform/ontology/pull/941</obo:IAO_0000233>
        <rdfs:label xml:lang="en">CRF sector (IPCC 2006): agricultural soils</rdfs:label>
    </owl:NamedIndividual>
    


    <!-- http://openenergy-platform.org/ontology/oeo/OEO_00010183 -->

    <owl:NamedIndividual rdf:about="http://openenergy-platform.org/ontology/oeo/OEO_00010183">
        <rdf:type rdf:resource="http://openenergy-platform.org/ontology/oeo/OEO_00010035"/>
        <oeo:OEO_00000504 rdf:resource="http://openenergy-platform.org/ontology/oeo/OEO_00000242"/>
        <obo:BFO_0000050 rdf:resource="http://openenergy-platform.org/ontology/oeo/OEO_00010047"/>
        <oeo:OEO_00010037>CRF 3.E</oeo:OEO_00010037>
        <oeo:OEO_00040001 rdf:datatype="http://www.w3.org/2001/XMLSchema#string">http://openenergy-platform.org/ontology/oeo/oeo-social</oeo:OEO_00040001>
        <obo:IAO_0000115>The CRF sector (IPCC 2006) &apos;prescribed burning of savannas&apos; is an agriculture, forestry and land use sector defined by the 2006 IPCC Guidelines for National Greenhouse Gas Inventories</obo:IAO_0000115>
        <obo:IAO_0000233>issue: https://github.com/OpenEnergyPlatform/ontology/issues/858
pull request: https://github.com/OpenEnergyPlatform/ontology/pull/941</obo:IAO_0000233>
        <rdfs:label xml:lang="en">CRF sector (IPCC 2006): prescribed burning of savannas</rdfs:label>
    </owl:NamedIndividual>
    


    <!-- http://openenergy-platform.org/ontology/oeo/OEO_00010184 -->

    <owl:NamedIndividual rdf:about="http://openenergy-platform.org/ontology/oeo/OEO_00010184">
        <rdf:type rdf:resource="http://openenergy-platform.org/ontology/oeo/OEO_00010035"/>
        <oeo:OEO_00000504 rdf:resource="http://openenergy-platform.org/ontology/oeo/OEO_00000242"/>
        <obo:BFO_0000050 rdf:resource="http://openenergy-platform.org/ontology/oeo/OEO_00010047"/>
        <oeo:OEO_00010037>CRF 3.F</oeo:OEO_00010037>
        <oeo:OEO_00040001 rdf:datatype="http://www.w3.org/2001/XMLSchema#string">http://openenergy-platform.org/ontology/oeo/oeo-social</oeo:OEO_00040001>
        <obo:IAO_0000115>The CRF sector (IPCC 2006) &apos;field burning of agricultural residues&apos; is an agriculture, forestry and land use sector defined by the 2006 IPCC Guidelines for National Greenhouse Gas Inventories:
CO2 emissions from urea application</obo:IAO_0000115>
        <obo:IAO_0000119>2006 IPCC Guidelines for National Greenhouse Gas Inventories, Volume 1, Chapter 8.5, https://www.ipcc-nggip.iges.or.jp/public/2006gl/</obo:IAO_0000119>
        <obo:IAO_0000233>issue: https://github.com/OpenEnergyPlatform/ontology/issues/858
pull request: https://github.com/OpenEnergyPlatform/ontology/pull/941</obo:IAO_0000233>
        <rdfs:label xml:lang="en">CRF sector (IPCC 2006): field burning of agricultural residues</rdfs:label>
    </owl:NamedIndividual>
    


    <!-- http://openenergy-platform.org/ontology/oeo/OEO_00010185 -->

    <owl:NamedIndividual rdf:about="http://openenergy-platform.org/ontology/oeo/OEO_00010185">
        <rdf:type rdf:resource="http://openenergy-platform.org/ontology/oeo/OEO_00010035"/>
        <oeo:OEO_00000504 rdf:resource="http://openenergy-platform.org/ontology/oeo/OEO_00000242"/>
        <obo:BFO_0000050 rdf:resource="http://openenergy-platform.org/ontology/oeo/OEO_00010047"/>
        <oeo:OEO_00010037>CRF 3.G</oeo:OEO_00010037>
        <oeo:OEO_00040001 rdf:datatype="http://www.w3.org/2001/XMLSchema#string">http://openenergy-platform.org/ontology/oeo/oeo-social</oeo:OEO_00040001>
        <obo:IAO_0000115>The CRF sector (IPCC 2006) &apos;liming&apos; is an agriculture, forestry and land use sector defined by the 2006 IPCC Guidelines for National Greenhouse Gas Inventories:
CO2 emissions from the use of lime in agricultural soils, managed forest soils or lakes.</obo:IAO_0000115>
        <obo:IAO_0000119>2006 IPCC Guidelines for National Greenhouse Gas Inventories, Volume 1, Chapter 8.5, https://www.ipcc-nggip.iges.or.jp/public/2006gl/</obo:IAO_0000119>
        <obo:IAO_0000233>issue: https://github.com/OpenEnergyPlatform/ontology/issues/858
pull request: https://github.com/OpenEnergyPlatform/ontology/pull/941</obo:IAO_0000233>
        <rdfs:label xml:lang="en">CRF sector (IPCC 2006): liming</rdfs:label>
    </owl:NamedIndividual>
    


    <!-- http://openenergy-platform.org/ontology/oeo/OEO_00010186 -->

    <owl:NamedIndividual rdf:about="http://openenergy-platform.org/ontology/oeo/OEO_00010186">
        <rdf:type rdf:resource="http://openenergy-platform.org/ontology/oeo/OEO_00010035"/>
        <oeo:OEO_00000504 rdf:resource="http://openenergy-platform.org/ontology/oeo/OEO_00000242"/>
        <obo:BFO_0000050 rdf:resource="http://openenergy-platform.org/ontology/oeo/OEO_00010047"/>
        <oeo:OEO_00010037>CRF 3.H</oeo:OEO_00010037>
        <oeo:OEO_00040001 rdf:datatype="http://www.w3.org/2001/XMLSchema#string">http://openenergy-platform.org/ontology/oeo/oeo-social</oeo:OEO_00040001>
        <obo:IAO_0000115>The CRF sector (IPCC 2006) &apos;urea application&apos; is an agriculture, forestry and land use sector defined by the 2006 IPCC Guidelines for National Greenhouse Gas Inventories</obo:IAO_0000115>
        <obo:IAO_0000233>issue: https://github.com/OpenEnergyPlatform/ontology/issues/858
pull request: https://github.com/OpenEnergyPlatform/ontology/pull/941</obo:IAO_0000233>
        <rdfs:label xml:lang="en">CRF sector (IPCC 2006): urea application</rdfs:label>
    </owl:NamedIndividual>
    


    <!-- http://openenergy-platform.org/ontology/oeo/OEO_00010187 -->

    <owl:NamedIndividual rdf:about="http://openenergy-platform.org/ontology/oeo/OEO_00010187">
        <rdf:type rdf:resource="http://openenergy-platform.org/ontology/oeo/OEO_00010035"/>
        <oeo:OEO_00000504 rdf:resource="http://openenergy-platform.org/ontology/oeo/OEO_00000242"/>
        <obo:BFO_0000050 rdf:resource="http://openenergy-platform.org/ontology/oeo/OEO_00010047"/>
        <oeo:OEO_00010037>CRF 3.I</oeo:OEO_00010037>
        <oeo:OEO_00040001 rdf:datatype="http://www.w3.org/2001/XMLSchema#string">http://openenergy-platform.org/ontology/oeo/oeo-social</oeo:OEO_00040001>
        <obo:IAO_0000115>The CRF sector (IPCC 2006) &apos;other carbon-containing fertilizers&apos; is an agriculture, forestry and land use sector defined by the 2006 IPCC Guidelines for National Greenhouse Gas Inventories</obo:IAO_0000115>
        <obo:IAO_0000233>issue: https://github.com/OpenEnergyPlatform/ontology/issues/858
pull request: https://github.com/OpenEnergyPlatform/ontology/pull/941</obo:IAO_0000233>
        <rdfs:label xml:lang="en">CRF sector (IPCC 2006): other carbon-containing fertilizers</rdfs:label>
    </owl:NamedIndividual>
    


    <!-- http://openenergy-platform.org/ontology/oeo/OEO_00010188 -->

    <owl:NamedIndividual rdf:about="http://openenergy-platform.org/ontology/oeo/OEO_00010188">
        <rdf:type rdf:resource="http://openenergy-platform.org/ontology/oeo/OEO_00010035"/>
        <oeo:OEO_00000504 rdf:resource="http://openenergy-platform.org/ontology/oeo/OEO_00000242"/>
        <obo:BFO_0000050 rdf:resource="http://openenergy-platform.org/ontology/oeo/OEO_00010047"/>
        <oeo:OEO_00010037>CRF 3.J</oeo:OEO_00010037>
        <oeo:OEO_00040001 rdf:datatype="http://www.w3.org/2001/XMLSchema#string">http://openenergy-platform.org/ontology/oeo/oeo-social</oeo:OEO_00040001>
        <obo:IAO_0000115>The CRF sector (IPCC 2006) &apos;agriculture - other&apos; is an agriculture, forestry and land use sector defined by the 2006 IPCC Guidelines for National Greenhouse Gas Inventories</obo:IAO_0000115>
        <obo:IAO_0000233>issue: https://github.com/OpenEnergyPlatform/ontology/issues/858
pull request: https://github.com/OpenEnergyPlatform/ontology/pull/941</obo:IAO_0000233>
        <rdfs:label xml:lang="en">CRF sector (IPCC 2006): agriculture - other</rdfs:label>
    </owl:NamedIndividual>
    


    <!-- http://openenergy-platform.org/ontology/oeo/OEO_00010189 -->

    <owl:NamedIndividual rdf:about="http://openenergy-platform.org/ontology/oeo/OEO_00010189">
        <rdf:type rdf:resource="http://openenergy-platform.org/ontology/oeo/OEO_00010035"/>
        <oeo:OEO_00000504 rdf:resource="http://openenergy-platform.org/ontology/oeo/OEO_00000242"/>
        <obo:BFO_0000050 rdf:resource="http://openenergy-platform.org/ontology/oeo/OEO_00010048"/>
        <oeo:OEO_00010037>CRF 4.A</oeo:OEO_00010037>
        <oeo:OEO_00040001 rdf:datatype="http://www.w3.org/2001/XMLSchema#string">http://openenergy-platform.org/ontology/oeo/oeo-social</oeo:OEO_00040001>
        <obo:IAO_0000115>The CRF sector (IPCC 2006) &apos;forest land&apos; is an agriculture, forestry and land use sector defined by the 2006 IPCC Guidelines for National Greenhouse Gas Inventories:
Emissions and removals from lands with woody vegetation consistent with thresholds used to define forest land in the national GHG inventory, sub-divided into managed and unmanaged, and possibly also by climatic region, soil type and vegetation type as appropriate. It also includes systems with vegetation that currently fall below, but are expected to later exceed, the threshold values used by a country to define the forest land category.</obo:IAO_0000115>
        <obo:IAO_0000119>2006 IPCC Guidelines for National Greenhouse Gas Inventories, Volume 1, Chapter 8.5, https://www.ipcc-nggip.iges.or.jp/public/2006gl/</obo:IAO_0000119>
        <obo:IAO_0000233>issue: https://github.com/OpenEnergyPlatform/ontology/issues/858
pull request: https://github.com/OpenEnergyPlatform/ontology/pull/941</obo:IAO_0000233>
        <rdfs:label xml:lang="en">CRF sector (IPCC 2006): forest land</rdfs:label>
    </owl:NamedIndividual>
    


    <!-- http://openenergy-platform.org/ontology/oeo/OEO_00010190 -->

    <owl:NamedIndividual rdf:about="http://openenergy-platform.org/ontology/oeo/OEO_00010190">
        <rdf:type rdf:resource="http://openenergy-platform.org/ontology/oeo/OEO_00010035"/>
        <oeo:OEO_00000504 rdf:resource="http://openenergy-platform.org/ontology/oeo/OEO_00000242"/>
        <obo:BFO_0000050 rdf:resource="http://openenergy-platform.org/ontology/oeo/OEO_00010048"/>
        <oeo:OEO_00010037>CRF 4.B</oeo:OEO_00010037>
        <oeo:OEO_00040001 rdf:datatype="http://www.w3.org/2001/XMLSchema#string">http://openenergy-platform.org/ontology/oeo/oeo-social</oeo:OEO_00040001>
        <obo:IAO_0000115>The CRF sector (IPCC 2006) &apos;cropland&apos; is an agriculture, forestry and land use sector defined by the 2006 IPCC Guidelines for National Greenhouse Gas Inventories:
Emissions and removals from arable and tillage land, rice fields, and agro-forestry systems where vegetation falls below the thresholds used for the forest land category.</obo:IAO_0000115>
        <obo:IAO_0000119>2006 IPCC Guidelines for National Greenhouse Gas Inventories, Volume 1, Chapter 8.5, https://www.ipcc-nggip.iges.or.jp/public/2006gl/</obo:IAO_0000119>
        <obo:IAO_0000233>issue: https://github.com/OpenEnergyPlatform/ontology/issues/858
pull request: https://github.com/OpenEnergyPlatform/ontology/pull/941</obo:IAO_0000233>
        <rdfs:label xml:lang="en">CRF sector (IPCC 2006): cropland</rdfs:label>
    </owl:NamedIndividual>
    


    <!-- http://openenergy-platform.org/ontology/oeo/OEO_00010191 -->

    <owl:NamedIndividual rdf:about="http://openenergy-platform.org/ontology/oeo/OEO_00010191">
        <rdf:type rdf:resource="http://openenergy-platform.org/ontology/oeo/OEO_00010035"/>
        <oeo:OEO_00000504 rdf:resource="http://openenergy-platform.org/ontology/oeo/OEO_00000242"/>
        <obo:BFO_0000050 rdf:resource="http://openenergy-platform.org/ontology/oeo/OEO_00010048"/>
        <oeo:OEO_00010037>CRF 4.C</oeo:OEO_00010037>
        <oeo:OEO_00040001 rdf:datatype="http://www.w3.org/2001/XMLSchema#string">http://openenergy-platform.org/ontology/oeo/oeo-social</oeo:OEO_00040001>
        <obo:IAO_0000115>The CRF sector (IPCC 2006) &apos;grassland&apos; is an agriculture, forestry and land use sector defined by the 2006 IPCC Guidelines for National Greenhouse Gas Inventories:
Emissions and removals from rangelands and pasture land that is not considered cropland. It also includes systems with woody vegetation that fall below the threshold values used in the forest land category and are not expected to exceed them, without human intervention. The category also includes all grassland from wild lands to recreational areas as well as agricultural and silvi-pastural systems, subdivided into managed and unmanaged, consistent with national definitions.</obo:IAO_0000115>
        <obo:IAO_0000119>2006 IPCC Guidelines for National Greenhouse Gas Inventories, Volume 1, Chapter 8.5, https://www.ipcc-nggip.iges.or.jp/public/2006gl/</obo:IAO_0000119>
        <obo:IAO_0000233>issue: https://github.com/OpenEnergyPlatform/ontology/issues/858
pull request: https://github.com/OpenEnergyPlatform/ontology/pull/941</obo:IAO_0000233>
        <rdfs:label xml:lang="en">CRF sector (IPCC 2006): grassland</rdfs:label>
    </owl:NamedIndividual>
    


    <!-- http://openenergy-platform.org/ontology/oeo/OEO_00010192 -->

    <owl:NamedIndividual rdf:about="http://openenergy-platform.org/ontology/oeo/OEO_00010192">
        <rdf:type rdf:resource="http://openenergy-platform.org/ontology/oeo/OEO_00010035"/>
        <oeo:OEO_00000504 rdf:resource="http://openenergy-platform.org/ontology/oeo/OEO_00000242"/>
        <obo:BFO_0000050 rdf:resource="http://openenergy-platform.org/ontology/oeo/OEO_00010048"/>
        <oeo:OEO_00010037>CRF 4.D</oeo:OEO_00010037>
        <oeo:OEO_00040001 rdf:datatype="http://www.w3.org/2001/XMLSchema#string">http://openenergy-platform.org/ontology/oeo/oeo-social</oeo:OEO_00040001>
        <obo:IAO_0000115>The CRF sector (IPCC 2006) &apos;wetlands&apos; is an agriculture, forestry and land use sector defined by the 2006 IPCC Guidelines for National Greenhouse Gas Inventories:
Emissions from land that is covered or saturated by water for all or part of the year (e.g., peatland) and that does not fall into the forest land, cropland, grassland or settlements categories. The category can be subdivided into managed and unmanaged according to national definitions. It includes reservoirs as a managed sub-division and natural rivers and lakes as unmanaged sub-divisions.</obo:IAO_0000115>
        <obo:IAO_0000119>2006 IPCC Guidelines for National Greenhouse Gas Inventories, Volume 1, Chapter 8.5, https://www.ipcc-nggip.iges.or.jp/public/2006gl/</obo:IAO_0000119>
        <obo:IAO_0000233>issue: https://github.com/OpenEnergyPlatform/ontology/issues/858
pull request: https://github.com/OpenEnergyPlatform/ontology/pull/941</obo:IAO_0000233>
        <rdfs:label xml:lang="en">CRF sector (IPCC 2006): wetlands</rdfs:label>
    </owl:NamedIndividual>
    


    <!-- http://openenergy-platform.org/ontology/oeo/OEO_00010193 -->

    <owl:NamedIndividual rdf:about="http://openenergy-platform.org/ontology/oeo/OEO_00010193">
        <rdf:type rdf:resource="http://openenergy-platform.org/ontology/oeo/OEO_00010035"/>
        <oeo:OEO_00000504 rdf:resource="http://openenergy-platform.org/ontology/oeo/OEO_00000242"/>
        <obo:BFO_0000050 rdf:resource="http://openenergy-platform.org/ontology/oeo/OEO_00010048"/>
        <oeo:OEO_00010037>CRF 4.E</oeo:OEO_00010037>
        <oeo:OEO_00040001 rdf:datatype="http://www.w3.org/2001/XMLSchema#string">http://openenergy-platform.org/ontology/oeo/oeo-social</oeo:OEO_00040001>
        <obo:IAO_0000115>The CRF sector (IPCC 2006) &apos;settlements&apos; is an agriculture, forestry and land use sector defined by the 2006 IPCC Guidelines for National Greenhouse Gas Inventories:
Emissions and removals from all developed land, including transportation infrastructure and human settlements of any size, unless they are already included under other categories.</obo:IAO_0000115>
        <obo:IAO_0000119>2006 IPCC Guidelines for National Greenhouse Gas Inventories, Volume 1, Chapter 8.5, https://www.ipcc-nggip.iges.or.jp/public/2006gl/</obo:IAO_0000119>
        <obo:IAO_0000233>issue: https://github.com/OpenEnergyPlatform/ontology/issues/858
pull request: https://github.com/OpenEnergyPlatform/ontology/pull/941</obo:IAO_0000233>
        <rdfs:label xml:lang="en">CRF sector (IPCC 2006): settlements</rdfs:label>
    </owl:NamedIndividual>
    


    <!-- http://openenergy-platform.org/ontology/oeo/OEO_00010194 -->

    <owl:NamedIndividual rdf:about="http://openenergy-platform.org/ontology/oeo/OEO_00010194">
        <rdf:type rdf:resource="http://openenergy-platform.org/ontology/oeo/OEO_00010035"/>
        <oeo:OEO_00000504 rdf:resource="http://openenergy-platform.org/ontology/oeo/OEO_00000242"/>
        <obo:BFO_0000050 rdf:resource="http://openenergy-platform.org/ontology/oeo/OEO_00010048"/>
        <oeo:OEO_00010037>CRF 4.F</oeo:OEO_00010037>
        <oeo:OEO_00040001 rdf:datatype="http://www.w3.org/2001/XMLSchema#string">http://openenergy-platform.org/ontology/oeo/oeo-social</oeo:OEO_00040001>
        <obo:IAO_0000115>The CRF sector (IPCC 2006) &apos;other land&apos; is an agriculture, forestry and land use sector defined by the 2006 IPCC Guidelines for National Greenhouse Gas Inventories:
Emissions and removals from bare soil, rock, ice, and all unmanaged land areas that do not fall into any of the other five categories.</obo:IAO_0000115>
        <obo:IAO_0000119>2006 IPCC Guidelines for National Greenhouse Gas Inventories, Volume 1, Chapter 8.5, https://www.ipcc-nggip.iges.or.jp/public/2006gl/</obo:IAO_0000119>
        <obo:IAO_0000233>issue: https://github.com/OpenEnergyPlatform/ontology/issues/858
pull request: https://github.com/OpenEnergyPlatform/ontology/pull/941</obo:IAO_0000233>
        <rdfs:label xml:lang="en">CRF sector (IPCC 2006): other land</rdfs:label>
    </owl:NamedIndividual>
    


    <!-- http://openenergy-platform.org/ontology/oeo/OEO_00010195 -->

    <owl:NamedIndividual rdf:about="http://openenergy-platform.org/ontology/oeo/OEO_00010195">
        <rdf:type rdf:resource="http://openenergy-platform.org/ontology/oeo/OEO_00010035"/>
        <oeo:OEO_00000504 rdf:resource="http://openenergy-platform.org/ontology/oeo/OEO_00000242"/>
        <obo:BFO_0000050 rdf:resource="http://openenergy-platform.org/ontology/oeo/OEO_00010048"/>
        <oeo:OEO_00010037>CRF 4.G</oeo:OEO_00010037>
        <oeo:OEO_00040001 rdf:datatype="http://www.w3.org/2001/XMLSchema#string">http://openenergy-platform.org/ontology/oeo/oeo-social</oeo:OEO_00040001>
        <obo:IAO_0000115>The CRF sector (IPCC 2006) &apos;harvested wood products&apos; is an agriculture, forestry and land use sector defined by the 2006 IPCC Guidelines for National Greenhouse Gas Inventories
CO2 net emissions or removals resulting from Harvest Wood Products.</obo:IAO_0000115>
        <obo:IAO_0000119>2006 IPCC Guidelines for National Greenhouse Gas Inventories, Volume 1, Chapter 8.5, https://www.ipcc-nggip.iges.or.jp/public/2006gl/</obo:IAO_0000119>
        <obo:IAO_0000233>issue: https://github.com/OpenEnergyPlatform/ontology/issues/858
pull request: https://github.com/OpenEnergyPlatform/ontology/pull/941</obo:IAO_0000233>
        <rdfs:label xml:lang="en">CRF sector (IPCC 2006): harvested wood products</rdfs:label>
    </owl:NamedIndividual>
    


    <!-- http://openenergy-platform.org/ontology/oeo/OEO_00010196 -->

    <owl:NamedIndividual rdf:about="http://openenergy-platform.org/ontology/oeo/OEO_00010196">
        <rdf:type rdf:resource="http://openenergy-platform.org/ontology/oeo/OEO_00010035"/>
        <oeo:OEO_00000504 rdf:resource="http://openenergy-platform.org/ontology/oeo/OEO_00000242"/>
        <obo:BFO_0000050 rdf:resource="http://openenergy-platform.org/ontology/oeo/OEO_00010048"/>
        <oeo:OEO_00010037>CRF 4.H</oeo:OEO_00010037>
        <oeo:OEO_00040001 rdf:datatype="http://www.w3.org/2001/XMLSchema#string">http://openenergy-platform.org/ontology/oeo/oeo-social</oeo:OEO_00040001>
        <obo:IAO_0000115>The CRF sector (IPCC 2006) &apos;land use, land-use change and forestry - other&apos; is an agriculture, forestry and land use sector defined by the 2006 IPCC Guidelines for National Greenhouse Gas Inventories</obo:IAO_0000115>
        <obo:IAO_0000233>issue: https://github.com/OpenEnergyPlatform/ontology/issues/858
pull request: https://github.com/OpenEnergyPlatform/ontology/pull/941</obo:IAO_0000233>
        <rdfs:label xml:lang="en">CRF sector (IPCC 2006): land use, land-use change and forestry - other</rdfs:label>
    </owl:NamedIndividual>
    


    <!-- http://openenergy-platform.org/ontology/oeo/OEO_00010197 -->

    <owl:NamedIndividual rdf:about="http://openenergy-platform.org/ontology/oeo/OEO_00010197">
        <rdf:type rdf:resource="http://openenergy-platform.org/ontology/oeo/OEO_00000367"/>
        <oeo:OEO_00000504 rdf:resource="http://openenergy-platform.org/ontology/oeo/OEO_00000242"/>
        <obo:BFO_0000051 rdf:resource="http://openenergy-platform.org/ontology/oeo/OEO_00010038"/>
        <obo:BFO_0000051 rdf:resource="http://openenergy-platform.org/ontology/oeo/OEO_00010046"/>
        <obo:BFO_0000051 rdf:resource="http://openenergy-platform.org/ontology/oeo/OEO_00010047"/>
        <obo:BFO_0000051 rdf:resource="http://openenergy-platform.org/ontology/oeo/OEO_00010049"/>
        <obo:BFO_0000051 rdf:resource="http://openenergy-platform.org/ontology/oeo/OEO_00010050"/>
        <oeo:OEO_00040001 rdf:datatype="http://www.w3.org/2001/XMLSchema#string">http://openenergy-platform.org/ontology/oeo/oeo-social</oeo:OEO_00040001>
        <obo:IAO_0000115>The CRF sector (IPCC 2006) &apos;total emissions excluding LULUCF&apos; is a sector defined by the 2006 IPCC Guidelines for National Greenhouse Gas Inventories. It encompasses the following IPCC 2006 sectors: energy; industrial processes and product use; agriculture; waste; and other.</obo:IAO_0000115>
        <obo:IAO_0000118>Total emissions: (UNFCCC)</obo:IAO_0000118>
        <obo:IAO_0000233>issue: https://github.com/OpenEnergyPlatform/ontology/issues/928
pull request: https://github.com/OpenEnergyPlatform/ontology/pull/944</obo:IAO_0000233>
        <rdfs:label xml:lang="en">CRF sector (IPCC 2006): total emissions excluding LULUCF</rdfs:label>
    </owl:NamedIndividual>
    <owl:Axiom>
        <owl:annotatedSource rdf:resource="http://openenergy-platform.org/ontology/oeo/OEO_00010197"/>
        <owl:annotatedProperty rdf:resource="http://purl.obolibrary.org/obo/IAO_0000118"/>
        <owl:annotatedTarget>Total emissions: (UNFCCC)</owl:annotatedTarget>
        <obo:IAO_0000116>Term used by the European Environment Agency (EEA) https://climate-energy.eea.europa.eu/topics/climate-change-mitigation/greenhouse-gas-emissions-inventory/data</obo:IAO_0000116>
    </owl:Axiom>
    


    <!-- http://openenergy-platform.org/ontology/oeo/OEO_00010198 -->

    <owl:NamedIndividual rdf:about="http://openenergy-platform.org/ontology/oeo/OEO_00010198">
        <rdf:type rdf:resource="http://openenergy-platform.org/ontology/oeo/OEO_00000367"/>
        <oeo:OEO_00000504 rdf:resource="http://openenergy-platform.org/ontology/oeo/OEO_00000242"/>
        <obo:BFO_0000051 rdf:resource="http://openenergy-platform.org/ontology/oeo/OEO_00010038"/>
        <obo:BFO_0000051 rdf:resource="http://openenergy-platform.org/ontology/oeo/OEO_00010046"/>
        <obo:BFO_0000051 rdf:resource="http://openenergy-platform.org/ontology/oeo/OEO_00010047"/>
        <obo:BFO_0000051 rdf:resource="http://openenergy-platform.org/ontology/oeo/OEO_00010048"/>
        <obo:BFO_0000051 rdf:resource="http://openenergy-platform.org/ontology/oeo/OEO_00010049"/>
        <obo:BFO_0000051 rdf:resource="http://openenergy-platform.org/ontology/oeo/OEO_00010050"/>
        <oeo:OEO_00040001 rdf:datatype="http://www.w3.org/2001/XMLSchema#string">http://openenergy-platform.org/ontology/oeo/oeo-social</oeo:OEO_00040001>
        <obo:IAO_0000115>The CRF sector (IPCC 2006) &apos;total emissions including LULUCF&apos; is a sector defined by the 2006 IPCC Guidelines for National Greenhouse Gas Inventories. It encompasses the following IPCC 2006 sectors: energy; industrial processes and product use; agriculture; land use, land-use change and forestry; waste; and other.</obo:IAO_0000115>
        <obo:IAO_0000118>Total net emissions (UNFCCC)</obo:IAO_0000118>
        <obo:IAO_0000233>issue: https://github.com/OpenEnergyPlatform/ontology/issues/928
pull request: https://github.com/OpenEnergyPlatform/ontology/pull/944</obo:IAO_0000233>
        <rdfs:label xml:lang="en">CRF sector (IPCC 2006): total emissions including LULUCF</rdfs:label>
    </owl:NamedIndividual>
    <owl:Axiom>
        <owl:annotatedSource rdf:resource="http://openenergy-platform.org/ontology/oeo/OEO_00010198"/>
        <owl:annotatedProperty rdf:resource="http://purl.obolibrary.org/obo/IAO_0000118"/>
        <owl:annotatedTarget>Total net emissions (UNFCCC)</owl:annotatedTarget>
        <obo:IAO_0000116>Term used by the European Environment Agency (EEA): https://climate-energy.eea.europa.eu/topics/climate-change-mitigation/greenhouse-gas-emissions-inventory/data</obo:IAO_0000116>
    </owl:Axiom>
    


    <!-- http://openenergy-platform.org/ontology/oeo/OEO_00010199 -->

    <owl:NamedIndividual rdf:about="http://openenergy-platform.org/ontology/oeo/OEO_00010199">
        <rdf:type rdf:resource="http://openenergy-platform.org/ontology/oeo/OEO_00000422"/>
        <rdf:type>
            <owl:Restriction>
                <owl:onProperty rdf:resource="http://openenergy-platform.org/ontology/oeo/OEO_00010232"/>
                <owl:someValuesFrom rdf:resource="http://openenergy-platform.org/ontology/oeo/OEO_00010227"/>
            </owl:Restriction>
        </rdf:type>
        <rdf:type>
            <owl:Restriction>
                <owl:onProperty rdf:resource="http://openenergy-platform.org/ontology/oeo/OEO_00010232"/>
                <owl:someValuesFrom rdf:resource="http://openenergy-platform.org/ontology/oeo/OEO_00010227"/>
            </owl:Restriction>
        </rdf:type>
        <oeo:OEO_00000504 rdf:resource="http://openenergy-platform.org/ontology/oeo/OEO_00000242"/>
        <obo:BFO_0000051 rdf:resource="http://openenergy-platform.org/ontology/oeo/OEO_00010200"/>
        <obo:BFO_0000051 rdf:resource="http://openenergy-platform.org/ontology/oeo/OEO_00010203"/>
        <oeo:OEO_00010037>CRF 1.D</oeo:OEO_00010037>
        <oeo:OEO_00040001 rdf:datatype="http://www.w3.org/2001/XMLSchema#string">http://openenergy-platform.org/ontology/oeo/oeo-social</oeo:OEO_00040001>
        <obo:IAO_0000115>The CRF sector (IPCC 2006) international bunkers is a transport sector defined by the 2006 IPCC Guidelines for National Greenhouse Gas Inventories. It encompasses international bunkers and multilateral operation.</obo:IAO_0000115>
        <obo:IAO_0000233>issue: https://github.com/OpenEnergyPlatform/ontology/issues/928
pull request: https://github.com/OpenEnergyPlatform/ontology/pull/944</obo:IAO_0000233>
        <rdfs:label xml:lang="en">CRF sector (IPCC 2006): international bunkers and multilateral operations</rdfs:label>
    </owl:NamedIndividual>
    <owl:Axiom>
        <owl:annotatedSource rdf:resource="http://openenergy-platform.org/ontology/oeo/OEO_00010199"/>
        <owl:annotatedProperty rdf:resource="http://www.w3.org/1999/02/22-rdf-syntax-ns#type"/>
        <owl:annotatedTarget>
            <owl:Restriction>
                <owl:onProperty rdf:resource="http://openenergy-platform.org/ontology/oeo/OEO_00010232"/>
                <owl:someValuesFrom rdf:resource="http://openenergy-platform.org/ontology/oeo/OEO_00010227"/>
            </owl:Restriction>
        </owl:annotatedTarget>
        <obo:IAO_0000233>issue: https://github.com/OpenEnergyPlatform/ontology/issues/858
pull request: https://github.com/OpenEnergyPlatform/ontology/pull/965</obo:IAO_0000233>
    </owl:Axiom>
    


    <!-- http://openenergy-platform.org/ontology/oeo/OEO_00010200 -->

    <owl:NamedIndividual rdf:about="http://openenergy-platform.org/ontology/oeo/OEO_00010200">
        <rdf:type rdf:resource="http://openenergy-platform.org/ontology/oeo/OEO_00010320"/>
        <rdf:type>
            <owl:Restriction>
                <owl:onProperty rdf:resource="http://openenergy-platform.org/ontology/oeo/OEO_00010232"/>
                <owl:someValuesFrom rdf:resource="http://openenergy-platform.org/ontology/oeo/OEO_00010227"/>
            </owl:Restriction>
        </rdf:type>
        <rdf:type>
            <owl:Restriction>
                <owl:onProperty rdf:resource="http://openenergy-platform.org/ontology/oeo/OEO_00010232"/>
                <owl:someValuesFrom rdf:resource="http://openenergy-platform.org/ontology/oeo/OEO_00010227"/>
            </owl:Restriction>
        </rdf:type>
        <oeo:OEO_00000504 rdf:resource="http://openenergy-platform.org/ontology/oeo/OEO_00000242"/>
        <obo:BFO_0000051 rdf:resource="http://openenergy-platform.org/ontology/oeo/OEO_00010201"/>
        <obo:BFO_0000051 rdf:resource="http://openenergy-platform.org/ontology/oeo/OEO_00010202"/>
        <oeo:OEO_00010037>CRF 1.D.1</oeo:OEO_00010037>
        <oeo:OEO_00040001 rdf:datatype="http://www.w3.org/2001/XMLSchema#string">http://openenergy-platform.org/ontology/oeo/oeo-social</oeo:OEO_00040001>
        <obo:IAO_0000115>The CRF sector (IPCC 2006) &apos;international bunkers&apos; is a transport sector defined by the 2006 IPCC Guidelines for National Greenhouse Gas Inventories. It encompasses international aviation and maritime navigation.</obo:IAO_0000115>
        <obo:IAO_0000233>issue: https://github.com/OpenEnergyPlatform/ontology/issues/928
pull request: https://github.com/OpenEnergyPlatform/ontology/pull/944

Make instance of &apos;international transport sector&apos;:
issue: https://github.com/OpenEnergyPlatform/ontology/issues/969
pull request: https://github.com/OpenEnergyPlatform/ontology/pull/1334</obo:IAO_0000233>
        <rdfs:label xml:lang="en">CRF sector (IPCC 2006): international bunkers</rdfs:label>
    </owl:NamedIndividual>
    <owl:Axiom>
        <owl:annotatedSource rdf:resource="http://openenergy-platform.org/ontology/oeo/OEO_00010200"/>
        <owl:annotatedProperty rdf:resource="http://www.w3.org/1999/02/22-rdf-syntax-ns#type"/>
        <owl:annotatedTarget>
            <owl:Restriction>
                <owl:onProperty rdf:resource="http://openenergy-platform.org/ontology/oeo/OEO_00010232"/>
                <owl:someValuesFrom rdf:resource="http://openenergy-platform.org/ontology/oeo/OEO_00010227"/>
            </owl:Restriction>
        </owl:annotatedTarget>
        <obo:IAO_0000233>issue: https://github.com/OpenEnergyPlatform/ontology/issues/858
pull request: https://github.com/OpenEnergyPlatform/ontology/pull/965</obo:IAO_0000233>
    </owl:Axiom>
    


    <!-- http://openenergy-platform.org/ontology/oeo/OEO_00010201 -->

    <owl:NamedIndividual rdf:about="http://openenergy-platform.org/ontology/oeo/OEO_00010201">
        <rdf:type rdf:resource="http://openenergy-platform.org/ontology/oeo/OEO_00010320"/>
        <rdf:type>
            <owl:Restriction>
                <owl:onProperty rdf:resource="http://openenergy-platform.org/ontology/oeo/OEO_00010232"/>
                <owl:someValuesFrom rdf:resource="http://openenergy-platform.org/ontology/oeo/OEO_00010227"/>
            </owl:Restriction>
        </rdf:type>
        <rdf:type>
            <owl:Restriction>
                <owl:onProperty rdf:resource="http://openenergy-platform.org/ontology/oeo/OEO_00010232"/>
                <owl:someValuesFrom rdf:resource="http://openenergy-platform.org/ontology/oeo/OEO_00010227"/>
            </owl:Restriction>
        </rdf:type>
        <oeo:OEO_00000504 rdf:resource="http://openenergy-platform.org/ontology/oeo/OEO_00000242"/>
        <obo:BFO_0000050 rdf:resource="http://openenergy-platform.org/ontology/oeo/OEO_00010200"/>
        <oeo:OEO_00010037>CRF 1.D.1.a</oeo:OEO_00010037>
        <oeo:OEO_00040001 rdf:datatype="http://www.w3.org/2001/XMLSchema#string">http://openenergy-platform.org/ontology/oeo/oeo-social</oeo:OEO_00040001>
        <obo:IAO_0000115>The CRF sector (IPCC 2006) &apos;international aviation&apos; is a transport sector defined by the 2006 IPCC Guidelines for National Greenhouse Gas Inventories. It encompasses emissions from flights that depart in one country and arrive in a different country.</obo:IAO_0000115>
        <obo:IAO_0000119>2006 IPCC Guidelines for National Greenhouse Gas Inventories, Volume 1, Chapter 8.5, https://www.ipcc-nggip.iges.or.jp/public/2006gl/</obo:IAO_0000119>
        <obo:IAO_0000233>issue: https://github.com/OpenEnergyPlatform/ontology/issues/928
pull request: https://github.com/OpenEnergyPlatform/ontology/pull/944

Make instance of &apos;international transport sector&apos;:
issue: https://github.com/OpenEnergyPlatform/ontology/issues/969
pull request: https://github.com/OpenEnergyPlatform/ontology/pull/1334</obo:IAO_0000233>
        <rdfs:label xml:lang="en">CRF sector (IPCC 2006): international aviation</rdfs:label>
    </owl:NamedIndividual>
    <owl:Axiom>
        <owl:annotatedSource rdf:resource="http://openenergy-platform.org/ontology/oeo/OEO_00010201"/>
        <owl:annotatedProperty rdf:resource="http://www.w3.org/1999/02/22-rdf-syntax-ns#type"/>
        <owl:annotatedTarget>
            <owl:Restriction>
                <owl:onProperty rdf:resource="http://openenergy-platform.org/ontology/oeo/OEO_00010232"/>
                <owl:someValuesFrom rdf:resource="http://openenergy-platform.org/ontology/oeo/OEO_00010227"/>
            </owl:Restriction>
        </owl:annotatedTarget>
        <obo:IAO_0000233>issue: https://github.com/OpenEnergyPlatform/ontology/issues/858
pull request: https://github.com/OpenEnergyPlatform/ontology/pull/965</obo:IAO_0000233>
    </owl:Axiom>
    


    <!-- http://openenergy-platform.org/ontology/oeo/OEO_00010202 -->

    <owl:NamedIndividual rdf:about="http://openenergy-platform.org/ontology/oeo/OEO_00010202">
        <rdf:type rdf:resource="http://openenergy-platform.org/ontology/oeo/OEO_00010320"/>
        <rdf:type>
            <owl:Restriction>
                <owl:onProperty rdf:resource="http://openenergy-platform.org/ontology/oeo/OEO_00010232"/>
                <owl:someValuesFrom rdf:resource="http://openenergy-platform.org/ontology/oeo/OEO_00010227"/>
            </owl:Restriction>
        </rdf:type>
        <rdf:type>
            <owl:Restriction>
                <owl:onProperty rdf:resource="http://openenergy-platform.org/ontology/oeo/OEO_00010232"/>
                <owl:someValuesFrom rdf:resource="http://openenergy-platform.org/ontology/oeo/OEO_00010227"/>
            </owl:Restriction>
        </rdf:type>
        <oeo:OEO_00000504 rdf:resource="http://openenergy-platform.org/ontology/oeo/OEO_00000242"/>
        <obo:BFO_0000050 rdf:resource="http://openenergy-platform.org/ontology/oeo/OEO_00010200"/>
        <oeo:OEO_00010037>CRF 1.D.1.b</oeo:OEO_00010037>
        <oeo:OEO_00040001 rdf:datatype="http://www.w3.org/2001/XMLSchema#string">http://openenergy-platform.org/ontology/oeo/oeo-social</oeo:OEO_00040001>
        <obo:IAO_0000115>The CRF sector (IPCC 2006) &apos;maritime navigation&apos; is a transport sector defined by the 2006 IPCC Guidelines for National Greenhouse Gas Inventories. Emissions from fuels used by vessels of all flags that are engaged in international water-borne navigation. The international navigation may take place at sea, on inland lakes and waterways and in coastal waters. It includes emissions from journeys that depart in one country and arrive in a different country. It excludes consumption by fishing vessels.</obo:IAO_0000115>
        <obo:IAO_0000119>2006 IPCC Guidelines for National Greenhouse Gas Inventories, Volume 1, Chapter 8.5, https://www.ipcc-nggip.iges.or.jp/public/2006gl/</obo:IAO_0000119>
        <obo:IAO_0000233>issue: https://github.com/OpenEnergyPlatform/ontology/issues/928
pull request: https://github.com/OpenEnergyPlatform/ontology/pull/944

Make instance of &apos;international transport sector&apos;:
issue: https://github.com/OpenEnergyPlatform/ontology/issues/969
pull request: https://github.com/OpenEnergyPlatform/ontology/pull/1334</obo:IAO_0000233>
        <rdfs:label xml:lang="en">CRF sector (IPCC 2006): maritime navigation</rdfs:label>
    </owl:NamedIndividual>
    <owl:Axiom>
        <owl:annotatedSource rdf:resource="http://openenergy-platform.org/ontology/oeo/OEO_00010202"/>
        <owl:annotatedProperty rdf:resource="http://www.w3.org/1999/02/22-rdf-syntax-ns#type"/>
        <owl:annotatedTarget>
            <owl:Restriction>
                <owl:onProperty rdf:resource="http://openenergy-platform.org/ontology/oeo/OEO_00010232"/>
                <owl:someValuesFrom rdf:resource="http://openenergy-platform.org/ontology/oeo/OEO_00010227"/>
            </owl:Restriction>
        </owl:annotatedTarget>
        <obo:IAO_0000233>issue: https://github.com/OpenEnergyPlatform/ontology/issues/858
pull request: https://github.com/OpenEnergyPlatform/ontology/pull/965</obo:IAO_0000233>
    </owl:Axiom>
    


    <!-- http://openenergy-platform.org/ontology/oeo/OEO_00010203 -->

    <owl:NamedIndividual rdf:about="http://openenergy-platform.org/ontology/oeo/OEO_00010203">
        <rdf:type rdf:resource="http://openenergy-platform.org/ontology/oeo/OEO_00000422"/>
        <rdf:type>
            <owl:Restriction>
                <owl:onProperty rdf:resource="http://openenergy-platform.org/ontology/oeo/OEO_00010232"/>
                <owl:someValuesFrom rdf:resource="http://openenergy-platform.org/ontology/oeo/OEO_00010227"/>
            </owl:Restriction>
        </rdf:type>
        <rdf:type>
            <owl:Restriction>
                <owl:onProperty rdf:resource="http://openenergy-platform.org/ontology/oeo/OEO_00010232"/>
                <owl:someValuesFrom rdf:resource="http://openenergy-platform.org/ontology/oeo/OEO_00010227"/>
            </owl:Restriction>
        </rdf:type>
        <oeo:OEO_00000504 rdf:resource="http://openenergy-platform.org/ontology/oeo/OEO_00000242"/>
        <obo:BFO_0000050 rdf:resource="http://openenergy-platform.org/ontology/oeo/OEO_00010199"/>
        <oeo:OEO_00010037>CRF 1.D.2</oeo:OEO_00010037>
        <oeo:OEO_00040001 rdf:datatype="http://www.w3.org/2001/XMLSchema#string">http://openenergy-platform.org/ontology/oeo/oeo-social</oeo:OEO_00040001>
        <obo:IAO_0000115>The CRF sector (IPCC 2006) &apos;multilateral operation&apos; is a transport sector defined by the 2006 IPCC Guidelines for National Greenhouse Gas Inventories:
Emissions from fuels used for aviation and waterborne navigation in multilateral operations pursuant to the Charter of the United Nations.</obo:IAO_0000115>
        <obo:IAO_0000119>2006 IPCC Guidelines for National Greenhouse Gas Inventories, Volume 2, Chapter 3.1, https://www.ipcc-nggip.iges.or.jp/public/2006gl/</obo:IAO_0000119>
        <obo:IAO_0000233>issue: https://github.com/OpenEnergyPlatform/ontology/issues/928
pull request: https://github.com/OpenEnergyPlatform/ontology/pull/944</obo:IAO_0000233>
        <rdfs:label xml:lang="en">CRF sector (IPCC 2006): multilateral operations</rdfs:label>
    </owl:NamedIndividual>
    <owl:Axiom>
        <owl:annotatedSource rdf:resource="http://openenergy-platform.org/ontology/oeo/OEO_00010203"/>
        <owl:annotatedProperty rdf:resource="http://www.w3.org/1999/02/22-rdf-syntax-ns#type"/>
        <owl:annotatedTarget>
            <owl:Restriction>
                <owl:onProperty rdf:resource="http://openenergy-platform.org/ontology/oeo/OEO_00010232"/>
                <owl:someValuesFrom rdf:resource="http://openenergy-platform.org/ontology/oeo/OEO_00010227"/>
            </owl:Restriction>
        </owl:annotatedTarget>
        <obo:IAO_0000233>issue: https://github.com/OpenEnergyPlatform/ontology/issues/858
pull request: https://github.com/OpenEnergyPlatform/ontology/pull/965</obo:IAO_0000233>
    </owl:Axiom>
    


    <!-- http://openenergy-platform.org/ontology/oeo/OEO_00010204 -->

    <owl:NamedIndividual rdf:about="http://openenergy-platform.org/ontology/oeo/OEO_00010204">
        <rdf:type rdf:resource="http://openenergy-platform.org/ontology/oeo/OEO_00000368"/>
        <oeo:OEO_00000503 rdf:resource="http://openenergy-platform.org/ontology/oeo/OEO_00000242"/>
        <oeo:OEO_00040001 rdf:datatype="http://www.w3.org/2001/XMLSchema#string">http://openenergy-platform.org/ontology/oeo/oeo-social</oeo:OEO_00040001>
        <obo:IAO_0000115>The MMR sector division is a sector division defined in Annex XII, Table 1 of Commission Implementing Regulation (EU) 749/2014. It uses CRF sectors (IPCC 2006) and adds further sectors.</obo:IAO_0000115>
        <obo:IAO_0000116>Annex XII, Table 1 of Commission Implementing Regulation (EU) 749/2014 https://eur-lex.europa.eu/legal-content/EN/TXT/HTML/?uri=CELEX:32014R0749&amp;from=EN#d1e32-67-1</obo:IAO_0000116>
        <obo:IAO_0000233>issue: https://github.com/OpenEnergyPlatform/ontology/issues/928
pull request: https://github.com/OpenEnergyPlatform/ontology/pull/944</obo:IAO_0000233>
        <rdfs:label xml:lang="en">MMR sector division</rdfs:label>
    </owl:NamedIndividual>
    


    <!-- http://openenergy-platform.org/ontology/oeo/OEO_00010205 -->

    <owl:NamedIndividual rdf:about="http://openenergy-platform.org/ontology/oeo/OEO_00010205">
        <rdf:type rdf:resource="http://openenergy-platform.org/ontology/oeo/OEO_00010320"/>
        <rdf:type>
            <owl:Restriction>
                <owl:onProperty rdf:resource="http://openenergy-platform.org/ontology/oeo/OEO_00010232"/>
                <owl:someValuesFrom rdf:resource="http://openenergy-platform.org/ontology/oeo/OEO_00010227"/>
            </owl:Restriction>
        </rdf:type>
        <rdf:type>
            <owl:Restriction>
                <owl:onProperty rdf:resource="http://openenergy-platform.org/ontology/oeo/OEO_00010232"/>
                <owl:someValuesFrom rdf:resource="http://openenergy-platform.org/ontology/oeo/OEO_00010227"/>
            </owl:Restriction>
        </rdf:type>
        <oeo:OEO_00000504 rdf:resource="http://openenergy-platform.org/ontology/oeo/OEO_00010204"/>
        <obo:BFO_0000050 rdf:resource="http://openenergy-platform.org/ontology/oeo/OEO_00010133"/>
        <oeo:OEO_00040001 rdf:datatype="http://www.w3.org/2001/XMLSchema#string">http://openenergy-platform.org/ontology/oeo/oeo-social</oeo:OEO_00040001>
        <obo:IAO_0000115>The MMR sector &apos;M.International aviation in the EU ETS&apos; is a transport sector that encompasses that part of the international aviation that is regulated by the European Union Emissions Trading System.</obo:IAO_0000115>
        <obo:IAO_0000233>issue: https://github.com/OpenEnergyPlatform/ontology/issues/928
pull request: https://github.com/OpenEnergyPlatform/ontology/pull/944

Make instance of &apos;international transport sector&apos;:
issue: https://github.com/OpenEnergyPlatform/ontology/issues/969
pull request: https://github.com/OpenEnergyPlatform/ontology/pull/1334</obo:IAO_0000233>
        <rdfs:label xml:lang="en">MMR sector: M.International aviation in the EU ETS</rdfs:label>
    </owl:NamedIndividual>
    <owl:Axiom>
        <owl:annotatedSource rdf:resource="http://openenergy-platform.org/ontology/oeo/OEO_00010205"/>
        <owl:annotatedProperty rdf:resource="http://www.w3.org/1999/02/22-rdf-syntax-ns#type"/>
        <owl:annotatedTarget>
            <owl:Restriction>
                <owl:onProperty rdf:resource="http://openenergy-platform.org/ontology/oeo/OEO_00010232"/>
                <owl:someValuesFrom rdf:resource="http://openenergy-platform.org/ontology/oeo/OEO_00010227"/>
            </owl:Restriction>
        </owl:annotatedTarget>
        <obo:IAO_0000233>issue: https://github.com/OpenEnergyPlatform/ontology/issues/858
pull request: https://github.com/OpenEnergyPlatform/ontology/pull/965</obo:IAO_0000233>
    </owl:Axiom>
    <rdf:Description>
        <rdf:type rdf:resource="http://www.w3.org/2002/07/owl#NegativePropertyAssertion"/>
        <owl:sourceIndividual rdf:resource="http://openenergy-platform.org/ontology/oeo/OEO_00010205"/>
        <owl:assertionProperty rdf:resource="http://openenergy-platform.org/ontology/oeo/OEO_00000504"/>
        <owl:targetIndividual rdf:resource="http://openenergy-platform.org/ontology/oeo/OEO_00010163"/>
    </rdf:Description>
    


    <!-- http://openenergy-platform.org/ontology/oeo/OEO_00010206 -->

    <owl:NamedIndividual rdf:about="http://openenergy-platform.org/ontology/oeo/OEO_00010206">
        <rdf:type rdf:resource="http://openenergy-platform.org/ontology/oeo/OEO_00000367"/>
        <oeo:OEO_00000503 rdf:resource="http://openenergy-platform.org/ontology/oeo/OEO_00000242"/>
        <obo:BFO_0000051 rdf:resource="http://openenergy-platform.org/ontology/oeo/OEO_00010197"/>
        <obo:BFO_0000051 rdf:resource="http://openenergy-platform.org/ontology/oeo/OEO_00010200"/>
        <oeo:OEO_00040001 rdf:datatype="http://www.w3.org/2001/XMLSchema#string">http://openenergy-platform.org/ontology/oeo/oeo-social</oeo:OEO_00040001>
        <obo:IAO_0000115>&apos;Total emissions excluding LULUCF and including international aviation&apos; is a sector that encompasses &apos;CRF sector (IPCC 2006): total emissions excluding LULUCF&apos; and &apos;CRF sector (IPCC 2006): international bunkers&apos;.</obo:IAO_0000115>
        <obo:IAO_0000118>total emissions with international transport (EEA)</obo:IAO_0000118>
        <rdfs:label xml:lang="en">total emissions excluding LULUCF and including international bunkers</rdfs:label>
    </owl:NamedIndividual>
    <owl:Axiom>
        <owl:annotatedSource rdf:resource="http://openenergy-platform.org/ontology/oeo/OEO_00010206"/>
        <owl:annotatedProperty rdf:resource="http://purl.obolibrary.org/obo/IAO_0000118"/>
        <owl:annotatedTarget>total emissions with international transport (EEA)</owl:annotatedTarget>
        <obo:IAO_0000116>Term used by the European Environment Agency (EEA): https://climate-energy.eea.europa.eu/topics/climate-change-mitigation/greenhouse-gas-emissions-inventory/data</obo:IAO_0000116>
    </owl:Axiom>
    


    <!-- http://openenergy-platform.org/ontology/oeo/OEO_00010207 -->

    <owl:NamedIndividual rdf:about="http://openenergy-platform.org/ontology/oeo/OEO_00010207">
        <rdf:type rdf:resource="http://openenergy-platform.org/ontology/oeo/OEO_00000367"/>
        <oeo:OEO_00000503 rdf:resource="http://openenergy-platform.org/ontology/oeo/OEO_00000242"/>
        <obo:BFO_0000051 rdf:resource="http://openenergy-platform.org/ontology/oeo/OEO_00010198"/>
        <obo:BFO_0000051 rdf:resource="http://openenergy-platform.org/ontology/oeo/OEO_00010200"/>
        <oeo:OEO_00040001 rdf:datatype="http://www.w3.org/2001/XMLSchema#string">http://openenergy-platform.org/ontology/oeo/oeo-social</oeo:OEO_00040001>
        <obo:IAO_0000115>&apos;Total emissions excluding LULUCF and including international aviation&apos; is a sector that &apos;CRF sector (IPCC 2006): total emissions including LULUCF&apos; and &apos;CRF sector (IPCC 2006): international bunkers&apos;.</obo:IAO_0000115>
        <obo:IAO_0000118>total net emissions with international transport (EEA)</obo:IAO_0000118>
        <rdfs:label xml:lang="en">total emissions including LULUCF and including international bunkers</rdfs:label>
    </owl:NamedIndividual>
    <owl:Axiom>
        <owl:annotatedSource rdf:resource="http://openenergy-platform.org/ontology/oeo/OEO_00010207"/>
        <owl:annotatedProperty rdf:resource="http://purl.obolibrary.org/obo/IAO_0000118"/>
        <owl:annotatedTarget>total net emissions with international transport (EEA)</owl:annotatedTarget>
        <obo:IAO_0000116>Term used by the European Environment Agency (EEA): https://climate-energy.eea.europa.eu/topics/climate-change-mitigation/greenhouse-gas-emissions-inventory/data</obo:IAO_0000116>
    </owl:Axiom>
    


    <!-- http://openenergy-platform.org/ontology/oeo/OEO_00010208 -->

    <owl:NamedIndividual rdf:about="http://openenergy-platform.org/ontology/oeo/OEO_00010208">
        <rdf:type rdf:resource="http://openenergy-platform.org/ontology/oeo/OEO_00000367"/>
        <oeo:OEO_00000503 rdf:resource="http://openenergy-platform.org/ontology/oeo/OEO_00000242"/>
        <obo:BFO_0000051 rdf:resource="http://openenergy-platform.org/ontology/oeo/OEO_00010197"/>
        <obo:BFO_0000051 rdf:resource="http://openenergy-platform.org/ontology/oeo/OEO_00010201"/>
        <oeo:OEO_00040001 rdf:datatype="http://www.w3.org/2001/XMLSchema#string">http://openenergy-platform.org/ontology/oeo/oeo-social</oeo:OEO_00040001>
        <obo:IAO_0000115>&apos;Total emissions excluding LULUCF and including international aviation&apos; is a sector that encompasses &apos;CRF sector (IPCC 2006): total emissions excluding LULUCF&apos; and &apos;CRF sector (IPCC 2006): international aviation&apos;.</obo:IAO_0000115>
        <obo:IAO_0000116>This definition corresponds to the 2020 emission target of the European Union.</obo:IAO_0000116>
        <obo:IAO_0000118>total emissions with international aviation (EU 2020)</obo:IAO_0000118>
        <obo:IAO_0000233>issue: https://github.com/OpenEnergyPlatform/ontology/issues/928
pull request: https://github.com/OpenEnergyPlatform/ontology/pull/944</obo:IAO_0000233>
        <rdfs:label xml:lang="en">total emissions excluding LULUCF and including international aviation</rdfs:label>
    </owl:NamedIndividual>
    <owl:Axiom>
        <owl:annotatedSource rdf:resource="http://openenergy-platform.org/ontology/oeo/OEO_00010208"/>
        <owl:annotatedProperty rdf:resource="http://purl.obolibrary.org/obo/IAO_0000118"/>
        <owl:annotatedTarget>total emissions with international aviation (EU 2020)</owl:annotatedTarget>
        <obo:IAO_0000116>Term used by the European Environment Agency (EEA): https://climate-energy.eea.europa.eu/topics/climate-change-mitigation/greenhouse-gas-emissions-inventory/data</obo:IAO_0000116>
    </owl:Axiom>
    


    <!-- http://openenergy-platform.org/ontology/oeo/OEO_00010209 -->

    <owl:NamedIndividual rdf:about="http://openenergy-platform.org/ontology/oeo/OEO_00010209">
        <rdf:type rdf:resource="http://openenergy-platform.org/ontology/oeo/OEO_00000367"/>
        <oeo:OEO_00000503 rdf:resource="http://openenergy-platform.org/ontology/oeo/OEO_00000242"/>
        <obo:BFO_0000051 rdf:resource="http://openenergy-platform.org/ontology/oeo/OEO_00010198"/>
        <obo:BFO_0000051 rdf:resource="http://openenergy-platform.org/ontology/oeo/OEO_00010201"/>
        <oeo:OEO_00040001 rdf:datatype="http://www.w3.org/2001/XMLSchema#string">http://openenergy-platform.org/ontology/oeo/oeo-social</oeo:OEO_00040001>
        <obo:IAO_0000115>&apos;Total emissions excluding LULUCF and including international aviation&apos; is a sector that &apos;CRF sector (IPCC 2006): total emissions including LULUCF&apos; and &apos;CRF sector (IPCC 2006): international aviation&apos;.</obo:IAO_0000115>
        <obo:IAO_0000116>This definition corresponds to the 2030 emission target as specified in the Nationally Determined Contribution (NDC) of the European Union .</obo:IAO_0000116>
        <obo:IAO_0000118>total net emissions with international aviation (NDC)</obo:IAO_0000118>
        <obo:IAO_0000233>issue: https://github.com/OpenEnergyPlatform/ontology/issues/928
pull request: https://github.com/OpenEnergyPlatform/ontology/pull/944</obo:IAO_0000233>
        <rdfs:label xml:lang="en">total emissions including LULUCF and including international aviation</rdfs:label>
    </owl:NamedIndividual>
    <owl:Axiom>
        <owl:annotatedSource rdf:resource="http://openenergy-platform.org/ontology/oeo/OEO_00010209"/>
        <owl:annotatedProperty rdf:resource="http://purl.obolibrary.org/obo/IAO_0000118"/>
        <owl:annotatedTarget>total net emissions with international aviation (NDC)</owl:annotatedTarget>
        <obo:IAO_0000116>Term used by the European Environment Agency (EEA): https://climate-energy.eea.europa.eu/topics/climate-change-mitigation/greenhouse-gas-emissions-inventory/data</obo:IAO_0000116>
    </owl:Axiom>
    


    <!-- http://openenergy-platform.org/ontology/oeo/OEO_00010228 -->

    <owl:NamedIndividual rdf:about="http://openenergy-platform.org/ontology/oeo/OEO_00010228">
        <rdf:type rdf:resource="http://openenergy-platform.org/ontology/oeo/OEO_00000367"/>
        <rdf:type>
            <owl:Restriction>
                <owl:onProperty rdf:resource="http://openenergy-platform.org/ontology/oeo/OEO_00010232"/>
                <owl:someValuesFrom rdf:resource="http://openenergy-platform.org/ontology/oeo/OEO_00010227"/>
            </owl:Restriction>
        </rdf:type>
        <oeo:OEO_00000504 rdf:resource="http://openenergy-platform.org/ontology/oeo/OEO_00000242"/>
        <oeo:OEO_00040001 rdf:datatype="http://www.w3.org/2001/XMLSchema#string">http://openenergy-platform.org/ontology/oeo/oeo-social</oeo:OEO_00040001>
        <obo:IAO_0000115>The CRF sector (IPCC 2006): &apos;CO2 emissions from biomass&apos; is a sector defined by the 2006 IPCC Guidelines for National Greenhouse Gas Inventories: CO2 emissions from biomass combustion are not included in national totals, but are recorded as an information item for cross-checking purposes as well as avoiding double counting.</obo:IAO_0000115>
        <obo:IAO_0000119>2006 IPCC Guidelines for National Greenhouse Gas Inventories, Volume 2, Chapter 1, https://www.ipcc-nggip.iges.or.jp/public/2006gl/</obo:IAO_0000119>
        <obo:IAO_0000233>issue: https://github.com/OpenEnergyPlatform/ontology/issues/858
pull request: https://github.com/OpenEnergyPlatform/ontology/pull/965</obo:IAO_0000233>
        <rdfs:label xml:lang="en">CRF sector (IPCC 2006): CO2 emissions from biomass</rdfs:label>
    </owl:NamedIndividual>
    


    <!-- http://openenergy-platform.org/ontology/oeo/OEO_00010229 -->

    <owl:NamedIndividual rdf:about="http://openenergy-platform.org/ontology/oeo/OEO_00010229">
        <rdf:type rdf:resource="http://openenergy-platform.org/ontology/oeo/OEO_00000367"/>
        <rdf:type>
            <owl:Restriction>
                <owl:onProperty rdf:resource="http://openenergy-platform.org/ontology/oeo/OEO_00010232"/>
                <owl:someValuesFrom rdf:resource="http://openenergy-platform.org/ontology/oeo/OEO_00010227"/>
            </owl:Restriction>
        </rdf:type>
        <oeo:OEO_00000504 rdf:resource="http://openenergy-platform.org/ontology/oeo/OEO_00000242"/>
        <oeo:OEO_00040001 rdf:datatype="http://www.w3.org/2001/XMLSchema#string">http://openenergy-platform.org/ontology/oeo/oeo-social</oeo:OEO_00040001>
        <obo:IAO_0000115>The CRF sector (IPCC 2006): &apos;CO2 captured&apos; is a sector defined by the 2006 IPCC Guidelines for National Greenhouse Gas Inventories: It encompasses the total amount of CO2 captured for storage.</obo:IAO_0000115>
        <obo:IAO_0000119>2006 IPCC Guidelines for National Greenhouse Gas Inventories, Volume 2, Chapter 5.9, https://www.ipcc-nggip.iges.or.jp/public/2006gl/</obo:IAO_0000119>
        <obo:IAO_0000233>issue: https://github.com/OpenEnergyPlatform/ontology/issues/858
pull request: https://github.com/OpenEnergyPlatform/ontology/pull/965</obo:IAO_0000233>
        <rdfs:label xml:lang="en">CRF sector (IPCC 2006): CO2 captured</rdfs:label>
    </owl:NamedIndividual>
    


    <!-- http://openenergy-platform.org/ontology/oeo/OEO_00010230 -->

    <owl:NamedIndividual rdf:about="http://openenergy-platform.org/ontology/oeo/OEO_00010230">
        <rdf:type rdf:resource="http://openenergy-platform.org/ontology/oeo/OEO_00000367"/>
        <rdf:type>
            <owl:Restriction>
                <owl:onProperty rdf:resource="http://openenergy-platform.org/ontology/oeo/OEO_00010232"/>
                <owl:someValuesFrom rdf:resource="http://openenergy-platform.org/ontology/oeo/OEO_00010227"/>
            </owl:Restriction>
        </rdf:type>
        <oeo:OEO_00000504 rdf:resource="http://openenergy-platform.org/ontology/oeo/OEO_00000242"/>
        <oeo:OEO_00040001 rdf:datatype="http://www.w3.org/2001/XMLSchema#string">http://openenergy-platform.org/ontology/oeo/oeo-social</oeo:OEO_00040001>
        <obo:IAO_0000115>The CRF sector (IPCC 2006): &apos;indirect CO2&apos; is a sector defined by the 2006 IPCC Guidelines for National Greenhouse Gas Inventories: It encompasses Methane, carbon monoxide (CO) or NMVOC emissions that will eventually be oxidised to CO2 in the atmosphere.</obo:IAO_0000115>
        <obo:IAO_0000119>2006 IPCC Guidelines for National Greenhouse Gas Inventories, Volume 1, Chapter 7.2.1.5, https://www.ipcc-nggip.iges.or.jp/public/2006gl/</obo:IAO_0000119>
        <obo:IAO_0000233>issue: https://github.com/OpenEnergyPlatform/ontology/issues/858
pull request: https://github.com/OpenEnergyPlatform/ontology/pull/965</obo:IAO_0000233>
        <rdfs:label xml:lang="en">CRF sector (IPCC 2006): indirect CO2</rdfs:label>
    </owl:NamedIndividual>
    


    <!-- http://openenergy-platform.org/ontology/oeo/OEO_00010304 -->

    <owl:NamedIndividual rdf:about="http://openenergy-platform.org/ontology/oeo/OEO_00010304">
        <rdf:type rdf:resource="http://openenergy-platform.org/ontology/oeo/OEO_00000368"/>
        <obo:IAO_0000115>The NC/BR sector division is a sector division defined by the UNFCCC reporting guidelines on national communications for Parties included in Annex I to the Convention.
(https://unfccc.int/sites/default/files/resource/cp2019_13a01_adv.pdf, 6/CP.25, VI, Table 2)</obo:IAO_0000115>
        <obo:IAO_0000233>issue: https://github.com/OpenEnergyPlatform/ontology/issues/1273
pull request: https://github.com/OpenEnergyPlatform/ontology/pull/1317</obo:IAO_0000233>
        <rdfs:label xml:lang="en">NC/BR sector division</rdfs:label>
    </owl:NamedIndividual>
    


    <!-- http://openenergy-platform.org/ontology/oeo/OEO_00010305 -->

    <owl:NamedIndividual rdf:about="http://openenergy-platform.org/ontology/oeo/OEO_00010305">
        <rdf:type rdf:resource="http://openenergy-platform.org/ontology/oeo/OEO_00000367"/>
        <oeo:OEO_00000504 rdf:resource="http://openenergy-platform.org/ontology/oeo/OEO_00010304"/>
        <obo:BFO_0000051 rdf:resource="http://openenergy-platform.org/ontology/oeo/OEO_00010040"/>
        <obo:BFO_0000051 rdf:resource="http://openenergy-platform.org/ontology/oeo/OEO_00010043"/>
        <obo:BFO_0000051 rdf:resource="http://openenergy-platform.org/ontology/oeo/OEO_00010044"/>
        <obo:BFO_0000051 rdf:resource="http://openenergy-platform.org/ontology/oeo/OEO_00010057"/>
        <obo:BFO_0000051 rdf:resource="http://openenergy-platform.org/ontology/oeo/OEO_00010058"/>
        <obo:IAO_0000115>The NC/BR sector &quot;energy&quot; is a sector defined by the NC/BR sector division that includes all energy use that is not related to transport or industry. The sector includes:
- CRF sector (IPCC 2006): energy industry
- CRF sector (IPCC 2006): fuel combustion - other sectors
- CRF sector (IPCC 2006): fuel combustion - other
- CRF sector (IPCC 2006): fugitive emissions from fuels
- CRF sector (IPCC 2006): CO2 transport and storage</obo:IAO_0000115>
        <obo:IAO_0000233>issue: https://github.com/OpenEnergyPlatform/ontology/issues/1273
pull request: https://github.com/OpenEnergyPlatform/ontology/pull/1317</obo:IAO_0000233>
        <rdfs:label xml:lang="en">NC/BR sector: energy</rdfs:label>
    </owl:NamedIndividual>
    


    <!-- http://openenergy-platform.org/ontology/oeo/OEO_00010306 -->

    <owl:NamedIndividual rdf:about="http://openenergy-platform.org/ontology/oeo/OEO_00010306">
        <rdf:type rdf:resource="http://openenergy-platform.org/ontology/oeo/OEO_00000422"/>
        <oeo:OEO_00000504 rdf:resource="http://openenergy-platform.org/ontology/oeo/OEO_00010304"/>
        <obo:IAO_0000115>The NC/BR sector &quot;transport&quot; is a transport sector defined by the NC/BR sector division. It aligns to the CRF sector (IPCC 2006): transport.</obo:IAO_0000115>
        <obo:IAO_0000233>issue: https://github.com/OpenEnergyPlatform/ontology/issues/1273
pull request: https://github.com/OpenEnergyPlatform/ontology/pull/1317</obo:IAO_0000233>
        <rdfs:label xml:lang="en">NC/BR sector: transport</rdfs:label>
    </owl:NamedIndividual>
    


    <!-- http://openenergy-platform.org/ontology/oeo/OEO_00010307 -->

    <owl:NamedIndividual rdf:about="http://openenergy-platform.org/ontology/oeo/OEO_00010307">
        <rdf:type rdf:resource="http://openenergy-platform.org/ontology/oeo/OEO_00000227"/>
        <oeo:OEO_00000504 rdf:resource="http://openenergy-platform.org/ontology/oeo/OEO_00010304"/>
        <obo:BFO_0000051 rdf:resource="http://openenergy-platform.org/ontology/oeo/OEO_00010046"/>
        <obo:BFO_0000051 rdf:resource="http://openenergy-platform.org/ontology/oeo/OEO_00010160"/>
        <obo:IAO_0000115>The NC/BR sector &quot;industry/industrial processes and product use&quot; is an industry sector defined by the NC/BR sector division. The sector includes:
- CRF sector (IPCC 2006): manufacture of solid fuels and other energy industries
- CRF sector (IPCC 2006): industrial processes and product use</obo:IAO_0000115>
        <obo:IAO_0000233>issue: https://github.com/OpenEnergyPlatform/ontology/issues/1273
pull request: https://github.com/OpenEnergyPlatform/ontology/pull/1317</obo:IAO_0000233>
        <rdfs:label xml:lang="en">NC/BR sector: industry/industrial processes and product use</rdfs:label>
    </owl:NamedIndividual>
    


    <!-- http://openenergy-platform.org/ontology/oeo/OEO_00010308 -->

    <owl:NamedIndividual rdf:about="http://openenergy-platform.org/ontology/oeo/OEO_00010308">
        <rdf:type rdf:resource="http://openenergy-platform.org/ontology/oeo/OEO_00010035"/>
        <obo:IAO_0000115>The NC/BR sector &quot;agriculture&quot; is an agriculture, forestry and land use sector defined by the NC/BR sector division. It aligns to the CRF sector (IPCC 2006): agriculture.</obo:IAO_0000115>
        <obo:IAO_0000233>issue: https://github.com/OpenEnergyPlatform/ontology/issues/1273
pull request: https://github.com/OpenEnergyPlatform/ontology/pull/1317</obo:IAO_0000233>
        <rdfs:label xml:lang="en">NC/BR sector: agriculture</rdfs:label>
    </owl:NamedIndividual>
    


    <!-- http://openenergy-platform.org/ontology/oeo/OEO_00010309 -->

    <owl:NamedIndividual rdf:about="http://openenergy-platform.org/ontology/oeo/OEO_00010309">
        <rdf:type rdf:resource="http://openenergy-platform.org/ontology/oeo/OEO_00010035"/>
        <oeo:OEO_00000504 rdf:resource="http://openenergy-platform.org/ontology/oeo/OEO_00010304"/>
        <obo:IAO_0000115>The NC/BR sector &quot;forestry/LULUCF&quot; is an agriculture, forestry and land use sector defined by the NC/BR sector division. It aligns to the CRF sector (IPCC 2006): land use, land-use change and forestry.</obo:IAO_0000115>
        <obo:IAO_0000233>issue: https://github.com/OpenEnergyPlatform/ontology/issues/1273
pull request: https://github.com/OpenEnergyPlatform/ontology/pull/1317</obo:IAO_0000233>
        <rdfs:label xml:lang="en">NC/BR sector: forestry/LULUCF</rdfs:label>
    </owl:NamedIndividual>
    


    <!-- http://openenergy-platform.org/ontology/oeo/OEO_00010310 -->

    <owl:NamedIndividual rdf:about="http://openenergy-platform.org/ontology/oeo/OEO_00010310">
        <rdf:type rdf:resource="http://openenergy-platform.org/ontology/oeo/OEO_00010036"/>
        <oeo:OEO_00000504 rdf:resource="http://openenergy-platform.org/ontology/oeo/OEO_00010304"/>
        <obo:IAO_0000115>The NC/BR sector &quot;waste management/waste&quot; is a waste and wastewater sector defined by the NC/BR sector division. It aligns to the CRF sector (IPCC 2006): waste.</obo:IAO_0000115>
        <obo:IAO_0000233>issue: https://github.com/OpenEnergyPlatform/ontology/issues/1273
pull request: https://github.com/OpenEnergyPlatform/ontology/pull/1317</obo:IAO_0000233>
        <rdfs:label xml:lang="en">NC/BR sector: waste management/waste</rdfs:label>
    </owl:NamedIndividual>
    


    <!-- http://openenergy-platform.org/ontology/oeo/OEO_00010311 -->

    <owl:NamedIndividual rdf:about="http://openenergy-platform.org/ontology/oeo/OEO_00010311">
        <rdf:type rdf:resource="http://openenergy-platform.org/ontology/oeo/OEO_00000367"/>
        <oeo:OEO_00000504 rdf:resource="http://openenergy-platform.org/ontology/oeo/OEO_00010304"/>
        <obo:IAO_0000115>The NC/BR sector &quot;other&quot; is a sector defined by the NC/BR sector division that includes everything that is not included in the other NC/BR sectors. It aligns to the CRF sector (IPCC 2006): other.</obo:IAO_0000115>
        <obo:IAO_0000233>issue: https://github.com/OpenEnergyPlatform/ontology/issues/1273
pull request: https://github.com/OpenEnergyPlatform/ontology/pull/1317</obo:IAO_0000233>
        <rdfs:label xml:lang="en">NC/BR sector: other</rdfs:label>
    </owl:NamedIndividual>
    


    <!-- 
    ///////////////////////////////////////////////////////////////////////////////////////
    //
    // General axioms
    //
    ///////////////////////////////////////////////////////////////////////////////////////
     -->

    <rdf:Description>
        <rdf:type rdf:resource="http://www.w3.org/2002/07/owl#AllDisjointClasses"/>
        <owl:members rdf:parseType="Collection">
            <rdf:Description rdf:about="http://openenergy-platform.org/ontology/oeo/OEO_00000145"/>
            <rdf:Description rdf:about="http://openenergy-platform.org/ontology/oeo/OEO_00000213"/>
            <rdf:Description rdf:about="http://openenergy-platform.org/ontology/oeo/OEO_00000422"/>
        </owl:members>
    </rdf:Description>
    <rdf:Description>
        <rdf:type rdf:resource="http://www.w3.org/2002/07/owl#AllDifferent"/>
        <owl:distinctMembers rdf:parseType="Collection">
            <rdf:Description rdf:about="http://openenergy-platform.org/ontology/oeo/OEO_00010058"/>
            <rdf:Description rdf:about="http://openenergy-platform.org/ontology/oeo/OEO_00010229"/>
        </owl:distinctMembers>
    </rdf:Description>
    <rdf:Description>
        <rdf:type rdf:resource="http://www.w3.org/2002/07/owl#AllDifferent"/>
        <owl:distinctMembers rdf:parseType="Collection">
            <rdf:Description rdf:about="http://openenergy-platform.org/ontology/oeo/OEO_00010059"/>
            <rdf:Description rdf:about="http://openenergy-platform.org/ontology/oeo/OEO_00010201"/>
        </owl:distinctMembers>
    </rdf:Description>
    <rdf:Description>
        <rdf:type rdf:resource="http://www.w3.org/2002/07/owl#AllDifferent"/>
        <owl:distinctMembers rdf:parseType="Collection">
            <rdf:Description rdf:about="http://openenergy-platform.org/ontology/oeo/OEO_00010062"/>
            <rdf:Description rdf:about="http://openenergy-platform.org/ontology/oeo/OEO_00010202"/>
        </owl:distinctMembers>
    </rdf:Description>
    <rdf:Description>
        <rdf:type rdf:resource="http://www.w3.org/2002/07/owl#AllDifferent"/>
        <owl:distinctMembers rdf:parseType="Collection">
            <rdf:Description rdf:about="http://openenergy-platform.org/ontology/oeo/OEO_00010305"/>
            <rdf:Description rdf:about="http://openenergy-platform.org/ontology/oeo/OEO_00010306"/>
            <rdf:Description rdf:about="http://openenergy-platform.org/ontology/oeo/OEO_00010307"/>
            <rdf:Description rdf:about="http://openenergy-platform.org/ontology/oeo/OEO_00010308"/>
            <rdf:Description rdf:about="http://openenergy-platform.org/ontology/oeo/OEO_00010309"/>
            <rdf:Description rdf:about="http://openenergy-platform.org/ontology/oeo/OEO_00010310"/>
            <rdf:Description rdf:about="http://openenergy-platform.org/ontology/oeo/OEO_00010311"/>
        </owl:distinctMembers>
    </rdf:Description>
</rdf:RDF>



<!-- Generated by the OWL API (version 4.5.6) https://github.com/owlcs/owlapi -->

